@prefix :          <https://vocabs.alliander.com/terms/> .
@prefix skos:      <http://www.w3.org/2004/02/skos/core#> .
@prefix dc:        <http://purl.org/dc/elements/1.1/> .
@prefix dct:       <http://purl.org/dc/terms/> .
@prefix dcat:      <http://www.w3.org/ns/dcat#> .
@prefix xsd:       <http://www.w3.org/2001/XMLSchema#> .
@prefix owl:       <http://www.w3.org/2002/07/owl#> .
@prefix foaf:      <http://xmlns.com/foaf/0.1/> .
@prefix rdfs:      <http://www.w3.org/2000/01/rdf-schema#> .

@prefix cim:       <http://iec.ch/TC57/ns/CIM/> .
@prefix eq:        <http://iec.ch/TC57/ns/CIM/CoreEquipment-EU/> .
@prefix op:        <http://iec.ch/TC57/ns/CIM/Operation-EU/> .
@prefix tp:        <http://iec.ch/TC57/ns/CIM/Topology-EU/> .
@prefix ssh:       <http://iec.ch/TC57/ns/CIM/StateVariables-EU/> .
@prefix dsm:       <http://iec.ch/TC57/2013/IEC62746/> .
@prefix maw:       <http://iec.ch/TC57/2013/IEC62325/> .
@prefix amw:       <http://iec.ch/TC57/IEC61968/> .
@prefix hemrm:     <http://vocabs.entsoe.com/terms/> .
@prefix elit:      <http://data.europa.eu/eli/terms/> .
@prefix eli:       <http://data.europa.eu/eli/ontology#> .
@prefix lido37940: <http://linkeddata.overheid.nl/terms/BWBR0037940/> .
@prefix lido50714: <http://linkeddata.overheid.nl/terms/BWBR0050714/> .
@prefix archi:     <http://www.opengroup.org/archimate/3.2/> .

:Ontology
  a               owl:Ontology, skos:ConceptScheme ;
  skos:prefLabel  "Energy System Concept Scheme"@en, "Energie System Begrippenkader"@nl ;
  dct:description "Terminology that Energy System Architecture (ESA) uses in its publications"@en,
                  "Begrippen die Energie System Architectuur (ESA) in zijn publicaties hanteert"@nl ;
  dct:identifier  "urn:uuid:48170043-3c6d-476d-b5d6-452bec944f42" ;
  dct:publisher   "Alliander"@en ;
  dct:creator     "Alliander"@en ;
  dct:created     "2025-04-20"^^xsd:date ;
  dct:modified    "2025-07-11"^^xsd:date ;
  dcat:theme      "vocabulary"@en ;
  rdfs:seeAlso    "https://www.electropedia.org/" ;
  rdfs:seeAlso    "https://begrippen.netbeheernederland.nl/energiesysteembeheer/nl/index" ;
  rdfs:seeAlso    <https://netbeheer-nederland.github.io/docs/> ;
  rdfs:seeAlso    <https://www.acm.nl/nl/energie/wetten-en-regels-voor-de-energiemarkt> ;
  owl:versionIRI  <http://vocabs.alliander.com/terms/20250605> .

# Definition and abbreviations

### skos:Collections
:4000
  a              skos:Collection ;
  skos:prefLabel "Operational Limit Collection"@en, "Operationele Limiet Collectie"@nl ;
  skos:definition
                 """A collection of terms and definitions in relation to the operating boundaries for secure grid operation."""@en,
                 """Een verzameling termen en definities met betrekking tot de operationele grenzen voor veilige netwerkexploitatie."""@nl ;
  skos:member    :4006, :4007 ;
  skos:inScheme  :Ontology ;
  dcat:theme     "vocabulary"@en .

:4001
  a               skos:Collection ;
  skos:prefLabel  "Asset Limit Collection"@en, "Fysieke Component Limiet Collectie"@nl ;
  skos:definition """A collection of terms and definitions in relation to the capacity rating of assets."""@en,
                  """Een verzameling termen en definities met betrekking tot de capaciteitsclassificatie van componenten."""@nl ;
  skos:member     :68, :116, :117 ;
  skos:related    amw:Asset ;
  skos:inScheme   :Ontology ;
  dcat:theme      "vocabulary"@en .

:4002
  a               skos:Collection ;
  skos:prefLabel  "Equipment Type Collection"@en, "Functionele Component Collectie"@nl ;
  skos:definition """A collection of terms and definitions related to equipments in the electrical grid."""@en,
                  """Een verzameling termen en definities met betrekking tot functionele componenten in het elektriciteitsnet."""@nl ;
  skos:member     :74, :73, :70, :105, :107, :69, :32, :64, :49, :119, :120 ;
  skos:related    eq:ConductingEquipment ;
  skos:inScheme   :Ontology ;
  dcat:theme      "vocabulary"@en .

:4003
  a                 skos:Collection ;
  skos:prefLabel    "Market Participant Collection"@en, "Marktdeelnemer Collectie"@nl ;
  skos:definition   """A collection of terms and definitions related to the actors and roles related to a market participant."""@en,
                    """Een verzameling termen en definities met betrekking tot actoren en rollen tot een marktdeelnemer."""@nl ;
  skos:member       :4004, :4005 ;
  skos:member       :76 ;
  skos:relatedMatch elit:944-25 ;
  skos:exactMatch   elit:943-25, maw:MarketParticipant ;
  skos:inScheme     :Ontology ;
  dcat:theme        "vocabulary"@en .

:4004
  a               skos:Collection ;
  skos:prefLabel  "Customer Collection"@en, "Klant Collectie"@nl ;
  skos:definition """A collection of terms and definitions related to the role 'Customer'."""@en,
                  """Een verzameling termen en definities met betrekking tot de rol 'Klant'."""@nl ;
  skos:member     :23 ;
  skos:inScheme   :Ontology ;
  dcat:theme      "vocabulary"@en .

:4005
  a               skos:Collection ;
  skos:prefLabel  "Flexibility Service Provider Collection"@en, "Flexibiliteitsdienstverlener Collectie"@nl ;
  skos:definition """A collection of terms and definitions related to the role 'Flexibility Service Provider'."""@en,
                  """Een verzameling termen en definities met betrekking tot de rol 'Flexibiliteitsdienstverlener'."""@nl ;
  skos:member     :23 ;
  skos:inScheme   :Ontology ;
  dcat:theme      "vocabulary"@en .

:4006
  a               skos:Collection ;
  skos:prefLabel  "Equipment Limit Collection"@en, ""@nl ;
  skos:definition """A collection of terms and definitions related to the role 'Flexibility Service Provider'."""@en,
                  """Een verzameling termen en definities met betrekking tot de rol 'Flexibiliteitsdienstverlener'."""@nl ;
  skos:member     :71, :113, :114, :116, :133, :134 ;
  skos:inScheme   :Ontology ;
  dcat:theme      "vocabulary"@en .

:4007
  a               skos:Collection ;
  skos:prefLabel  "Equipment Limit Violation"@en, "Component limiet overschrijding"@nl ;
  skos:definition """A collection of terms and definitions related to the 'Equipment Limit Violation'."""@en,
                  """Een verzameling termen en definities met betrekking tot de 'Flexibiliteitsdienstverlener'."""@nl ;
  skos:member     :77, :78, :79, :80 ;
  skos:inScheme   :Ontology ;
  dcat:theme      "vocabulary"@en .

:4008
  a              skos:Collection ;
  skos:prefLabel "Grid Operators Platform for Congestion Solutions"@en,
                 "Grid Operators Platform for Congestion Solutions"@nl ;
  skos:altLabel  "GOPACS" ;
  skos:definition
                 """A collection of terms and definitions related to the 'Grid Operators Platform for Congestion Solutions'."""@en,
                 """Een verzameling termen en definities met betrekking tot de 'Grid Operators Platform for Congestion Solutions'."""@nl ;
  skos:member    :328, :329, :330, :331, :332, :333, :334 ;
  skos:inScheme   :Ontology ;
  dcat:theme      "vocabulary"@en .


### rdfs Classes
foaf:Agent
  a          rdfs:Class ;
  rdfs:label "Agent" .

:begrippencode-elektriciteit-BWBR0037938
  a              foaf:Document ;
  skos:prefLabel "Concept code electricity"@en, "Begrippencode elektriciteit"@nl ;
  foaf:page      <https://wetten.overheid.nl/jci1.3:c:BWBR0037938> .

### skos:Concepts
:1
  a                 skos:Concept ;
  skos:prefLabel    "Afroepbaar Vermogen"@nl, "Demandable Capacity"@en ;
  skos:altLabel     "Demandable Power"@en ;
  skos:definition   "Het verschil tussen de hoge en lage vermogensgrens."@nl,
                    "The difference between a high and low power limit."@en ;
  dc:source         "B4401" ;
  dct:identifier    "urn:uuid:26dc929b-57da-4002-81e9-f212f72e4fd1" ;
  owl:versionInfo   1 ;
  skos:topConceptOf :Ontology ;
  skos:inScheme     :Ontology .

:2
  a                 skos:Concept ;
  skos:prefLabel    "Aanwezige Transportcapaciteit"@nl, "Available Transport Capacity"@en ;
  skos:definition   "De maximale capaciteit dat een net aan kan, met inachtneming van de van toepassing zijnde netontwerpcriteria en operationele veiligheidsgrenzen."@nl,
                    "The maximum capacity that a grid can handle, subject to applicable grid design criteria and operational safety limits."@en ;
  dc:source         "B4401" ;
  dct:identifier    "urn:uuid:26dc929b-57da-4002-81e9-f212f72e4fd2" ;
  owl:versionInfo   1 ;
  skos:topConceptOf :Ontology ;
  skos:inScheme     :Ontology .

:3
  a                 skos:Concept ;
  skos:prefLabel    "Demandable Period"@en, "Afroepbare Periodes"@nl ;
  skos:definition   "Dit zijn de tussen de klant en de netbeheerder overeengekomen tijdssloten waarin door de netbeheerder een afregelverzoek mag worden geplaatst."@nl,
                    "These are the time slots agreed upon between the customer and the grid operator in which an adjustment request may be placed by the grid operator."@en ;
  skos:altLabel     "Availability Windows"@en, "Beschikbaarheidsvenster"@nl ;
  dc:source         "B4401" ;
  dct:identifier    "urn:uuid:26dc929b-57da-4002-81e9-f212f72e4fd3" ;
  owl:versionInfo   1 ;
  skos:topConceptOf :Ontology ;
  skos:inScheme     :Ontology .

:4
  a                 skos:Concept ;
  skos:prefLabel    "Afroepbaar Vermogen Limiet"@nl, "Demandable Capacity Limit"@en ;
  skos:altLabel     "Afroeplimiet"@nl ;
  skos:definition   "Dit is de limiet die de klant krijgt opgelegd tijdens de afroep. Een klant mag niet boven deze limiet uitkomen."@nl ;
  dc:source         "B4401" ;
  dct:identifier    "urn:uuid:51cbc2cf-7450-5bc1-b04f-a44780b52c86" ;
  owl:versionInfo   "1" ;
  skos:exactMatch   elit:1485-2 ;
  skos:topConceptOf :Ontology ;
  skos:inScheme     :Ontology .

:5
  a                 skos:Concept ;
  skos:prefLabel    "Unused Capacity"@en, "Capaciteit niet in gebruik"@nl ;
  skos:definition   "Vaak zal de klant niet zijn volledige GTV gebruiken, en dus een deel van zijn capaciteit niet gebruiken. Dit deel is dan ook niet effectief beschikbaar om afgeroepen te worden en hiermee wordt rekening gehouden in de afroep."@nl ;
  dc:source         "B4401" ;
  dct:identifier    "urn:uuid:97be4ed2-2940-53e0-be5d-8d34155cb241" ;
  owl:versionInfo   "1" ;
  skos:topConceptOf :Ontology ;
  skos:inScheme     :Ontology .

:6
  a                  skos:Concept ;
  skos:prefLabel     "Day-Ahead Market"@en, "Day-ahead handel"@nl ;
  skos:altLabel      "DAM"@nl ;
  skos:definition    "Day-ahead handel verwijst naar de handel in elektriciteit voor de volgende dag, die bijvoorbeeld plaatsvindt op EPEX Spot in Parijs (spotmarkt van EEX, de European Power Exchange), op EXAA in Wenen (Energy Exchange Austria), of in bilaterale OTC-contracten (Over-the-Counter Trading). De EPEX Spotmarkt is onderverdeeld in verschillende marktgebieden: België, Nederland, Frankrijk, Zwitserland, Duitsland en Oostenrijk, Verenigd Koninkrijk, en sinds kort ook de Scandinavische landen. Voor de afzonderlijke marktregio's verschilt de handel verder afhankelijk van de respectieve transmissienetbeheerders. Op de gekoppelde nationale markten, moeten de marktdeelnemers hun biedingen voor de veilingen van de volgende dag elke dag vóór 12.00 uur indienen. De marktresultaten worden elke dag om 12.40 uur gepubliceerd en de marktdeelnemers worden geïnformeerd over het succes van hun biedingen."@nl ;
  skos:editorialNote """The day ahead market which determines the commitment and schedules of resources."""@en ;
  dc:source          "B4401" ;
  dct:identifier     "urn:uuid:46e54699-fcc2-599f-af8c-3de1b0a2322d" ;
  owl:versionInfo    "1" ;
  skos:broadMatch    elit:1222-34 ;
  skos:topConceptOf  :Ontology ;
  skos:inScheme      :Ontology .

:7
  a                 skos:Concept ;
  skos:prefLabel    "Effective demand"@en, "Effectieve afroep"@nl ;
  skos:definition   """Mocht de klant zijn volledige GTV gebruiken (en dus exact op de hoge vermogensgrens zitten), dan is het afroepbaar vermogen ook de maximale hoeveelheid effectieve afroep/curtailment die uitgevoerd kan worden. Vaak vallen de prognoses echter onder het GTV, en dus zal de uiteindelijke effectieve afroep/curtailment lager uitvallen dan het afroepbaar vermogen."""@nl ;
  dc:source         "B4401" ;
  dct:identifier    "urn:uuid:6b7de77b-cf14-597d-aab2-5de09481f222" ;
  owl:versionInfo   "1" ;
  skos:topConceptOf :Ontology ;
  skos:inScheme     :Ontology .

:8
  a                 skos:Concept ;
  skos:prefLabel    "Effectively Available Capacity"@en, "Effectief beschikbaar vermogen"@nl ;
  skos:definition   "Het deel van de capaciteit dat wel wordt gebruikt door de klant en effectief beschikbaar is om afgeroepen te worden. Dit is het vermogen dat ingeperkt moet worden om het congestieprobleem op te lossen."@nl ;
  dc:source         "B4401" ;
  dct:identifier    "urn:uuid:0cc84423-45f7-51aa-8599-20c19f832702" ;
  owl:versionInfo   "1" ;
  skos:topConceptOf :Ontology ;
  skos:inScheme     :Ontology .

:9
  a                 skos:Concept ;
  skos:prefLabel    "Contracted Transport Capacity"@en, "Gecontracteerd transportvermogen"@nl ;
  skos:altLabel     "GTV" ;
  skos:definition   "het afgesproken transportvermogen van een klant waarvoor de netbeheerder ruimte reserveert op het net (wordt soms ook contractwaarde genoemd)."@nl ;
  skos:altLabel     "GTV" ;
  dc:source         "B4401" ;
  dct:identifier    "urn:uuid:0f9d66a8-e6d3-5541-bd39-e8b9e681137a" ;
  owl:versionInfo   "1" ;
  skos:topConceptOf :Ontology ;
  skos:inScheme     :Ontology .

:10
  a                 skos:Concept ;
  skos:prefLabel    "Regulated grid load"@en, "Geregelde netbelasting"@nl ;
  skos:definition   """the power profile that, after applying congestion management, is expected to actually occur on an asset."""@en,
                    """het vermogensprofiel dat, na toepassing van congestiemanagement, wordt verwacht daadwerkelijk op te treden op een asset."""@nl ;
  dc:source         "B4401" ;
  dct:identifier    "urn:uuid:0610628d-f988-5b54-a030-14d879e58cd1" ;
  owl:versionInfo   "1" ;
  skos:topConceptOf :Ontology ;
  skos:inScheme     :Ontology .

:11
  a                 skos:Concept ;
  skos:prefLabel    "High Power Limit"@en, "Hoge vermogensgrens"@nl ;
  skos:altLabel     "Maximale transportcapaciteit"@nl ;
  skos:definition   "De maximale transportcapaciteit die een klant mag gebruiken op het moment dat er geen beperking is. Buiten de beperkte tijdsvensters om (in geval van CBC-T) en voor alle momenten zonder afroep (in geval van CBC-A) mag de klant dus tot zijn hoge vermogensgrens transport laten plaatsvinden. In de ATO en in dit document wordt dit ook wel GTV genoemd."@nl ;
  dc:source         "B4401" ;
  dct:identifier    "urn:uuid:ba3ee5ba-40b7-5092-808e-0d45f338ac9b" ;
  owl:versionInfo   "1" ;
  skos:topConceptOf :Ontology ;
  skos:inScheme     :Ontology .

:12
  a                 skos:Concept ;
  skos:prefLabel    "Contingency Element"@en, "Knelpuntelement"@nl ;
  skos:definition   "An asset or group of assets that are operationally monitored against overload."@en,
                    "Een asset of groep van assets die operationeel worden bewaakt tegen overbelasting."@nl ;
  dc:source         "B4401" ;
  dct:type          archi:BusinessObject ;
  dct:identifier    "urn:uuid:21843d7f-b928-4c7b-8a46-f4f1a142f2b5" ;
  owl:versionInfo   "1" ;
  skos:topConceptOf :Ontology ;
  skos:inScheme     :Ontology .

:13
  a                 skos:Concept ;
  skos:prefLabel    "Low Power Limit"@en, "lage vermogensgrens"@nl ;
  skos:altLabel     "Minimum transportcapaciteit"@nl ;
  skos:definition   "De minimale transportcapaciteit, een capaciteit die de klant te allen tijde mag gebruiken. Dit vermogen is altijd beschikbaar voor de klant, en de afroeplimiet mag nooit lager zijn dan dit getal."@nl ;
  dc:source         "B4401" ;
  dct:identifier    "urn:uuid:c902bb45-3798-570b-a1f7-b15be5552373" ;
  owl:versionInfo   "1" ;
  skos:topConceptOf :Ontology ;
  skos:inScheme     :Ontology .

:14
  a                 skos:Concept ;
  skos:prefLabel    "Supply by grid operator"@en, "Levering door netbeheerder"@nl ;
  skos:altLabel     "Levering door net"@nl, "LDN" ;
  skos:definition   """A net power flow from the distribution grid to the customer(s)."""@en,
                    "Een netto vermogensstroom van het distributienet naar de klant(en)."@nl ;
  skos:relatedMatch lido37940:152 ;
  dc:source         "B4401" ;
  dct:identifier    "urn:uuid:9cf19402-9443-5a34-863b-ad5bb819b793" ;
  owl:versionInfo   "1" ;
  skos:editorialNote
                    """The use of the LDN term is allowed when there is a transfer point with a customer; in this case, the passive sign convention applies."""@en,
                    """Het gebruik van de LDN term is toegestaan wanneer er sprake is van een overdrachtspunt met een klant; hierbij is de passive sign convention van toepassing."""@nl ;
  rdfs:seeAlso      <https://alliander.atlassian.net/wiki/x/zwGIyQ> ;
  skos:topConceptOf :Ontology ;
  skos:inScheme     :Ontology .

:15
  a                 skos:Concept ;
  skos:prefLabel    "Retrieved by grid operator"@en, "Opname door netbeheerder"@nl ;
  skos:altLabel     "Opname door net"@nl, "ODN" ;
  skos:definition   "Een netto vermogensstroom van de klant(en) naar het distributienet."@nl ;
  skos:relatedMatch lido37940:152 ;
  dc:source         "B4401" ;
  dct:identifier    "urn:uuid:92f080bc-771f-5268-94dc-0779a1075a55" ;
  owl:versionInfo   "1" ;
  skos:editorialNote
                    "Het gebruik van de ODN term is toegestaan wanneer er sprake is van een overdrachtspunt met een klant; hierbij is de passive sign convention van toepassing."@nl ;
  rdfs:seeAlso      <https://alliander.atlassian.net/wiki/x/zwGIyQ> ;
  skos:topConceptOf :Ontology ;
  skos:inScheme     :Ontology .

:16
  a                 skos:Concept ;
  skos:prefLabel    "Affected System Operator"@en, "Betrokken Systeembeheerder"@nl ;
  skos:definition   "means any DSO or TSO significantly affected by congestion or voltage issues on the grid of another systems operator, or whose grid may provide solutions to these issues or that data on the grid or the grid users are necessary to forecast, detect or solve such issues"@en ;
  dc:source         "B4401" ;
  dct:identifier    "urn:uuid:98b1d8a1-3b83-50cc-876f-548d006d46ba" ;
  owl:versionInfo   "1" ;
  skos:topConceptOf :Ontology ;
  skos:inScheme     :Ontology .

:17
  a                 skos:Concept ;
  skos:prefLabel    "Activation"@en, "Activering"@nl ;
  skos:definition   "The requested change of electricity consumption/production by a demand response resource, initiated by a system operator or market signal, requiring the provider to deliver the contracted load modification (increase, decrease, or shift) within the agreed time and magnitude, subject to verification and settlement."@en,
                    "De gevraagde wijziging van elektriciteitsverbruik/-productie door een vraagresponsmiddel, geïnitieerd door een systeembeheerder of marktsignaal, waarbij de aanbieder verplicht is de gecontracteerde lastwijziging (verhoging, verlaging of verschuiving) binnen de afgesproken tijd en omvang te leveren, onder voorbehoud van verificatie en afwikkeling."@nl ;
  dct:identifier    "urn:uuid:65f792b4-57f5-5dba-b6e5-c3eaa93f4f9d" ;
  skos:related      :18, :35 ;
  skos:relatedMatch elit:944-20 ;
  owl:versionInfo   "1" ;
  skos:topConceptOf :Ontology ;
  skos:inScheme     :Ontology .

:18
  a                 skos:Concept ;
  skos:prefLabel    "Activation Interval"@en, "Activeringsinterval"@nl ;
  skos:altLabel     "Activation Window"@en ;
  skos:definition   "An activation interval for operating registered resource refers to the specific period during which this resource is scheduled, commanded, or allowed to be active to provide energy, capacity, or ancillary services to the grid. This interval is typically defined by a start time and an end time, during which this resource must follow operational constraints, such as power output levels, response times, or grid support functions.The activation interval occurs within a availability window. The activation interval in itself is not part of the registered resource, but the properties for activation are."@en,
                    "Een activeringsinterval voor een geregistreerd middel verwijst naar de specifieke periode waarin dit middel is gepland, aangestuurd of toegestaan om actief te zijn om energie, capaciteit of aanvullende diensten aan het net te leveren. Dit interval wordt doorgaans gedefinieerd door een starttijd en een eindtijd, waarin dit middel zich moet houden aan operationele beperkingen, zoals vermogensniveaus, responstijden of netondersteuningsfuncties. Het activeringsinterval vindt plaats binnen een beschikbaarheidsvenster. Het activeringsinterval op zich maakt geen deel uit van het geregistreerde middel, maar de eigenschappen voor activering wel."@nl ; ;
  dct:identifier    "urn:uuid:65f792b4-57f5-5dba-b6e5-c3eaa93f4f9e" ;
  skos:editorialNote
                    "An activation window is a period of time agreed between the Buyer of Flexibility and the Flexibility Service Provider to activate the flexibility service in question. The activation window begins when the Buyer of Flexibility requires the activation and includes the time for ramping up and down, as opposite to a “delivery period” that only includes the period of time where the Resource or Pool of Resources delivers the full effect" ;
  rdfs:seeAlso      <https://mwgstorage1.blob.core.windows.net/public/Ebix/ebIX%20BRS%20for%20Measure%20and%20quantification%20of%20flexibility%20services%20-%20v1r0A%2020231115.pdf> ;
  owl:versionInfo   "1" ;
  skos:topConceptOf :Ontology ;
  skos:inScheme     :Ontology .

:19
  a                 skos:Concept ;
  skos:prefLabel    "Allocation Point"@en, "Allocatiepunt"@nl ;
  skos:definition   """A virtual point at the transfer point of a connection, where the energy exchange between an installation and the grid is administratively assigned to a market party as if the measurement had taken place at the transfer point of the connection;"""@en,
                    """Virtueel punt ter plaatse van het overdrachtspunt van een aansluiting, waar de energie-uitwisseling tussen een installatie en het net administratief aan een marktpartij wordt toegewezen alsof de meting op het overdrachtspunt van de aansluiting heeft plaatsgevonden;"""@nl ;
  skos:narrowMatch  lido37940:130 ;
  skos:exactMatch   maw:MarketEvaluationPoint ;
  skos:narrower     :20, :21 ;
  skos:relatedMatch hemrm:PartyConnectedToTheGrid, hemrm:BalanceResponsibleParty, hemrm:SystemOperator,
                    hemrm:MeteredDataResponsible, hemrm:EnergySupplier ;
  dct:identifier    "urn:uuid:165adbc9-b394-5c53-b414-becae1973fb4" ;
  dct:type          archi:BusinessObject ;
  owl:versionInfo   "1" ;
  rdfs:seeAlso      <https://energiedatawijzer.nl/wp-content/uploads/Documenten/Topics_MFF/TS013-Vertaalslag-van-Meetgegevens-naar-Allocatiepunten-en-of-Overdrachtspunten-1.0.pdf> ;
  skos:topConceptOf :Ontology ;
  skos:inScheme     :Ontology .

:20
  a               skos:Concept ;
  skos:prefLabel  "Primary Allocation Point"@en, "Primair allocatiepunt"@nl ;
  skos:broader    :19 ;
  skos:exactMatch lido37940:130 ;
  dct:type        archi:BusinessObject ;
  owl:versionInfo "1" ;
  dct:identifier  "urn:uuid:e007a242-381d-4b8c-a684-e9e58087354e" ;
#  skos:topConceptOf :Ontology ;
  skos:inScheme   :Ontology .

:21
  a               skos:Concept ;
  skos:prefLabel  "Secondary Allocation Point"@en, "Secundair allocatiepunt"@nl ;
  skos:definition ""@nl ;
  skos:broader    :19 ;
  skos:exactMatch lido37940:161 ;
  dct:type        archi:BusinessObject ;
  owl:versionInfo "1" ;
  dct:identifier  "urn:uuid:349b90e9-c357-444a-9128-f9300f4ee393" ;
#  skos:topConceptOf :Ontology ;
  skos:inScheme   :Ontology .

:22
  a                 skos:Concept ;
  skos:prefLabel    "Common Information Model"@en ;
  skos:definition   """The Common Information Model (CIM) is a standardized, object-oriented conceptual framework developed by the electric utility industry to enable consistent representation, exchange, and integration of power system information across diverse applications and systems. CIM provides a shared vocabulary and schema for electrical network components, their attributes, and relationships, facilitating interoperability and data exchange in electric power operations, planning, and management."""@en ;
  foaf:homepage     <https://www.entsoe.eu/digital/common-information-model/> ;
  owl:versionInfo   "1" ;
  dct:identifier    "urn:uuid:93640816-8d1b-4932-abdd-6a3904cd42d8" ;
  skos:topConceptOf :Ontology ;
  skos:inScheme     :Ontology .

:23
  a                 skos:Concept ;
  skos:prefLabel    "Customer"@en ;
  skos:definition   """A Customer is an individual or organization that is directly connected to the grid and receives services from a distribution or transmission system operator under a contractual agreement."""@en,
                    """Een klant is een persoon of organisatie die rechtstreeks op het net is aangesloten en op basis van een contractuele overeenkomst diensten ontvangt van een distributie- of transmissiesysteembeheerder."""@nl ;
  skos:relatedMatch maw:MarketParticipant ;
  dct:type          archi:BusinessObject ;
  skos:exactMatch   elit:944-1, elit:943-34 ;
  dct:identifier    "urn:uuid:a06856ce-d048-49f5-815a-6d1564157a02" ;
  dct:type          archi:BusinessObject, archi:BusinessRole ;
  skos:topConceptOf :Ontology ;
  skos:inScheme     :Ontology .

:24
  a                 skos:Concept ;
  skos:prefLabel    "Connection Point"@en, "Overdrachtspunt"@nl ;
  skos:altLabel     "Point of connection"@en, "Aansluitpunt"@nl, "OVP", "PoCC", "PCC" ;
  skos:definition   """The point at which a utility's electrical system connects to a customer’s system.
- It's the demarcation point between the DSO and the 'party connected to the grid'.
- It is used in standards such as IEEE 1547, which defines requirements for connecting distributed generation (e.g., solar panels, wind turbines) to the electric grid.
- At the connection, power quality (PQ) measurements are often taken to assess disturbances like voltage sags, harmonics, or flicker.
"""@en, """Een aansluitpunt is de fysieke of logische grens waar een klantinstallatie wordt aangesloten op het distributie- of transmissiesysteem. Het bepaalt de verantwoordelijkheidsgrenzen en wordt gebruikt voor de beoordeling van de stroomkwaliteit, metingen en naleving van de normen voor netaansluiting."""@nl ;
  dc:source         "IEC 61000-4-30" ;
  dct:identifier    "urn:uuid:44c7aa0e-16c3-5442-b3d4-f83396038417" ;
  owl:versionInfo   "1" ;
  skos:example      """If a factory connects to the power grid, the point where the factory’s internal electrical distribution system connects to the grid is the connection point."""@en ;
  skos:exactMatch   elit:631-15, lido37940:126, amw:UsagePoint ;
  skos:relatedMatch hemrm:PartyConnectedToTheGrid ;
  dct:type          archi:BusinessObject ;
  rdfs:seeAlso      <https://www.phasetophase.nl/boek/boek_1_2.html#_2.5> ;
  skos:topConceptOf :Ontology ;
  skos:inScheme     :Ontology .

:25
  a                 skos:Concept ;
  skos:prefLabel    "Business Domain"@en, "Business Domein"@nl ;
  skos:definition   """A business domain is essentially the scope of knowledge, activities, and responsibilities that define a distinct area of an organization’s business. It is often used in strategy, enterprise architecture, and software design to set clear boundaries around what belongs to one area versus another."""@en,
                    """Een business domein is in wezen de reikwijdte van kennis, activiteiten en verantwoordelijkheden die een duidelijk gebied van de bedrijfsvoering van een organisatie definiëren. Het wordt vaak gebruikt in strategie, enterprise architectuur en softwareontwerp om duidelijke grenzen te stellen rond wat tot het ene gebied behoort versus het andere."""@nl ;
  skos:example      "The Billing domain is responsible for generating, validating, and distributing customer invoices. It excludes payment collection, which is handled by the Payments domain."@en ;
  dct:identifier    "urn:uuid:48170043-3c6d-476d-b5d6-452bec944f42" ;
  foaf:homepage     <https://alliander.atlassian.net/wiki/x/IYBK6w> ;
  skos:narrower     :125, :126, :127, :128 ;
  dct:type          archi:BusinessCollaboration ;
  owl:versionInfo   "1" ;
  skos:topConceptOf :Ontology ;
  skos:inScheme     :Ontology .

:26
  a                 skos:Concept ;
  skos:prefLabel    "Connectivity"@en ;
  skos:altLabel     "Network Model"@en ;
  skos:definition   """Connectivity means the whole composition of only functional, non-reducible, electrotechnical components, where these are able to transport or distribute energy and without considering breaker status. It includes the primary function of current- and voltage transformers (auxiliary equipment).i.e. including amongst all switches (load switches, isolators, earthing switches, tapchangers) with their conducting properties in the primary grid.i.e. everything that cannot be related to a (future, current or past) switching action is not connectivity.i.e. from a model perspective the simplest example expressed in IEC CIM would be: Equipment A - Terminal - ConnectivityNode - Terminal - Equipment B.i.e. a substation is then a grouping component."""@en ;
  skos:editorialNote
                    "Network model: A network model represents the electrical system as a graph of connected elements."@en ;
  skos:narrowMatch  :27 ;
  dct:identifier    "urn:uuid:91cf0746-fcde-54e1-a9ac-8e1112cd9c61" ;
  dct:type          archi:BusinessObject ;
  owl:versionInfo   "1" ;
  skos:topConceptOf :Ontology ;
  skos:inScheme     :Ontology .

:27
  a                 skos:Concept ;
  skos:prefLabel    "Topology"@en, "Topologie"@nl ;
  skos:definition   """Topology aims to provide connectivity in a reduced and optimal form for different kinds of studies/downstream processing and provides what's actually connected. The topology is provided in an invariant way, where other variables of the studies do change.means the data concerning the connectivity of the different transmission system or distribution system elements in a substation and includes the electrical configuration and the position of circuit breakers and isolators."""@en,
                    """Topologie heeft als doel om connectiviteit te bieden in een gereduceerde en optimale vorm voor verschillende soorten studies/afgeleide verwerking en biedt wat daadwerkelijk is verbonden. De topologie wordt op een ongewijzigde manier geleverd, waarbij andere variabelen van de studies wel veranderen."""@nl ;
  dct:identifier    "urn:uuid:8cd1aac8-f88d-4011-9d1a-894db825a1b8" ;
  dct:type          archi:BusinessObject ;
  owl:versionInfo   "1" ;
  skos:related      :26 ;
  skos:narrower     :122, :123, :124 ;
  skos:narrowMatch  elit:1485-64 ;
  skos:topConceptOf :Ontology ;
  skos:inScheme     :Ontology .

:28
  a               skos:Concept ;
  skos:prefLabel  "Demand congestion"@en, "Afnamecongestie"@nl ;
  skos:altLabel   "Consumption congestion"@en ;
  skos:definition """This refers to an imbalanced grid situation where the demand for electricity exceeds the available transportation capacity."""@en,
                  """Dit verwijst naar situaties waarin de vraag naar elektriciteit hoger is dan de beschikbare capaciteit om deze te leveren."""@nl ;
  dct:identifier  "urn:uuid:4ee6e311-cdd5-4d9c-b6af-978813cd0e77" ;
  skos:broader    :86 ;
  skos:broadMatch elit:943-4 ;
  skos:related    :29 ;
  owl:versionInfo "1" ;
#  skos:topConceptOf :Ontology ;
  skos:inScheme   :Ontology .

:29
  a                 skos:Concept ;
  skos:prefLabel    "Congestion Service Provider"@en, "Congestie Service Provider"@nl ;
  skos:altLabel     "CSP" ;
  skos:definition   """CSP’s act as intermediaries between large business customers and grid operators, helping prevent congestion on the electricity grid by adjusting clients' electricity production or consumption in response to grid needs, with financial compensation. Only CSPs can submit bids on the open energy market through platforms connected to GOPACS. Businesses can either partner with an existing CSP or become one themselves if they have a contracted capacity of 1,000 kW or more."""@en,
                    """"""@nl ;
  skos:altLabel     "CSP" ;
  skos:broadMatch   hemrm:FlexibilityServiceProvider ;
  skos:exactMatch   lido37940:33 ;
  skos:relatedMatch elit:943-4, maw:MarketRole ;
  dct:identifier    "urn:uuid:85a04e5d-ee34-4243-9b8a-fc91e0eb4931" ;
  dct:type          archi:BusinessRole ;
  owl:versionInfo   "1" ;
  skos:topConceptOf :Ontology ;
  skos:inScheme     :Ontology .

:30
  a                 skos:Concept ;
  skos:prefLabel    "Real Time Markets"@en, "Real-time markten"@nl ;
  skos:altLabel     "RTM" ;
  skos:definition   """Real-time markets are markets where electricity is traded for immediate delivery. These markets allow for rapid adjustments to supply and demand imbalances that may arise due to unexpected changes in generation or consumption. Participants in real-time markets can include generators, consumers, and other market players who can respond quickly to changing conditions."""@en ;
  skos:editorialNote
                    """Though not explicitly defined in one sentence, within the EUR‑Lex MiFID/MiFIR legal framework, a real‑time market refers to a trading venue or platform committed to executing trades and publishing post‑trade data within the regulatory maximum latency (5 minutes) as required to maintain continuous, near-instant transparency to the market."""@en ;
  skos:note         "real time markets which finalize dispatch for system resources"@en ;
  skos:changeNote   "In Review"@en ;
  owl:versionInfo   "1" ;
  dct:identifier    "urn:uuid:c6bca9b8-75bc-4597-8868-a61d4c6932c8" ;
  skos:topConceptOf :Ontology ;
  skos:inScheme     :Ontology .

:31
  a               skos:Concept ;
  skos:prefLabel  "Injection congestion"@en, "Invoedingscongestie"@nl ;
  skos:altLabel   "Generation congestion"@en ;
  skos:definition """This refers to an imbalanced grid situation where the supply of electricity exceeds the available transportation capacity."""@en,
                  """Dit verwijst naar situaties waarin de hoeveelheid opgewekte elektriciteit hoger is dan de capaciteit van het netwerk om deze op te nemen."""@nl ;
  skos:broader    :86 ;
  dct:identifier  "urn:uuid:2db4a30a-995a-51d0-8093-96581d118803" ;
  owl:versionInfo "1" ;
  skos:broadMatch elit:943-4 ;
  skos:related    :29 ;
#  skos:topConceptOf :Ontology ;
  skos:inScheme   :Ontology .

:32
  a                 skos:Concept ;
  skos:prefLabel    "Line"@en, "Verbinding"@nl ;
  skos:definition   """"""@en,
                    """Een kabel, lijn, een samenstel van één of meer serieel met elkaar verbonden kabel- en/of lijndelen met het doel om elektriciteit te transporteren of te distribueren. Een verbinding wordt gemarkeerd door twee knooppunten."""@nl ;
  foaf:homepage     <https://alliander.atlassian.net/wiki/x/woErvQ> ;
  skos:exactMatch   eq:Line ;
  dct:identifier    "urn:uuid:c7b5e972-335f-4acb-bdf1-14e7d1e2c4ab" ;
  dct:type          archi:BusinessObject ;
  owl:versionInfo   "1" ;
  skos:topConceptOf :Ontology ;
  skos:inScheme     :Ontology .

:33
  a                 skos:Concept ;
  skos:prefLabel    "Connection Agreement"@en, "Aansluitovereenkomst"@nl ;
  skos:definition   """Agreement between a connected party and a grid operator regarding the connection to a grid and the transportation of electricity over that grid;"""@en,
                    """Overeenkomst tussen een aangeslotene en een netbeheerder betreffende de aansluiting op een net en het transport van elektriciteit over dat net;"""@nl ;
  dct:identifier    "urn:uuid:1b315825-b80c-46ad-82de-17f095893cb0" ;
  dct:type          archi:BusinessObject ;
  owl:versionInfo   "1" ;
  skos:exactMatch   lido37940:3, elit:631-14 ;
  skos:related      :55 ;
  skos:narrowMatch  amw:CustomerAgreement ;
  skos:topConceptOf :Ontology ;
  skos:inScheme     :Ontology .

:34
  a                 skos:Concept ;
  skos:prefLabel    "D"@en, "D"@nl ;
  skos:definition   "The abbreviation D is used to indicate which day congestion falls on. Thus, D-1 means the day before the congestion."@en,
                    "De afkorting D wordt gebruikt om aan te geven op welke dag de congestie valt. Dus D-1 betekent de dag voor de congestie."@nl ;
  dct:identifier    "urn:uuid:2e5ca0cf-7837-4691-95f7-cd7765c1f5f8" ;
  owl:versionInfo   "1" ;
  skos:topConceptOf :Ontology ;
  skos:inScheme     :Ontology .

:35
  a                 skos:Concept ;
  skos:prefLabel    "Demand Response"@en, "Vraagrespons"@nl ;
  skos:altLabel     "Demand-side flexibility"@en ;
  skos:definition   "Changes in electric usage by demand-side resources from their normal consumption patterns in response to changes in the price of electricity over time, or to incentive payments designed to induce lower electricity use at times of high wholesale market prices or when system reliability is jeopardized.”"@en,
                    "Wijzigingen in het elektriciteitsverbruik door vraagzijde bronnen ten opzichte van hun normale verbruikspatronen als reactie op veranderingen in de prijs van elektriciteit in de tijd, of op prikkels die zijn ontworpen om een lager elektriciteitsverbruik te stimuleren op momenten van hoge groothandelsmarktprijzen of wanneer de systeembetrouwbaarheid in gevaar is.”"@nl ;
  dct:identifier    "urn:uuid:8052865c-f3ce-49c5-a304-ccd46ce279ec" ;
  owl:versionInfo   "1" ;
  rdfs:seeAlso      <https://sympower.net/articles/what-is-demand-response> ;
  skos:exactMatch   dsm:DemandResponse ;
  skos:exactMatch   elit:944-20 ;
  skos:topConceptOf :Ontology ;
  skos:inScheme     :Ontology .

:36
  a                 skos:Concept ;
  skos:prefLabel    "Demand Response Product "@en, "Vraagresponse product"@nl ;
  skos:definition   "means products offered by DSOs for shifting (in time) and/or modulating (increase or decrease) electricity consumption and/or production through controlled operation by executing remedial actions.The shifting a shift in time can be stationary in nature or on individual call.Example: The curtailment product CBC-T has a stationary shift in time.refer to technologies and systems used to manage and adjust consumers' electricity demand in response to supply conditions. These products are critical in balancing the grid, enhancing reliability, and integrating renewable energy sources. The kind of remedial actions are derived from the D/R product properties."@en ;
  skos:related      :35 ;
  skos:relatedMatch dsm:DemandResponse ;
  dct:identifier    "urn:uuid:79d1b045-1594-4a69-b5df-25c5bb6df09b" ;
  dct:type          archi:BusinessObject ;
  owl:versionInfo   "1" ;
  skos:topConceptOf :Ontology ;
  skos:inScheme     :Ontology .

:37
  a                 skos:Concept ;
  skos:prefLabel    "Demand Side Response"@en ;
  skos:definition   "means D/R products operated in line with operating constraints and consumer preferences, in response to signals from, and acting in agreement with, regulated electricity market participants"@en ;
  skos:relatedMatch elit:944-25 ;
  skos:relatedMatch dsm:DemandResponse ;
  dct:identifier    "urn:uuid:44a346c9-379f-440e-a34b-c3e6a74ac9e3" ;
  owl:versionInfo   "1" ;
  skos:topConceptOf :Ontology ;
  skos:inScheme     :Ontology .

:38
  a                 skos:Concept ;
  skos:prefLabel    "Demand Side Response Service System"@en ;
  skos:definition   "represents an IT-system encapsulation of business functionality to support the services of the D/R products."@en ;
  dct:identifier    "urn:uuid:70619e3d-a066-4b3f-b75e-0418586e3631" ;
  owl:versionInfo   "1" ;
  skos:topConceptOf :Ontology ;
  skos:inScheme     :Ontology .

:39
  a                 skos:Concept ;
  skos:prefLabel    "Demand Side Response Service Provider"@en ;
  skos:definition   "means an organization using ESAs to provide demand-side-related energy management services to regulated electricity market participants"@en ;
  dct:identifier    "urn:uuid:1674c8c7-8acd-4c79-bac5-729b8e090ba6" ;
  owl:versionInfo   "1" ;
  skos:topConceptOf :Ontology ;
  skos:inScheme     :Ontology .

:40
  a                 skos:Concept ;
  skos:prefLabel    "Sign Convention"@en, "Stroomrichting Conventie"@nl ;
  skos:definition   """A sign convention is a choice of the physical significance of signs (plus or minus) for a set of quantities, in a case where the choice of sign is arbitrary. "Arbitrary" here means that the same physical system can be correctly described using different choices for the signs, as long as one set of definitions is used consistently. Disagreement about sign conventions is a frequent source of confusion, frustration, misunderstandings, and even outright errors."""@en ;
  skos:altLabel     "SC" ;
  foaf:homepage     <https://alliander.atlassian.net/wiki/x/AQBwyg> ;
  owl:versionInfo   "1" ;
  skos:narrower     :41 ;
  dct:identifier    "urn:uuid:e25aa2e9-ca8f-4fcd-adc3-163e134275e8" ;
  skos:topConceptOf :Ontology ;
  skos:inScheme     :Ontology .

:41
  a               skos:Concept ;
  skos:prefLabel  "Passive Sign Convention"@en ;
  skos:definition """the reference direction of the current variable (the arrow representing the direction of positive current) points into the positive reference terminal of the voltage variable. This means that if the voltage and current variables have positive values, current flows through the device from the positive to the negative terminal, doing work on the component, as occurs in a passive component. So power flowing into the component from the line is defined as positive; the power variable represents power dissipation in the component. Therefore:
    - Active components (power sources) will have negative resistance and negative power flow
    - Passive components (loads) will have positive resistance and positive power flow"""@en ;
  skos:altLabel   "PSC" ;
  skos:broader    :40 ;
  foaf:homepage   <https://alliander.atlassian.net/wiki/x/AQBwyg> ;
  rdfs:seeAlso    <https://en.wikipedia.org/wiki/Passive_sign_convention> ;
  owl:versionInfo "1" ;
  dct:identifier  "urn:uuid:e28b3533-a11c-4357-9a05-e850c39aabf5" ;
#  skos:topConceptOf :Ontology ;
  skos:inScheme   :Ontology .

:42
  a                 skos:Concept ;
  skos:prefLabel    "Energy Smart Appliance (ESA)"@en ;
  skos:definition   "means an appliance that can operate D/R products; it is communications-enabled and can respond \"automatically\" to operating constraints by shifting or modulating its electricity consumption and/ or production."@en ;
  dct:identifier    "urn:uuid:71b2f9d5-d01d-4af9-b8d5-e104b3e9cf78" ;
  owl:versionInfo   "1" ;
  skos:topConceptOf :Ontology ;
  skos:inScheme     :Ontology .

:43
  a                 skos:Concept ;
  skos:prefLabel    "Energy Consumer"@en, "Energie Afnemer"@nl ;
  skos:definition   """An Energy Consumer is an entity (individual or organization), or system that consumes/produces electrical energy, and is used in grid calculations to assign load or generation profiles and support operational control actions. This encompasses a wide range of users, from household appliances and industrial machinery to entire facilities and infrastructures."""@en,
                    """Een energieverbruiker is een entiteit (persoon of organisatie) of systeem dat elektrische energie verbruikt/produceert en wordt gebruikt in netberekeningen om belastings- of opwekkingsprofielen toe te wijzen en operationele controlemaatregelen te ondersteunen. Dit omvat een breed scala aan gebruikers, van huishoudelijke apparaten en industriële machines tot complete faciliteiten en infrastructuren."""@nl ;
  skos:editorialNote
                    """The EnergyConsumer can optionally be associated with a meter through the usage point and market evaluation point."""@en ;
  skos:editorialNote
                    """It has a reference to locate the point of control for executing a remedial action when operating a D/R product."""@en,
                    """Het heeft een referentie om het controlepunt te lokaliseren voor het uitvoeren van een herstelactie bij het gebruik van een D/R-product."""@nl ;
  skos:broader      :105 ;
  skos:related      :75 ;
  skos:broadMatch   eq:EnergyConsumer ;
  skos:relatedMatch hemrm:Consumer, hemrm:Producer, amw:UsagePoint ;
  dct:identifier    "urn:uuid:558309d3-42a0-55d7-a8b8-854fe1502586" ;
  dct:type          archi:BusinessObject, archi:BusinessRole ;
  owl:versionInfo   "1" ;
  skos:topConceptOf :Ontology ;
  skos:inScheme     :Ontology .

:44
  a                 skos:Concept ;
  skos:prefLabel    "Asset Functional Characteristics"@en ;
  skos:definition   """The Asset Functional Characteristics business object describes the combination and interdependencies of asset data (technical information), engineering data, design parameters, environment conditions (both static and dynamic), asset condition data and asset maintenance strategy to form the safe operational space and operational constraints. For example, inherent/permanent thermal rating of assets deployed in the network including changes in electrical asset performance limits based on temperature, wind speed and solar radiation, which set the frame for a variety of actual operational limits on network elements"""@en,
                    """De ‘Functionele kenmerken van activa’ beschrijft de combinatie en onderlinge afhankelijkheden van activagegevens (technische informatie), engineeringgegevens, ontwerpparameters, omgevingsomstandigheden (zowel statisch als dynamisch), gegevens over de toestand van activa en de onderhoudsstrategie voor activa om de veilige operationele ruimte en operationele beperkingen te vormen. Bijvoorbeeld de inherente/permanente thermische classificatie van activa die in het netwerk worden ingezet, inclusief veranderingen in de prestatielimieten van elektrische activa op basis van temperatuur, windsnelheid en zonnestraling, die het kader vormen voor een verscheidenheid aan feitelijke operationele limieten voor netwerkelementen."""@nl ;
  skos:narrowMatch  amw:AssetInfo ;
  skos:relatedMatch eq:ConductingEquipment ;
  dct:identifier    "urn:uuid:91df4007-635e-4c49-a82d-15e8e881686d" ;
  dct:type          archi:BusinessObject ;
  foaf:homepage     <https://alliander.atlassian.net/l/cp/Rm90h0nK> ;
  owl:versionInfo   "1" ;
  skos:topConceptOf :Ontology ;
  skos:inScheme     :Ontology .

:45
  a                 skos:Concept ;
  skos:prefLabel    "Estimation"@en ;
  skos:definition   "An estimation (model, intuition) means an approximate calculation when the exact data is unavailable (assumptions)."@en ;
  dc:source         "Data Science" ;
  dct:identifier    "urn:uuid:11889854-aa72-4a76-b042-10631fabe202" ;
  owl:versionInfo   "1" ;
  skos:topConceptOf :Ontology ;
  skos:inScheme     :Ontology .

:46
  a                 skos:Concept ;
  skos:prefLabel    "Energy Carrier"@en, "Energiedrager"@nl ;
  skos:definition   "A medium that contains usable energy"@en, "Een medium dat bruikbare energie bevat"@nl ;
  foaf:homepage     "https://www.cbs.nl/nl-nl/onze-diensten/methoden/begrippen/energiedrager" ;
  skos:exactMatch   <https://vocabs.cbs.nl/def/begrippen/830> ;
  dct:identifier    "urn:uuid:fb80d523-a716-4be9-ba32-c47024d58f04" ;
  skos:topConceptOf :Ontology ;
  skos:inScheme     :Ontology .

:47
  a                 skos:Concept ;
  skos:prefLabel    "Flexible Customer"@en ;
  skos:definition   "Role: means a customer that contributes to or intends to contribute to the provision of services for systems operators or the provision of wholesale market products via a service provider using CUs under his control"@en ;
  skos:broadMatch   elit:944-1 ;
  skos:relatedMatch maw:MarketRole, elit:944-24c, elit:944-8 ;
  dct:identifier    "urn:uuid:50699874-ec5d-4565-bccc-7cf76bd56a6b" ;
  dct:type          archi:BusinessRole ;
  owl:versionInfo   "1" ;
  skos:topConceptOf :Ontology ;
  skos:inScheme     :Ontology .

:48
  a                 skos:Concept ;
  skos:prefLabel    "Energy Forecast"@en ;
  skos:altLabel     "Forecast"@en ;
  skos:definition   "An Energy Forecast represents expected future energy values for consumption, production, or exchange over defined time intervals. It is derived from forecasting models using measurements and external inputs and supports operational planning, congestion management, and market processes."@en,
                    "Een energieprognose geeft de verwachte toekomstige energiewaarden weer voor verbruik, productie of uitwisseling over bepaalde tijdsintervallen. Deze prognose is afgeleid van voorspellingsmodellen op basis van metingen en externe input en ondersteunt de operationele planning, congestiebeheer en marktprocessen."@nl ;
  skos:example      "As an example, the expected (future) values for measurements on terminals (points on the grid) are based on a machine learning model and available meter readings."@en ;
  skos:relatedMatch eq:EnergyArea, elit:1222-4 ;
  dc:source         "Data Science" ;
  dct:identifier    "urn:uuid:b9a80f80-7e6c-444c-b398-23bf2c915cd9" ;
  dct:type          archi:BusinessObject ;
  owl:versionInfo   "1" ;
  skos:topConceptOf :Ontology ;
  skos:inScheme     :Ontology .

:49
  a                      skos:Concept ;
  skos:prefLabel         "PowerTransformer"@en, "Vermogenstransformator"@nl ;
  skos:altLabel          "Transformer"@en, "Transformator"@nl ;
  skos:definition        """A static device with two or more windings which, by electromagnetic induction, converts a system of alternating voltage and current into another system of different voltage and current, usually of the same frequency."""@en,
                         """Een statisch apparaat met twee of meer wikkelingen die door elektromagnetische inductie een systeem van wisselspanning en -stroom omzet in een ander systeem met een andere spanning en stroom, meestal van dezelfde frequentie."""@nl ;
  skos:exactMatch        eq:PowerTransformer, eq:PowerTransformerEnd ;
  skos:broaderTransitive eq:TransformerEnd ;
  dc:source              "IEC 60050" ;
  dct:identifier         "urn:uuid:cafdec10-7e95-46e1-b993-1babe8970c44" ;
  dct:type               archi:BusinessObject ;
  foaf:homepage          <https://alliander.atlassian.net/l/cp/DysrmvsV> ;
  owl:versionInfo        "1" ;
  skos:topConceptOf      :Ontology ;
  skos:inScheme          :Ontology .

:50
  a                 skos:Concept ;
  skos:prefLabel    "Intermediate System Operator"@en ;
  skos:definition   "means any DSO or TSO significantly affected by balancing and local services bids from SPU or SPG connected to another system."@en ;
  dct:identifier    "urn:uuid:ffba03d4-117d-5066-ac4a-709dfe1227b8" ;
  dct:type          archi:BusinessActor ;
  owl:versionInfo   "1" ;
  skos:topConceptOf :Ontology ;
  skos:inScheme     :Ontology .

:51
  a                 skos:Concept ;
  skos:prefLabel    "Scenario"@en ;
  skos:definition   """A scenario defines the operating parameters, when executing a study on a contingency. These operating parameters are:
- the topological island (result of topology processing) of the power system on a given time (of time-frame).
- the forecasted state of the power system on a given time-frame"""@en ;
  skos:relatedMatch elit:1222-4 ;
  dct:identifier    "urn:uuid:aadaafa2-967f-50dc-b2a4-ee76e794322f" ;
  dct:type          archi:BusinessObject ;
  owl:versionInfo   "1" ;
  skos:topConceptOf :Ontology ;
  skos:inScheme     :Ontology .

:52
  a                 skos:Concept ;
  skos:prefLabel    "Trace"@en, "Traject"@nl ;
  skos:definition   """means an ordered sequence of connectivity nodes and conducting equipment in an electrical network graph. This sequence starts and ends at a connectivity node and alternates between:
- Connectivity nodes, which represent points of electrical connection.
- Conducting equipment, which connect two adjacent connectivity nodes and convey power or signals.
"""@en, """Een geordende reeks van connectiviteitsknooppunten en geleidend materieel in een elektrisch netwerkdiagram. Deze reeks begint en eindigt bij een connectiviteitsknooppunt"""@nl ;
  dct:identifier    "urn:uuid:42234cf6-99c1-50b2-8bfa-a9ebd113a9f3" ;
  dct:type          archi:BusinessObject ;
  owl:versionInfo   "1" ;
  skos:topConceptOf :Ontology ;
  skos:inScheme     :Ontology .

:53
  a                 skos:Concept ;
  skos:prefLabel    "Maintenance"@en, "Onderhoud"@nl ;
  skos:definition   "The combination of all technical and management actions intended to retain an item in, or restore it to, a state in which it can perform as required"@en,
                    "De combinatie van alle technische en beheersmaatregelen die bedoeld zijn om een object in een staat te behouden waarin het kan functioneren zoals vereist, of om het in die staat te herstellen."@nl ;
  dct:identifier    "urn:uuid:927d4d77-9355-5892-a6ab-916c0b818ffb" ;
  owl:versionInfo   "1" ;
  skos:topConceptOf :Ontology ;
  skos:inScheme     :Ontology .

:54
  a                 skos:Concept ;
  skos:prefLabel    "Contingency"@en, "Onvoorziene omstandigheden"@nl ;
  skos:definition   "A modeled capacity scenario used by distributed system operators to analyse operational security, grid constraints, and remedial actions during day-ahead, intra-day, or near-real-time operation."@en ;
  skos:scopeNote    "Used in flexibility frameworks where contingencies act as activation conditions for demand response, redispatch, or congestion management products."@en ;
  skos:exactMatch   elit:1222-10 ;
  skos:exactMatch   cim:Contingency ;
  foaf:homepage     <https://alliander.atlassian.net/l/cp/GDQyJ2PF> ;
  rdfs:seeAlso      <https://alliander.atlassian.net/l/cp/E4u2ycRZ> ;
  dct:identifier    "urn:uuid:16b97568-f784-57e7-898d-0d03a6b8e7be" ;
  dct:type          archi:BusinessObject ;
  owl:versionInfo   "1" ;
  skos:topConceptOf :Ontology ;
  skos:inScheme     :Ontology .

:55
  a                 skos:Concept ;
  skos:prefLabel    "Connection"@en, "Aansluiting"@nl ;
  skos:altLabel     "Network Connection"@en ;
  skos:definition   "One or more connections between a grid and an immovable property as referred to in Article 16 in the Grid Code, parts a through d, of the Property Valuation Act, or between a grid and another grid at a different voltage level (border supply)."@en,
                    """Eén of meer verbindingen tussen een net en een onroerende zaak als bedoeld in artikel 16 in de netcode, onderdelen a tot en met d, van de Wet waardering onroerende zaken, dan wel tussen een net en een ander net op een ander spanningsniveau (grenslevering)."""@nl ;
  owl:versionInfo   "1" ;
  skos:relatedMatch elit:631-15, lido37940:126 ;
  dct:identifier    "urn:uuid:4ddf9840-2c67-45ac-a10e-4e18a77dd692" ;
  dct:type          archi:BusinessObject ;
  skos:topConceptOf :Ontology ;
  skos:inScheme     :Ontology .

:56
  a               skos:Concept ;
  skos:prefLabel  "Normal State"@en, "Normale toestand"@nl ;
  skos:definition """A situation in which the system is within operational security limits in the N-situation and after the occurrence of any contingency from the contingency list, taking into account the effect of the available remedial actions"""@en,
                  """Situatie waarin het systeem binnen de operationeleveiligheidsgrenzen in de N-situatie functioneert en nadat zich een uitvalsituatie uit de lijst van uitvalsituaties heeft voorgedaan, met inachtneming van het effect van de beschikbare remediërende maatregelen."""@nl ;
  skos:broader    :59 ;
  skos:broadMatch elit:1485-5 ;
  skos:related    elit:1222-7 ;
  owl:versionInfo "1" ;
  dct:identifier  "urn:uuid:02a28b4c-a8f3-4aa8-8c7b-77d96cacc804" ;
#  skos:topConceptOf :Ontology .
  skos:inScheme   :Ontology .

:57
  a               skos:Concept ;
  skos:prefLabel  "Alert state"@en, "Alarmtoestand"@nl ;
  skos:definition """The system state in which the system is within operational security limits, but a contingency from the contingency list has been detected and in case of its occurrence the available remedial actions are not sufficient to keep the normal state"""@en,
                  """Toestand van het systeem wanneer het zich binnen de operationeleveiligheidsgrenzen bevindt, maar een uitvalsituatie uit de lijst van uitvalsituaties is waargenomen waarbij, mocht die zich daadwerkelijk voordoen, de beschikbare remediërende maatregelen niet toereikend zijn om de normale toestand te handhaven;"""@nl ;
  skos:broader    :59 ;
  skos:broadMatch elit:1485-17 ;
  skos:related    elit:1222-7 ;
  owl:versionInfo "1" ;
  dct:identifier  "urn:uuid:a4a6c3c9-ab1e-4727-b692-db2ec750117f" ;
#  skos:topConceptOf :Ontology ;
  skos:inScheme   :Ontology .

:58
  a               skos:Concept ;
  skos:prefLabel  "Emergency state"@en, "Noodtoestand"@nl ;
  skos:definition """The system state in which one or more operational security limits are violated."""@en,
                  """Systeemtoestand waarin één of meer operationeleveiligheidsgrenzen worden geschonden."""@nl ;
  skos:broader    :59 ;
  skos:broadMatch elit:1485-37 ;
  skos:related    elit:1222-7 ;
  owl:versionInfo "1" ;
  dct:identifier  "urn:uuid:713e48c0-2799-42af-9a72-7a35297ea477" ;
#  skos:topConceptOf :Ontology ;
  skos:inScheme   :Ontology .

:59
  a                 skos:Concept ;
  skos:prefLabel    "System State"@en, "Systeemtoestand"@nl ;
  skos:definition   """The operational state of the distribution system in relation to the operational security limits which can be normal state, alert state, emergency state, blackout state and restoration state;"""@en,
                    """Operationele toestand van het distributiesysteem ten aanzien van de operationeleveiligheidsgrenzen. Een distributiesysteem kan zich bevinden in de normale toestand, de alarmtoestand, de noodtoestand, de black-outtoestand en de hersteltoestand."""@nl ;
  skos:narrower     :56, :57, :58 ;
  skos:relatedMatch elit:1485-36 ;
  owl:versionInfo   "1" ;
  dct:identifier    "urn:uuid:ee63c58c-c445-4d19-a09b-5ba5a01bc9ce" ;
  dct:type          archi:BusinessObject ;
  skos:topConceptOf :Ontology ;
  skos:inScheme     :Ontology .

:60
  a                 skos:Concept ;
  skos:prefLabel    "Operational security limits"@en ;
  skos:definition   "The acceptable operating boundaries for secure grid operation such as thermal limits, voltage limits, short-circuit current limits, frequency and dynamic stability limits."@en ;
  skos:exactMatch   elit:1222-7 ;
  skos:related      :59 ;
  skos:narrower     :71, :115 ;
  owl:versionInfo   "1" ;
  dct:identifier    "urn:uuid:a50905a9-d292-4ab0-bb48-db9b7d11fe3a" ;
  dct:type          archi:BusinessObject ;
  skos:topConceptOf :Ontology ;
  skos:inScheme     :Ontology .

:61
  a                 skos:Concept ;
  skos:prefLabel    "Prediction"@en ;
  skos:definition   "A prediction is a statement about a specific future event. Forecasting and estimating are sub-disciplines of prediction"@en ;
  dc:source         "Data Science" ;
  dct:identifier    "urn:uuid:bb133e6c-4565-51cb-a31f-26e5ab3d4d11" ;
  owl:versionInfo   "1" ;
  skos:topConceptOf :Ontology ;
  skos:inScheme     :Ontology .

:62
  a                  skos:Concept ;
  skos:prefLabel     "Component"@en, "Component"@nl ;
  skos:definition    """Constituent part of a device which cannot be physically divided into smaller parts without losing its particular function."""@en,
                     """Een onverdeelbaar onderdeel van een apparaat dat zijn functie verliest als het in kleinere delen wordt gesplitst."""@nl ; ;
  skos:editorialNote """It is an essential part that cannot be further divided without losing its purpose."""@en,
                     """Het is een essentieel onderdeel dat niet verder kan worden opgedeeld zonder zijn doel te verliezen."""@nl ;
  dc:source          "IEC 60050 (IEV 151-11-21)" ;
  owl:versionInfo    "1" ;
  dct:identifier     "urn:uuid:7e4fb8b5-5673-4fba-abea-485648599592" ;
  skos:topConceptOf  :Ontology ;
  skos:inScheme      :Ontology .

:63
  a                 skos:Concept ;
  skos:prefLabel    "Energy System"@en, "Energie Systeem"@nl ;
  skos:definition   """A system that includes all components and processes involved in the production, distribution, and consumption of energy, including generation sources, transmission networks, distribution systems, and end-use applications. It encompasses the entire energy value chain, from primary energy sources to final energy services, and includes both physical infrastructure and operational practices."""@en,
                    """Een systeem dat alle componenten en processen omvat die betrokken zijn bij de productie, distributie en consumptie van energie, inclusief energiebronnen, transmissienetwerken, distributiesystemen en eindgebruikstoepassingen. Het omvat de gehele energiewaardeketen, van primaire energiebronnen tot eindenergievoorzieningen, en omvat zowel fysieke infrastructuur als operationele praktijken."""@nl ;
  skos:editorialNote
                    """The IPCC (Intergovernmental Panel on Climate Change) defines an energy system as: 'all components related to the production, conversion, delivery, and use of energy.' This encompasses generation, transport, storage, distribution, and consumption across sectors"""@en ;
  skos:related      :81 ;
  skos:changeNote   "In Review"@en ;
  rdfs:seeAlso      <https://en.wikipedia.org/wiki/Energy_system> ;
  owl:versionInfo   "1" ;
  dct:identifier    "urn:uuid:122b078c-5196-40b0-96ac-4c3767cf5e94" ;
  skos:topConceptOf :Ontology ;
  skos:inScheme     :Ontology .

:64
  a                 skos:Concept ;
  skos:prefLabel    "Primary Substation"@en ;
  skos:definition   """Three variants are defined, which could be derivable from the collection of equipment. The type and variant can be combined to indicate the concrete implementation of the substation."""@en,
                    """Drie varianten zijn gedefinieerd, die afgeleid kunnen worden van de verzameling van apparatuur. Het type en de variant kunnen worden gecombineerd om de concrete implementatie van het station aan te geven."""@nl ;
  skos:narrower     :65, :66, :67 ;
  skos:relatedMatch eq:Substation, eq:VoltageLevel ;
  foaf:homepage     <https://alliander.atlassian.net/wiki/x/R4YovQ> ;
  rdfs:seeAlso      <https://www.phasetophase.nl/boek/boek_1_2.html#_2.4.6> ;
  dct:identifier    "urn:uuid:59a52f76-8ac7-4ad6-9b91-bb272b561b4a" ;
  dct:type          archi:BusinessObject ;
  skos:topConceptOf :Ontology ;
  skos:inScheme     :Ontology .

:65
  a              skos:Concept ;
  skos:prefLabel "Primary Transforming Substation"@en, "Onderstation"@nl ;
  skos:altLabel  "OS"@nl ;
  skos:definition
                 """Transforming - includes power transformer interconnecting two or more networks of different voltages levels"""@en,
                 """Transformeren - omvat een krachtstroomtransformator die twee of meer netwerken van verschillende spanningsniveaus met elkaar verbindt."""@nl ;
  skos:broader   :64 ;
  dct:identifier "urn:uuid:fd0e7359-e5c5-4861-bd86-b0692093a46d" ;
#  skos:topConceptOf :Ontology ;
  skos:inScheme  :Ontology .

:66
  a              skos:Concept ;
  skos:prefLabel "Primary Regulating SubStation"@en, "RegelStation"@nl ;
  skos:altLabel  "RS" ;
  skos:definition
                 """Regulating - includes power transformer with special winding divided into several sections enabling the voltage to be varied at will."""@en,
                 """Regulerend - omvat een transformator met speciale winding verdeeld in verschillende secties waardoor de spanning naar wens kan worden gevarieerd."""@nl ;
  skos:broader   :64 ;
  dct:identifier "urn:uuid:9915b9f8-ccf9-45fe-a5ff-24affd2296f9" ;
#  skos:topConceptOf :Ontology ;
  skos:inScheme  :Ontology .

:67
  a               skos:Concept ;
  skos:prefLabel  "Primary Switching SubStation"@en, "SchakelStation"@nl ;
  skos:altLabel   "SS"@nl ;
  skos:definition """Switching - includes switchgear and usually busbars (Schakel)."""@en,
                  """Schakelend - omvat schakelinstallaties en meestal rails."""@nl ;
  skos:broader    :64 ;
  dct:identifier  "urn:uuid:488b9eb0-ebee-4f0c-937f-cda12aaa5d28" ;
#  skos:topConceptOf :Ontology ;
  skos:inScheme   :Ontology .

:68
  a                 skos:Concept ;
  skos:prefLabel    "Asset Policy Limit"@en, "Beleid Fysieke Component Limiet"@nl ;
  skos:definition   """It means is the maximum capacity, rating, or performance value—such as current, power, or load—that an asset can safely handle under specified operating and environmental conditions, as defined by standards or supplier specifications.
  Rules or guidelines that specify what is permitted or restricted for an Asset or Asset Type. Each policy covers a specific operational aspect and is applied together with the values relevant for enforcing that rule.
- Scope: Defines where and to whom the policy applies, including conditions such as soil type, temperature, or other environmental factors.
- Value: A numerical parameter, either assigned or computed, that quantifies the policy’s limit or requirement."""@en,
                    """Is de maximale capaciteit, beoordeling of prestatiewaarde, zoals stroom, vermogen of belasting, die een actief veilig kan verwerken onder gespecificeerde bedrijfs- en omgevingsomstandigheden, zoals gedefinieerd door normen of leveranciersspecificaties."""@nl ;
  skos:changeNote   "In Review"@en ;
  dct:type          archi:BusinessObject ;
  owl:versionInfo   "1" ;
  dct:identifier    "urn:uuid:d7fe56cf-262b-4515-a9c0-2d71f1f125f1" ;
  skos:topConceptOf :Ontology ;
  skos:inScheme     :Ontology .

:69
  a               skos:Concept ;
  skos:prefLabel  "Feeder"@en, "Route"@nl ;
  skos:altLabel   "MV-route"@nl, "MS-route"@nl ;
  skos:definition """An electric line originating at a main substation and supplying one or more secondary substations"""@en,
                  """Representatie van een (of meerdere) afgaande veld op een station. De route groepering bevat dan alle onderliggende netcomponenten die gevoed worden vanuit dit veld."""@nl ;
  skos:editorialNote
                  """the concept of a feeder is not always a direct class but is often modeled as a set of interconnected Equipment objects within a TopologicalIsland or ConnectivityNode. Sometimes, utilities create a specific class or use a Terminal or ConnectivityNode group to represent a feeder for operational or reporting purposes."""@en ;
  skos:broader    :107 ;
  skos:broadMatch eq:EquipmentContainer, tp:ConnectivityNodeContainer ;
  dct:identifier  "urn:uuid:02e7ef9c-3b86-503e-8b1b-b6b1bdd8e8fe" ;
  dct:type        archi:BusinessObject ;
  owl:versionInfo "1" ;
  foaf:homepage   <https://alliander.atlassian.net/wiki/x/c4SGvQ> ;
#  skos:topConceptOf :Ontology ;
  skos:inScheme   :Ontology .

:70
  a               skos:Concept ;
  skos:prefLabel  "BusbarSection"@en, "Rail"@nl ;
  skos:definition """A busbar section is a part of a busbar system that can be isolated from the rest of the busbar system for maintenance or operational purposes. It is typically used in substations and switchyards to connect multiple circuits or equipment, allowing for flexibility in operation and maintenance."""@en,
                  """Een railssectie is een deel van een railsysteem dat kan worden geïsoleerd van de rest van het railsysteem voor onderhouds- of operationele doeleinden. Het wordt meestal gebruikt in onderstations en schakelparken om meerdere circuits of apparatuur te verbinden, waardoor flexibiliteit in werking en onderhoud mogelijk is."""@nl ; ;
  skos:exactMatch eq:BusbarSection ;
  dct:identifier  "urn:uuid:d6012e43-5e6d-57ad-b7dc-9302e69f8cb5" ;
  dct:type        archi:BusinessObject ;
  owl:versionInfo "1" ;
  skos:broader    :105 ;
  foaf:homepage   <https://alliander.atlassian.net/wiki/x/vwB4vg> ;
#  skos:topConceptOf :Ontology ;
  skos:inScheme   :Ontology .

:71
  a               skos:Concept ;
  skos:prefLabel  "Equipment Operating Limit"@en, "Functionele Component Limiet"@nl ;
  skos:definition """A generic limit that applies to a equipment item (e.g., line, breaker, transformer), representing its physical or operational capability such as current rating, voltage withstand, or thermal capacity."""@en,
                  """Een generieke limiet die van toepassing is op materieel (bijv. lijn, schakelaar, transformator) en die de fysieke of operationele capaciteit ervan vertegenwoordigt, zoals stroomsterkte, spanningsweerstand of thermische capaciteit."""@nl ;
  skos:broader    :133, :134 ;
  skos:changeNote "In Review"@en ;
  owl:versionInfo "1" ;
  dct:identifier  "urn:uuid:724c8d13-413d-4fb4-b6e5-ff14eae9190f" ;
#  skos:topConceptOf :Ontology ;
  skos:inScheme   :Ontology .


:72
  a                 skos:Concept ;
  skos:prefLabel    "Settlement Condition"@en, "afwikkelingsvoorwaarden"@nl ;
  skos:definition   """Settlement Conditions define the rules and criteria for evaluating performance and calculating payments or penalties for flexibility and demand‑response products, including the required capacity or energy deviation."""@en,
                    """De afwikkelingsvoorwaarden definiëren de regels en criteria voor het evalueren van prestaties en het berekenen van betalingen of boetes voor flexibiliteits- en vraagresponsproducten, met inbegrip van de vereiste capaciteit of energieafwijking."""@nl ;
  skos:editorialNote
                    """The settlement conditions describe the amount of capacity that needs to be managed (mitigate, curtailled, etc) these conditions are communicated to agents (IT-components), to search for a possible solution based on a particular D/R product."""@en ;
  dct:identifier    "urn:uuid:1acdd42f-10c7-5a1f-a0c4-49f6541e8999" ;
  dct:type          archi:BusinessObject ;
  skos:relatedMatch elit:1485-93, elit:944-20 ;
  skos:broadMatch   elit:2195-29 ;
  skos:topConceptOf :Ontology ;
  owl:versionInfo   "1" ;
  skos:inScheme     :Ontology .

:73
  a               skos:Concept ;
  skos:prefLabel  "Bay"@en, "Veld"@nl ;
  skos:definition "Abstract designation of a coupling point on a rail. Contains the connection and protection, but a field can also be empty (in which case the switch does allow for something to be connected in the future)"@en,
                  "Abstracte benoeming van een koppelpunt op een rail. Bevat de verbinding en de beveiliging, maar een veld kan ook leeg zijn (dan biedt de schakelinstallatie wel de mogelijkheid om in de toekomst iets te koppelen)"@nl ;
  skos:editorialNote
                  """Velden op een rail kunnen verbonden zijn met andere stations (kabelveld), een transformator (trafoveld) of met een andere rail in dezelfde installatie (koppelveld)"""@nl ;
  skos:altLabel   "ALV", "Afgaand Veld"@nl ;
  skos:note       "it's not a piece of equipment by itself but a container that groups components which are physically adjacent and functionally related."@en ;
  skos:broadMatch eq:EquipmentContainer ;
  skos:broader    :105 ;
  dct:identifier  "urn:uuid:24441efb-914a-5b51-b0e0-8458c977d02e" ;
  dct:type        archi:BusinessObject ;
  owl:versionInfo "1" ;
#  skos:topConceptOf :Ontology ;
  skos:inScheme   :Ontology .

:74
  a               skos:Concept ;
  skos:prefLabel  "ACLineSegment"@en, "Kabel"@nl ;
  skos:definition "Elektriciteitskabel waarmee elektrische energie kan worden getransporteerd of gedistribueerd. Kabels worden door middel van moffen galvanisch aan elkaar verbonden. Samen met de eindsluitingen vormt de gehele samenstelling van kabels waar door middel van een schakelaar de connectie met de netvoeding verbonden of verbroken kan worden, één Verbinding."@nl ;
  skos:note       """LV-main cable"""@nl, """LS-hoofdkabel"""@nl ;
  skos:broader    :105 ;
  dct:identifier  "urn:uuid:443cb89d-6f1b-5298-ac54-d8cfe7350227" ;
  dct:type        archi:BusinessObject ;
  rdfs:seeAlso    <https://phasetophase.nl/boek/boek_1_4.html#_4.1> ;
  owl:versionInfo "1" ;
#  skos:topConceptOf :Ontology ;
  skos:inScheme   :Ontology .

:75
  a                 skos:Concept ;
  skos:prefLabel    "Market Evaluation Point"@en ;
  skos:altLabel     "MEP" ;
  skos:definition   """A Market Evaluation Point is a logical point in the electricity system at which market-relevant quantities—such as energy consumption, production, or flexibility—are measured, aggregated, or allocated for use in market processes."""@en,
                    """Een marktevaluatiepunt is een logisch punt in het elektriciteitssysteem waar marktgerelateerde hoeveelheden – zoals energieverbruik, productie of flexibiliteit – worden gemeten, samengevoegd of toegewezen voor gebruik in marktprocessen."""@nl ;
  skos:relatedMatch eq:EnergyConsumer, maw:MarketParticipant ;
  skos:exactMatch   maw:MarketEvaluationPoint ;
  skos:narrowMatch  lido37940:130, lido37940:161 ;
  dct:identifier    "urn:uuid:801a94c4-14f0-52df-9904-21c119086668" ;
  dct:type          archi:BusinessObject ;
  owl:versionInfo   "1" ;
  skos:topConceptOf :Ontology ;
  skos:inScheme     :Ontology .

:76
  a                 skos:Concept ;
  skos:prefLabel    "Market Participant"@en ;
  skos:definition   """A Market Participant is an entity that participates in one or more energy markets by producing, consuming, trading, or providing flexibility, capacity, or ancillary services."""@en,
                    """Een marktdeelnemer is een entiteit die deelneemt aan een of meer energiemarkten door te produceren, te consumeren, te handelen of flexibiliteit, capaciteit of ondersteunende diensten te leveren."""@nl ;
  skos:editorialNote
                    """This actor enables operating demand and response products for capacity management in energy balancing, congestion management, and voltage control."""@nl ;
  skos:example      "An example of market participant on the grid and from the DSO perspective would be a customer using the grid to either consume electricity, produce electricity, or both." ;
  skos:relatedMatch elit:944-25 ;
  skos:exactMatch   elit:943-25, maw:MarketParticipant ;
  dct:identifier    "urn:uuid:6818069a-c337-5661-bba4-912595695fd8" ;
  dct:type          archi:BusinessObject, archi:BusinessActor ;
  owl:versionInfo   "1" ;
  skos:topConceptOf :Ontology ;
  skos:inScheme     :Ontology .

:77
  a                 skos:Concept ;
  skos:prefLabel    "Current Violation"@en ;
  skos:definition   """A situation where the current exceeds or falls below specified limits in the distribution system"""@en ;
  skos:relatedMatch elit:631-31 ;
  dct:identifier    "urn:uuid:3e2f3b1e-1f3e-5c4e-8f3a-5c6e7d8f9a0b" ;
  owl:versionInfo   "1" ;
  skos:topConceptOf :Ontology ;
  skos:inScheme     :Ontology .

:78
  a                 skos:Concept ;
  skos:prefLabel    "Voltage Violation"@en ;
  skos:definition   "A situation where the voltage exceeds or falls below specified limits in the distribution system"@en ;
  skos:relatedMatch elit:631-3 ;
  skos:narrowMatch  elit:1485-145 ;
  dct:identifier    "urn:uuid:4f5e6d7c-8b9a-0b1c-2d3e-4f5a6b7c8d9e" ;
  owl:versionInfo   "1" ;
  skos:topConceptOf :Ontology ;
  skos:inScheme     :Ontology .

:79
  a                 skos:Concept ;
  skos:prefLabel    "Active Power Violation"@en ;
  skos:definition   "A situation where the active power exceeds or falls below specified limits in the distribution system"@en ;
  skos:relatedMatch elit:631-20 ;
  dct:identifier    "urn:uuid:5a6b7c8d-9e0f-1a2b-3c4d-5e6f7a8b9c0d" ;
  owl:versionInfo   "1" ;
  skos:topConceptOf :Ontology ;
  skos:inScheme     :Ontology .

:80
  a                 skos:Concept ;
  skos:prefLabel    "Reactive Power Violation"@en ;
  skos:definition   "A situation where the reactive power exceeds or falls below specified limits in the distribution system"@en ;
  skos:relatedMatch elit:631-28 ;
  dct:identifier    "urn:uuid:6b7c8d9e-0f1a-2b3c-4d5e-6f7a8b9c0d1e" ;
  owl:versionInfo   "1" ;
  skos:topConceptOf :Ontology ;
  skos:inScheme     :Ontology .

:81
  a                  skos:Concept ;
  skos:prefLabel     "Energy System Integration"@en, "Energie Systeem Integratie"@nl ;
  skos:definition    "Energy system integration means creating stronger links between different types of energy carriers (such as electricity, liquid, gas and solid fuels, heat and cold), energy infrastructure and consumption sectors. This integration supports the optimisation of the energy system to deliver decarbonised, reliable and resource-efficient energy services, at the least possible cost. "@en ;
  skos:editorialNote """EU policy documents such as the EU Strategy for Energy System Integration (2020) explain 'energy system integration' as: 'the coordinated planning and operation of the energy system as a whole, across multiple energy carriers and connected infrastructure, and all final consumers.'
The aim: optimise energy services by linking electricity, gas, heat, cooling, and fuels more closely, improving efficiency and facilitating decarbonization."""@en ;
  skos:related       :63 ;
  foaf:homepage      <https://energy.ec.europa.eu/topics/eus-energy-system/energy-system-integration_en> ;
  skos:changeNote    "In Review"@en ;
  dct:identifier     "urn:uuid:8d9e0f1a-2b3c-4d5e-6f7a-8b9c0d1e2f3a" ;
  owl:versionInfo    "1" ;
  skos:topConceptOf  :Ontology ;
  skos:inScheme      :Ontology .

:82
  a               skos:Concept ;
  skos:prefLabel  "Product"@en, "Product"@nl ;
  skos:definition "Any interoperable good or service, including interconnected or related offering."@en ;
  dc:source       "IEC 60050 (IEV 902-02-03, 904-01-07)" ;
  skos:narrower   :83, :36 ;
  skos:changeNote "In Review"@en ;
  owl:versionInfo "1" ;
  dct:identifier  "urn:uuid:7c8d9e0f-1a2b-3c4d-5e6f-7a8b9c0d1e2f" ;
  dct:type        archi:BusinessObject ;
#  skos:topConceptOf :Ontology ;
  skos:inScheme   :Ontology .

:83
  a                 skos:Concept ;
  skos:prefLabel    "Market Product"@en, "Markt Product"@nl ;
  skos:definition   """A Market Product is a standardized good or service traded in an energy market, such as energy, capacity, or ancillary services."""@en,
                    """Een marktproduct is een gestandaardiseerd goed of dienst dat op een energiemarkt wordt verhandeld, zoals energie, capaciteit of ondersteunende diensten."""@nl ;
  skos:editorialNote
                    """For example, market products could include energy contracts, capacity or ancillary services exchanged using IEC 62325 standards"""@en ;
  skos:broader      :82 ;
  skos:exactMatch   maw:MarketProduct ;
  skos:related      :36 ;
  skos:relatedMatch elit:944-20, elit:1485-93 ;
  skos:changeNote   "In Review"@en ;
  owl:versionInfo   "1" ;
  dct:identifier    "urn:uuid:9e0f1a2b-3c4d-5e6f-7a8b-9c0d1e2f3a4b" ;
  dct:type          archi:BusinessObject ;
#  skos:topConceptOf :Ontology ;
  skos:inScheme     :Ontology .

:84
  a                 skos:Concept ;
  skos:prefLabel    "Voltage Agnostic"@en, "Spanningsonafhankelijk"@nl ;
  skos:definition   "This means the ability of a device, system, or function to operate independently of the specific voltage level applied."@en ;
  skos:editorialNote
                    """Voltage agnostic refers to an IT system that operates independently of the voltage level. It can function effectively across a range of voltages without requiring specific adaptations or configurations for each voltage level."""@en ;
  skos:changeNote   "In Review"@en ;
  dct:identifier    "urn:uuid:0f1a2b3c-4d5e-6f7a-8b9c-0d1e2f3a4b5c" ;
  owl:versionInfo   "1" ;
  skos:topConceptOf :Ontology ;
  skos:inScheme     :Ontology .

:85
  a                 skos:Concept ;
  skos:prefLabel    "Aangeslotene"@nl, "Connected Customer"@en ;
  skos:definition   """A natural person or legal entity that is connected to the electricity grid. A connected customer can be a consumer, producer, or prosumer of electricity."""@en,
                    """Een natuurlijk persoon of rechtspersoon die is aangesloten op het elektriciteitsnet. Een aangesloten klant kan een verbruiker, producent of prosument van elektriciteit zijn."""@nl ;
  skos:exactMatch   lido37940:1 ;
  skos:relatedMatch hemrm:PartyConnectedToTheGrid, hemrm:Producer, hemrm:Consumer, hemrm:FlexibilityServiceProvider ;
  owl:versionInfo   "1" ;
  dct:identifier    "urn:uuid:60d4740f-4f6b-421b-baaa-05f2685fd72d" ;
  dct:type          archi:BusinessActor ;
  skos:topConceptOf :Ontology ;
  skos:inScheme     :Ontology .

:86
  a                 skos:Concept ;
  skos:prefLabel    "Congestion"@en, "Congestie"@nl ;
  skos:definition   """In the context of an electricity network, congestion means that there is too much demand or too much supply of electricity at a certain point in the network, causing the transport capacity of the network (cables, transformers, or connections) to be temporarily or structurally insufficient to handle all desired energy flows."""@en,
                    """In de context van een elektriciteitsnetwerk betekent congestie dat er teveel vraag of teveel aanbod van elektriciteit is op een bepaald punt in het net, waardoor de transportcapaciteit van het netwerk (kabels, transformatoren of verbindingen) tijdelijk of structureel onvoldoende is om alle gewenste energiestromen te verwerken."""@nl ;
  skos:editorialNote
                    """The characteristic of the energy system produced by a constraint on the optimum economic operation, such that the marginal price of energy to serve the next increment of load, exclusive of losses, at different locations on the energy system is unequal"""@en ;
  skos:exactMatch   elit:943-4 ;
  skos:relatedMatch lido37940:33 ;
  skos:narrower     :31, :28 ;
  skos:related      :29 ;
  owl:versionInfo   "1" ;
  dct:identifier    "urn:uuid:4283e541-2bdc-43bd-a10e-fad0baf09732" ;
  skos:topConceptOf :Ontology ;
  skos:inScheme     :Ontology .

:87
  a                 foaf:Agent, skos:Concept ;
  skos:prefLabel    "Charge Point Operator"@en, "Laadpuntbeheerder"@nl ;
  skos:altLabel     "CPO" ;
  skos:definition   "means a Charge Point Operator represents a Market Participant with the Market Role responsible for the maintenance and commercial exploitation of and communication with the charge station."@en ;
  dct:identifier    "urn:uuid:326993f1-1b8d-51e0-859f-2352fd9dfbfd" ;
  dct:type          archi:BusinessActor ;
  owl:versionInfo   "1" ;
  skos:topConceptOf :Ontology ;
  skos:inScheme     :Ontology .

:88
  a                 skos:Concept ;
  skos:prefLabel    "Grid Aware Charging"@en, "Net bewust Laden"@nl ;
  skos:altLabel     "NBL" ;
  skos:definition   "means Grid Aware Charging, also described as Grid Friendly Charging. Net bewust Laden is a term that describes the methodology of reducing peak loads on the (distribution) grid caused by electric vehicles charging at charge stations."@en ;
  dct:identifier    "urn:uuid:fb57faf3-23c0-506e-ab9d-9f3fd0edac25" ;
  owl:versionInfo   "1" ;
  skos:topConceptOf :Ontology ;
  skos:inScheme     :Ontology .

:89
  a                 skos:Concept ;
  skos:prefLabel    "Ramp Up Period"@en, "Oplopende Periode"@nl ;
  skos:definition   """Period at the beginning of the active interval expressed as a Duration, during which a registered resource moves from its former state to its requested state to comply with new operational condition.If there is no ramp up period, then all other rules are processed as if there were a ramp up period of zero length."""@en,
                    """Periode aan het begin van het actieve interval, uitgedrukt als een duur, waarin een geregistreerde bron van zijn vorige staat naar zijn gevraagde staat beweegt om te voldoen aan nieuwe operationele voorwaarden. Als er geen oplopende periode is, worden alle andere regels verwerkt alsof er een oplopende periode van nul lengte was."""@nl ;
  dct:identifier    "urn:uuid:52957a81-7d0e-505f-a685-0c60daa38fb8" ;
  owl:versionInfo   "1" ;
  skos:topConceptOf :Ontology ;
  skos:inScheme     :Ontology .

:90
  a                 skos:Concept ;
  skos:prefLabel    "Recovery Period"@en ;
  skos:definition   """Period at the end of the Active availability window expressed as a Duration during which the effect of the response may be reversed while the system returns to its base operational condition.If negative, then the recovery period occurs within the bounds of the activation window, i.e. it ends at the same moment as does the activation window."""@en ;
  dct:identifier    "urn:uuid:6a6b3bae-6ea8-5c86-80a8-2ecc65066691" ;
  owl:versionInfo   "1" ;
  skos:topConceptOf :Ontology ;
  skos:inScheme     :Ontology .

:91
  a                 skos:Concept ;
  skos:prefLabel    "Elementary Equipment"@en, "Elementaire Apparatuur"@nl ;
  skos:definition   """An elementary equipment refers to a basic, indivisible component that performs a specific electrical or functional role and cannot be decomposed further within the modeling or operational framework"""@en,
                    """Een elementaire apparatuur verwijst naar een basis, ondeelbaar component dat een specifieke elektrische of functionele rol vervult en niet verder kan worden ontleed binnen het model- of operationele kader"""@nl ; ;
  owl:versionInfo   "1" ;
  skos:broadMatch   eq:ConductingEquipment, eq:Equipment ;
  dct:identifier    "urn:uuid:1b2538d9-43f4-4e52-88d7-4599bc421710" ;
  dct:type          archi:BusinessObject ;
  skos:topConceptOf :Ontology ;
  skos:inScheme     :Ontology .

:92
  a                 skos:Concept ;
  skos:prefLabel    "Infeed"@en, "Terug Levering"@nl ;
  skos:altLabel     "Export Energy"@en ;
  skos:definition   "Infeed is the delivery of electricity to the grid by a producer or a consumer who generates electricity themselves."@en,
                    "Teruglevering is het terugleveren van elektriciteit aan het net door een producent of een consument die zelf elektriciteit opwekt."@nl ;
  foaf:homepage     <https://alliander.atlassian.net/wiki/x/BwKnxQ> ;
  owl:versionInfo   "1" ;
  dct:identifier    "urn:uuid:c81b7da3-96c8-4d75-81f3-5c646ddaaeaf" ;
  skos:topConceptOf :Ontology ;
  skos:inScheme     :Ontology .

:93
  a                 skos:Concept ;
  skos:prefLabel    "Schedule"@en, "Program"@nl ;
  skos:definition   """A schedule means a timestamped representation of expected behaviour on related Registered Resource / Registered Inter Ties. Schedules are requested by a Market Participant and are provided by the DSO. A schedule describes the capacity in (active and reactive power, current and, voltage) that is assigned to the Market Participant."""@en ;
  dct:identifier    "urn:uuid:dd1d8e96-2bca-59de-bfb5-5875e5225458" ;
  dct:type          archi:BusinessObject ;
  skos:relatedMatch elit:1485-44, elit:943-25 ;
  skos:relatedMatch maw:RegisteredResource, maw:RegisteredInterTie ;
  owl:versionInfo   "1" ;
  skos:topConceptOf :Ontology ;
  skos:inScheme     :Ontology .

:94
  a                 skos:Concept ;
  skos:prefLabel    "Programmable Time Unit"@en, "Programmeerbare Tijdseenheid"@nl ;
  skos:altLabel     "PTU" ;
  skos:definition   "represents a single timestamped entry within a schedule.Trading intervals in electricity markets (Program Time Unit or Imbalance Settlement Period). Effectively another term for a quarter-hour value."@en,
                    "Een enkele tijdstempel binnen een schema. Handelsintervallen in elektriciteitsmarkten (Program Time Unit of Imbalance Settlement Period). Effectief een andere term voor een kwartierwaarde."@nl ;
  dct:identifier    "urn:uuid:6b162f61-250f-584c-ba0e-81bda695e9cd" ;
  skos:exactMatch   elit:2195-30 ;
  owl:versionInfo   "1" ;
  skos:topConceptOf :Ontology ;
  skos:inScheme     :Ontology .

:95
  a                 skos:Concept ;
  skos:prefLabel    "Charging Station"@en ;
  skos:definition   "It means the physical system where EVs can be charged, and is behind the point of common coupling."@en ;
  dct:created       "2025-04-23"^^xsd:date ;
  dct:identifier    "urn:uuid:9cf29ba3-b6cf-52fc-8e9a-6d95f8aed96f" ;
  owl:versionInfo   "1" ;
  skos:topConceptOf :Ontology ;
  skos:inScheme     :Ontology .

:96
  a                 skos:Concept ;
  skos:prefLabel    "Market Schedule"@en, "Marktschema"@nl ;
  skos:definition   """A Market Schedule defines the planned allocation of energy or capacity for a specific market product over defined time intervals. It represents the outcome of market clearing, assigning resources based on market results and merit order. For ancillary services, it specifies the allocation of reserve capacity to eligible resources."""@en,
                    """Een marktschema definieert de geplande toewijzing van energie of capaciteit voor een specifiek marktproduct over bepaalde tijdsintervallen. Het vertegenwoordigt het resultaat van marktclearing, waarbij middelen worden toegewezen op basis van marktresultaten en verdienste. Voor ondersteunende diensten specificeert het de toewijzing van reservecapaciteit aan in aanmerking komende middelen."""@nl ;
  skos:example      """A MarketSchedule might specify that a power producer will deliver 100 MW from 1 PM to 2 PM tomorrow."""@en ;
  skos:relatedMatch elit:943-25 ;
  skos:broadMatch   elit:1485-44 ;
  dc:source         "IEC 61968-1" ;
  dct:identifier    "urn:uuid:4f23391b-b464-5aa0-bde6-92983586dcd1" ;
  dct:type          archi:BusinessObject ;
  owl:versionInfo   "1" ;
  skos:topConceptOf :Ontology ;
  skos:inScheme     :Ontology .

:97
  a                 skos:Concept ;
  skos:prefLabel    "Operational Constraints"@en, "Operationele Beperkingen"@nl ;
  skos:definition   "means a condition for the market participant in which there is need to activate and comply with a remedial action to respect operational security limits"@en,
                    "Een voorwaarde voor de marktdeelnemer waarin het nodig is om een herstelmaatregel te activeren en te voldoen aan operationele veiligheidslimieten"@nl ;
  skos:altLabel     "OC" ;
  dct:identifier    "urn:uuid:dc6108fb-8a0d-5d1a-adb2-a7c2196119da" ;
  dct:type          archi:BusinessObject ;
  owl:versionInfo   "1" ;
  skos:related      :98 ;
  skos:relatedMatch elit:1485-1, elit:1222-7, elit:943-25 ;
  skos:topConceptOf :Ontology ;
  skos:inScheme     :Ontology .

:98
  a                 skos:Concept ;
  skos:prefLabel    "Remedial Action"@en, "Herstelmaatregel"@nl ;
  skos:altLabel     "RA"@en ;
  skos:definition   """A remedial action is described by one of many grid state alterations applied to a grid model state or particular scenario in order to resolve one or more Identified constraints. Only costly remedial actions require a cost characteristic.
Remedial action describes one or more actions that can be performed on a given power system model situation to eliminate one or more identified breaches of constraints. The remedial action can be costly, and have a cost characteristic, or non costly.
"""@en ;
  skos:editorialNote
                    """"A named set of operating constraints imposed on one or more market participants or assets, which must be validated via real-time or near-real-time measurements, and whose purpose is to mitigate a specific system risk or condition."""@en ;
  rdfs:seeAlso      <https://eepublicdownloads.entsoe.eu/clean-documents/EDI/Library/cim_based/Contingency%20list,%20remedial%20actions%20and%20additional%20constraints_document%20UML%20model%20and%20schema_v2.4.pdf> ;
  rdfs:seeAlso      <https://eepublicdownloads.entsoe.eu/clean-documents/CIM_documents/Grid_Model_CIM/Remedial_action_settlement_document_UML_model_and_schema_v1.2.pdf> ;
  skos:relatedMatch elit:1485-1 ;
  skos:exactMatch   elit:1222-13 ;
  dct:identifier    "urn:uuid:c9b6db85-b0a3-53bf-ab46-1aea6544a5db" ;
  dct:type          archi:BusinessObject ;
  owl:versionInfo   "1" ;
  skos:topConceptOf :Ontology ;
  skos:inScheme     :Ontology .

:99
  a                 skos:Concept ;
  skos:prefLabel    "TenneT Pocket"@en, "TenneT Pocket"@nl ;
  skos:definition   "means a coherent part of the interconnected system, operated by a single System Operator and shall include connected HV/MV/LV electrotechnical components.To divide the area of TenneT into pockets that are all connected to the 120 or 220 and 380 KV grid make net compartments."@en ;
  dct:identifier    "urn:uuid:62e227b4-7ce1-55ed-85ca-bf2b394af0ab" ;
  dct:type          archi:BusinessObject ;
  owl:versionInfo   "1" ;
  skos:relatedMatch elit:943-67 ;
  skos:narrowMatch  eq:ControlArea ;
  skos:topConceptOf :Ontology ;
  skos:inScheme     :Ontology .

:100
  a               skos:Concept ;
  skos:prefLabel  "Control Action"@en, "Controle Actie"@nl ;
  skos:definition """An intervention performed to control or adjust the state of an conducting equipment in the power system."""@en,
                  """Een interventie die wordt uitgevoerd om de staat van een geleidend component in het elektriciteitsnet te beheersen of aan te passen."""@nl ; ;
  skos:example    """Adjusting the forecasted energy load on a EnergyConsumer based on a settlement condition."""@en ;
  skos:related    :98, :102 ;
  dct:identifier  "urn:uuid:dd09ea05-7cf5-5113-9f85-57f5655e0b1a" ;
  dct:type        archi:BusinessObject ;
  owl:versionInfo "1" ;
  skos:inScheme   :Ontology ;
  skos:inScheme   :Ontology .

:102
  a                 skos:Concept ;
  skos:prefLabel    "Remedial Action Plan"@en ;
  skos:altLabel     "RAP" ;
  skos:definition   """A predefined set of actions to be taken by a system operator or utility to maintain or restore power system security and stability following a disturbance or outage. Actions may include generator redispatch, load shedding, or network reconfiguration."""@en ;
  dct:identifier    "urn:uuid:0f1b6c3d-2a4e-5b8c-9f7d-8c1e2f3a4b5c" ;
  dct:type          archi:BusinessObject ;
  owl:versionInfo   "1" ;
  skos:related      :98 ;
  skos:topConceptOf :Ontology ;
  skos:inScheme     :Ontology .

:103
  a                 skos:Concept ;
  skos:prefLabel    "Delivery Period"@en ;
  skos:definition   """means the period of delivery of a during which the flexibility service provider delivers the full requested change of power in-feed to, or the full requested change of withdrawals from the system."""@en ;
  skos:related      :98 ;
  skos:narrowMatch  elit:2195-32 ;
  dct:identifier    "urn:uuid:3c1f5b6a-7d8e-5f9b-8a1c-2b3d4e5f6a7b" ;
  owl:versionInfo   "1" ;
  skos:topConceptOf :Ontology ;
  skos:inScheme     :Ontology .

:104
  a                skos:Concept ;
  skos:prefLabel   "Contingency Equipment"@en, "Knelpuntcomponent"@nl ;
  skos:definition  """A Contingency Equipment means an equipment identified in advance, or as a result of contingency analysis, to model and manage the impact of potential failures on on system security and operational performance."""@en,
                   """Onder een knelpuntcomponent wordt verstaan: apparatuur die vooraf of op basis van een analyse is geïdentificeerd om de impact van mogelijke storingen op de veiligheid en operationele prestaties van het systeem te modelleren en te beheren."""@nl ;
  skos:broadMatch  cim:ContingencyElement ;
  skos:narrowMatch cim:ContingencyEquipment ;
  dct:type         archi:BusinessObject ;
  skos:broader     :12 ;
  skos:related     elit:1222-10 ;
  dct:identifier   "urn:uuid:8499a071-beef-4076-9040-660556d58f69" ;
  owl:versionInfo  "1" ;
#  skos:topConceptOf :Ontology ;
  skos:inScheme    :Ontology .

:105
  a                 skos:Concept ;
  skos:prefLabel    "Conducting Equipment"@en, "Geleidend Component"@nl ;
  skos:altLabel     "Component"@nl ;
  skos:definition   """Conducting Equipment comprises physical components of the power system designed to carry or interrupt electrical current. It includes lines, transformers, busbars, breakers, and switches that form the conductive path between terminals and support connectivity and limit modelling."""@en,
                    """Geleidende apparatuur bestaat uit fysieke componenten van het energiesysteem die zijn ontworpen om elektrische stroom te geleiden of te onderbreken. Het omvat leidingen, transformatoren, stroomrails, stroomonderbrekers en schakelaars die het geleidende pad tussen aansluitingen vormen en connectiviteit en beperkende modellering ondersteunen."""@nl ;
  skos:example      """
  - conductors (such as wires, busbars, and cables)
  - connection components (such as terminals and joints)
  """@en ;
  skos:narrower     :43, :70, :73 ;
  skos:related      :62, :71, :104 ;
  skos:broadMatch   eq:Equipment ;
  skos:exactMatch   eq:ConductingEquipment ;
  skos:relatedMatch elit:1222-10 ;
  dc:source         "IEC 60050 (IEV 151-11-25)" ;
  rdfs:seeAlso      <https://electropedia.org/iev/iev.nsf/display?openform&ievref=151-11-25> ;
  dct:identifier    "urn:uuid:e0c67167-568e-4361-b9dc-b3251bf6a0a8" ;
  dct:type          archi:BusinessObject ;
  owl:versionInfo   "2" ;
  skos:topConceptOf :Ontology ;
  skos:inScheme     :Ontology .

:106
  a                 skos:Concept ;
  skos:prefLabel    "Terminal"@en, "Terminal"@nl ;
  skos:definition   """A Terminal is a conductive connection point of a piece of conducting equipment that defines how the equipment electrically connects to the network via connectivity nodes."""@en,
                    """Een terminal is een geleidend verbindingspunt van een stuk geleidend apparatuur dat bepaalt hoe de apparatuur elektrisch wordt aangesloten op het netwerk via connectiviteitsknooppunten."""@nl ;
  skos:narrowMatch  eq:Terminal ;
  skos:note         """This means a terminal is a point of electrical connection — a physical conductive component designed to connect a wire, a busbar, or another piece of equipment — allowing the flow of current into or out of the apparatus."""@en ;
  dc:source         "IEC 60050 (IEV 151-12-12)" ;
  dct:identifier    "urn:uuid:70ac9b15-f539-4edc-83bf-400e2bd1852f" ;
  dct:type          archi:BusinessObject ;
  foaf:homepage     <https://alliander.atlassian.net/l/cp/duZf6PeN> ;
  rdfs:seeAlso      <https://netbeheer-nederland.github.io/docs/im-tc57cim/latest/schema/class/Terminal.html> ;
  rdfs:seeAlso      <https://electropedia.org/iev/iev.nsf/display?openform&ievref=151-12-12> ;
  owl:versionInfo   "1" ;
  skos:topConceptOf :Ontology ;
  skos:inScheme     :Ontology .

:107
  a                 skos:Concept ;
  skos:prefLabel    "Equipment Container"@en, "Component container"@nl ;
  skos:altLabel     "Composite equipment"@en ;
  skos:definition   """Container or enclosure designed to provide an assembly of electrical equipment to fulfil specific purposes."""@en,
                    """Container of behuizing, die is ontworpen om elektrische apparatuur samen te voegen voor specifieke doeleinden."""@nl ;
  skos:narrowMatch  eq:EquipmentContainer ;
  skos:editorialNote
                    """An equipment container acts as an composite equipment and refers to a higher-level assembly composed of multiple interconnected elementary equipment that together perform a more complex or coordinated function."""@en ;
  skos:example      """A substation, which may include transformers, switchgear, and other equipment, is an example of an equipment container that houses various conducting equipment to manage and control electrical power flow."""@en ;
  skos:example      """A busbar chamber, which contains busbars and associated connections, is an example of an equipment container that provides a physical and functional assembly for conducting equipment."""@en ;
  skos:example      """A feeder section, which contains multiple cables, breakers and measurement devices to manage the flow of electricity in a specific section of the distribution network."""@en ;
  foaf:homepage     <https://alliander.atlassian.net/l/cp/A87VmG3T> ;
  dct:identifier    "urn:uuid:55f084ed-67ad-4621-80d4-f425b0165091" ;
  dct:type          archi:BusinessObject ;
  owl:versionInfo   "1" ;
  skos:topConceptOf :Ontology ;
  skos:inScheme     :Ontology .

:108
  a                 skos:Concept ;
  skos:prefLabel    "Analog"@en, "Meeting"@nl ;
  skos:definition   """Of a quantity or a system in which the information is represented by a physical variable that is continuous in time and/or magnitude."""@en,
                    """Van een grootheid of een systeem waarbij de informatie wordt weergegeven door een fysieke variabele die continu is in tijd en/of grootte."""@nl ;
  skos:exactMatch   op:Analog ;
  skos:broadMatch   op:Measurement ;
  dc:source         "IEC 60050 (IEV 351-41-24)" ;
  dct:identifier    "urn:uuid:6c5743a7-72d0-4cff-81d1-0fdda1d56813" ;
  dct:type          archi:BusinessObject ;
  dct:type          archi:BusinessObject ;
  foaf:homepage     <https://alliander.atlassian.net/wiki/x/e4_AvQ> ;
  rdfs:seeAlso      <https://alliander.atlassian.net/wiki/x/xwd_wg> ;
  rdfs:seeAlso      <https://electropedia.org/iev/iev.nsf/display?openform&ievref=351-41-24> ;
  owl:versionInfo   "1" ;
  skos:topConceptOf :Ontology ;
  skos:inScheme     :Ontology .

:109
  a                 skos:Concept ;
  skos:prefLabel    "Topological Island"@en, "Topologisch Eiland"@nl ;
  skos:definition   """A Topological Island is an electrically connected subset of the network that remains connected under a given topology configuration. It defines the effective electrical boundary used in contingency analysis and security assessments."""@en,
                    """Een topologisch eiland is een elektrisch verbonden subset van het netwerk die verbonden blijft onder een bepaalde topologieconfiguratie. Het definieert de effectieve elektrische grens die wordt gebruikt in noodsituatieanalyses en veiligheidsbeoordelingen."""@nl ;
  skos:exactMatch   ssh:TopologicalIsland ;
  skos:related      tp:TopologicalNode, elit:1222-10, cim:ContingencyEquipment ;
  skos:note         """Only energised TopologicalNode-s shall be part of the topological island."""@en ;
  skos:note         """The main role of TopologicalIsland is to group nodes that are internally connected and disconnected from all other groups in the network, allowing power flow and stability calculations to treat it as an independent network."""@en ;
  skos:broadMatch   elit:1485-64 ;
  foaf:homepage     <https://alliander.atlassian.net/l/cp/Y1DNs37g> ;
  dct:identifier    "urn:uuid:081006e5-e0b9-4551-b8ed-eb84fe8b9fd9" ;
  dct:type          archi:BusinessObject ;
  owl:versionInfo   "1" ;
  skos:topConceptOf :Ontology ;
  skos:inScheme     :Ontology .

:110
  a                 skos:Concept ;
  skos:prefLabel    "Curtailment"@en, "Afregeling"@nl ;
  skos:definition   """means the deliberate reduction of electricity generation or consumption initiated by the system operator to manage congestion or ensure system security."""@en,
                    """betekent dat de teruglevercapaciteit van een opwekinstallatie onder bepaalde voorwaarden tijdelijk wordt verminderd."""@nl ;
  skos:broadMatch   elit:943-26, elit:1485-91 ;
  dct:identifier    "urn:uuid:c34fac28-3997-40d4-90a5-814ade44505e" ;
  owl:versionInfo   "1" ;
  skos:narrower     :111, :112 ;
  skos:topConceptOf :Ontology ;
  skos:inScheme     :Ontology .

:111
  a               skos:Concept ;
  skos:prefLabel  "Load curtailment"@en ;
  skos:altLabel   "Load shedding"@en ;
  skos:definition """The deliberate disconnection or reduction of electrical load (typically by the system operator) to maintain the stability and integrity of the power system when there is a shortage of available generation or a risk of system collapse."""@en ;
  skos:note       """EU legislation (such as network codes and Regulation (EU) 2019/943) frequently refers to load shedding as a last-resort measure under emergency conditions, when the power system is under stress and other measures (like redispatch, reserve activation, or voltage reductions) are no longer enough to keep it within operational limits."""@en ;
  skos:exactMatch elit:1485-109 ;
  skos:broader    :110 ;
  dct:identifier  "urn:uuid:361ed7ea-88c2-4ba3-94c8-6292ee78bd45" ;
  owl:versionInfo "1" ;
#  skos:topConceptOf :Ontology ;
  skos:inScheme   :Ontology .

:112
  a               skos:Concept ;
  skos:prefLabel  "Generation curtailment"@en ;
  skos:definition """The deliberate disconnection or reducing a generator's output, such as wind or solar (typically by the system operator) to maintain grid stability or avoid overloading, when there is a shortage of available load or a risk of system collapse."""@en ;
  skos:broader    :110 ;
  dct:identifier  "urn:uuid:29e75445-bff2-430e-99d3-11fe1d7fcc88" ;
  owl:versionInfo "1" ;
#  skos:topConceptOf :Ontology ;
  skos:inScheme   :Ontology .

:113
  a                  skos:Concept ;
  skos:prefLabel     "N Limit"@en, "N Limiet"@nl ;
  skos:altLabel      "Congestion limit"@en, "Congestie Limiet"@nl ;
  skos:definition    """The N Limit refers to situation where a forecasted or realised power flow violates operational security limits, such as (a) the thermal limit of element(s) of the grid or (b) voltage stability or (c) the angle stability limits of the grid."""@en,
                     """"""@nl ;
  skos:editorialNote """The congestion limit is an example of the N Limit, beyond which congestion occurs."""@en ;
  rdfs:seeAlso       <https://www.entsoe.eu/network_codes/cacm/> ;
  rdfs:seeAlso       <https://energy.ec.europa.eu/topics/energy-efficiency/energy-efficiency-targets-directive-and-rules/energy-efficiency-directive_en> ;
  skos:relatedMatch  elit:943-4, elit:1222-18, elit:1485-3 ;
  skos:changeNote    "In Review"@en ;
  dct:identifier     "urn:uuid:2e826219-82a5-4bb6-94f9-ee0316157159" ;
  dct:type           archi:BusinessObject ;
  owl:versionInfo    "1" ;
  skos:topConceptOf  :Ontology ;
  skos:inScheme      :Ontology .

:114
  a                 skos:Concept ;
  skos:prefLabel    "N-1 Limit"@en, "N-1 Limiet"@nl ;
  skos:altLabel     "BZIV", "Bedrijfszeker installatievermogen"@nl ;
  skos:definition   """The N-1 Limit refers to the maximum allowable operational state of a power system such that, following the unexpected loss (contingency) of any single system element (such as a transmission line, transformer, or generator), the remaining elements within a control area are still capable of maintaining operational security. This means that no operational security limits—such as voltage, frequency, or thermal loading thresholds—are violated after the contingency occurs."""@en,
                    """De N-1 Limiet verwijst naar de maximaal toelaatbare operationele staat van een elektriciteitssysteem, zodanig dat na het onverwachte verlies (contingentie) van een enkel systeemonderdeel (zoals een transmissielijn, transformator of generator), de resterende onderdelen binnen een controlegebied nog steeds in staat zijn om de operationele veiligheid te handhaven. Dit betekent dat er geen operationele veiligheidslimieten - zoals spannings-, frequentie- of thermische belastingsdrempels - worden overschreden nadat de contingentie zich voordoet."""@nl ; ;
  skos:changeNote   "In Review"@en ;
  skos:relatedMatch elit:1485-15, elit:1485-14 ;
  dct:identifier    "urn:uuid:8cedf8d0-4909-5019-88ac-f0d904c0bf04" ;
  dct:type          archi:BusinessObject ;
  owl:versionInfo   "1" ;
  skos:topConceptOf :Ontology ;
  skos:inScheme     :Ontology .

:115
  a                 skos:Concept ;
  skos:prefLabel    "System Operating Limit"@en, "Systeem Operationele Limiet"@nl ;
  skos:definition   """An System Operating Limit defines the secure operational boundaries of the energy system—such as voltage, frequency, and load/generation capacity—within which flexibility services, including demand & response, can be safely activated by market-based flexibility providers. These limits ensure that system reliability and equipment protection are maintained while enabling market participation in grid balancing and congestion management, in line with EU electricity market design and regulatory frameworks."""@en,
                    """Een Systeem Operationele Limiet definieert de veilige operationele grenzen van het energiesysteem - zoals spanning, frequentie en laad-/opwekkingscapaciteit - binnen welke flexibiliteitsdiensten, inclusief vraag & aanbod, veilig kunnen worden geactiveerd door marktgebaseerde flexibiliteitsaanbieders. Deze limieten zorgen ervoor dat de systeembetrouwbaarheid en apparatuurbescherming worden gehandhaafd, terwijl marktdeelname aan netbalancering en congestiebeheer wordt mogelijk gemaakt, in lijn met het EU-ontwerp van de elektriciteitsmarkt en regelgevende kaders."""@nl ;
  skos:changeNote   "In Review"@en ;
  rdfs:seeAlso      <https://www.nerc.com/pa/comp/guidance/EROEndorsedImplementationGuidance/System_Operating_Limit_definition_and_Exceedance_Clarification_endorsed.pdf> ;
  dct:identifier    "urn:uuid:ea6f5ec0-f562-4f40-b5b0-4e7526b30963" ;
  dct:type          archi:BusinessObject ;
  owl:versionInfo   "1" ;
  skos:broader      :60 ;
  skos:topConceptOf :Ontology ;
  skos:inScheme     :Ontology .

:116
  a                  skos:Concept ;
  skos:prefLabel     "Maximum Continuous Load"@en, "Maximale Continue Belasting"@nl ;
  skos:definition    "means the highest amount of power or current an asset can safely carry continuously under normal operating conditions, as specified by design standards or supplier ratings."@en,
                     "betekent de hoogste hoeveelheid vermogen of stroom die een actief component veilig continu kan dragen onder normale bedrijfsomstandigheden, zoals gespecificeerd door ontwerpnormen of leveranciersbeoordelingen."@nl ; ;
  skos:editorialNote "The load can be expressed in power or current."@en ;
  skos:narrower      :117, :118, :119, :120 ;
  skos:changeNote    "In Review"@en ;
  dct:identifier     "urn:uuid:9aab67e8-549b-4ac0-bbf3-aabe50336877" ;
  owl:versionInfo    "1" ;
  skos:topConceptOf  :Ontology ;
  skos:inScheme      :Ontology .

:117
  a                 skos:Concept ;
  skos:prefLabel    "Nominal Asset Limit"@en, "Nominale Component Limiet"@nl ;
  skos:definition   "means the the maximum continuous load an electrical asset can safely sustain continuously under normal conditions, as defined by standards or supplier specifications. This value, known as the nominal asset limit, sets the standard maximum capacity for safe and reliable operation."@en,
                    "betekent de maximale continue belasting die een elektrisch component veilig kan dragen onder normale omstandigheden, zoals gedefinieerd door normen of leveranciersspecificaties. Deze waarde, bekend als de nominale component limiet, stelt de standaard maximale capaciteit vast voor veilige en betrouwbare werking."@nl ;
  skos:changeNote   "In Review"@en ;
  skos:broader      :116 ;
  dct:identifier    "urn:uuid:43e4c8a0-3c0c-4652-b696-f097aa86bd3e" ;
  dct:type          archi:BusinessObject ;
  owl:versionInfo   "1" ;
  skos:topConceptOf :Ontology ;
  skos:inScheme     :Ontology .

:118
  a                 skos:Concept ;
  skos:prefLabel    "Static Equipment Limit"@en, "Statische Component Limiet"@nl ;
  skos:definition   "means the maximum continuous load an electrical asset can carry under constant load and specific, location-based environmental conditions, defined by the asset’s nominal value at the maximum steady-state temperature."@en,
                    "betekent de maximale continue belasting die een elektrisch component kan dragen onder constante belasting en specifieke, locatiegebonden omgevingsomstandigheden, gedefinieerd door de nominale waarde van het component bij de maximale stationaire temperatuur."@nl ; ; ;
  skos:changeNote   "In Review"@en ;
  skos:broader      :116 ;
  dct:identifier    "urn:uuid:22aefa12-75d9-4ac4-98eb-599409d02bbe" ;
  dct:type          archi:BusinessObject ;
  owl:versionInfo   "1" ;
  skos:topConceptOf :Ontology ;
  skos:inScheme     :Ontology .

:119
  a                 skos:Concept ;
  skos:prefLabel    "Cyclic Equipment Limit"@en, "Cyclische Component Limiet"@nl ;
  skos:definition   "means the maximum load an electrical asset can safely carry over a defined period, based on a scaled, periodic load profile and considering environmental conditions that may change over time."@en,
                    "betekent de maximale belasting die een elektrisch component veilig kan dragen over een gedefinieerde periode, gebaseerd op een geschaalde, periodieke belastingprofiel en rekening houdend met omgevingsomstandigheden die in de loop van de tijd kunnen veranderen."@nl ; ;
  skos:changeNote   "In Review"@en ;
  skos:broader      :116 ;
  dct:identifier    "urn:uuid:8242c025-9d63-4b0c-b9d9-0d6ef8ef5926" ;
  dct:type          archi:BusinessObject ;
  owl:versionInfo   "1" ;
  skos:topConceptOf :Ontology ;
  skos:inScheme     :Ontology .

:120
  a                 skos:Concept ;
  skos:prefLabel    "Dynamic Equipment Limit"@en, "Dynamische Component Limiet"@nl ;
  skos:definition   "means the real-time maximum load an electrical asset can safely carry, determined by a predicted load profile and current environmental conditions for short-term periods (intraday or day-ahead), and calculated using a validated model."@en,
                    "betekent de maximale stroom die een elektrisch component veilig kan dragen, bepaald door een voorspeld belastingprofiel en actuele omgevingsomstandigheden voor kortetermijnperioden (intraday of dag vooruit), en berekend met behulp van een gevalideerd model."@nl ; ; ;
  skos:changeNote   "In Review"@en ;
  skos:broader      :116 ;
  owl:versionInfo   "1" ;
  dct:identifier    "urn:uuid:e75279d3-81e6-435b-96a2-dc6bd37e34dd" ;
  dct:type          archi:BusinessObject ;
  skos:topConceptOf :Ontology ;
  skos:inScheme     :Ontology .

:121
  a                 skos:Concept ;
  skos:prefLabel    "Resource"@en ;
  skos:definition   "delivers the capability to modify generation injection and/or consumption patterns in the energy system (like electricity or gas). It is a market representation of an asset, or a group of assets having this capability. A Resource represents for example grid assets, energy generating units, energy consuming units, energy storing units or a virtual power plant."@en ;
  skos:altLabel     "Flexibility Resource"@en ;
  skos:editorialNote
                    """A Resource is a market representation of an asset, or a group of assets having the capability to modify generation injection and/or consumption patterns in the energy system (like electricity or gas)."""@en ;
  skos:example      """A Resource can be a single generator, a group of generators, or even a virtual power plant that aggregates multiple generation units to provide flexibility services to the grid."""@en ;
  skos:related      elit:1485-44, elit:943-25 ;
  dct:identifier    "urn:uuid:77d99843-fc5e-40a5-9f29-4641b354b6a7" ;
  dct:type          archi:BusinessObject ;
  owl:versionInfo   "1" ;
  skos:topConceptOf :Ontology ;
  skos:inScheme     :Ontology .

:122
  a               skos:Concept ;
  skos:prefLabel  "Circuit"@en, "Circuit"@nl ;
  skos:definition """A circuit is a logical electrical construct composed of one or more islands, (closed)bridges and their interconnections, used to represent feeders or supply paths for operational and analytical purposes."""@en,
                  """Een circuit is een logische elektrische constructie die bestaat uit een of meer eilanden, (gesloten) bruggen en hun onderlinge verbindingen, die worden gebruikt om voedingskabels of toevoerpaden weer te geven voor operationele en analytische doeleinden."""@nl ;
  skos:editorialNote
                  """The most simple version of a Circuit is an Island, but can be aggregated to higher levels to form logical models like the Feeder."""@en ;
  skos:related    :69 ;
  skos:broader    :27 ;
  dct:identifier  "urn:uuid:4def7553-e3f6-454b-b064-1c4e5ebce03f" ;
  dct:type        archi:BusinessObject ;
  owl:versionInfo "1" ;
#  skos:topConceptOf :Ontology ;
  skos:inScheme   :Ontology .

:123
  a               skos:Concept ;
  skos:prefLabel  "Island"@en, "NetEiland"@nl ;
  skos:definition "An Island is the smallest not switchable part of the grid (Connectivity) were all Equipments have the same BaseVoltage."@en,
                  "Een NetEiland is het kleinste niet-schakelbare deel van het net (Connectiviteit) waar alle Componenten dezelfde BasisSpanning hebben."@nl ;
  skos:related    :122, :26 ;
  skos:broader    :27 ;
  dct:identifier  "urn:uuid:1e7ac12b-6126-4ac8-a588-679df37adb1f" ;
  dct:type        archi:BusinessObject ;
  owl:versionInfo "1" ;
#  skos:topConceptOf :Ontology ;
  skos:inScheme   :Ontology .

:124
  a                  skos:Concept ;
  skos:prefLabel     "Bridge"@en, "Brug"@nl ;
  skos:definition    "A Bridges form the boundaries of a Island and consists of a PowerTransformer or a combination of one or multiple switching Equipments."@en,
                     "Een Brug vormt de grens van een NetEiland en bestaat uit een PowerTransformer of een combinatie van één of meerdere schakelcomponenten."@nl ;
  skos:editorialNote """Bridges based on a power transformer with a designated power supply."""@en ;
  skos:related       :26, :49, :122 ;
  skos:broader       :27 ;
  dct:identifier     "urn:uuid:78c14c4a-bdd6-4858-bc83-0b1b8104b8ca" ;
  dct:type           archi:BusinessObject ;
  owl:versionInfo    "1" ;
#  skos:topConceptOf :Ontology ;
  skos:inScheme      :Ontology .

:125
  a               skos:Concept ;
  skos:prefLabel  "Asset Management"@en, "Assetbeheer"@nl ;
  skos:definition "Asset Management in the energy domain encompasses systematically managing the energy assets in scope with their characteristics. It involves the strategic utilization of data, technology, and best practices to achieve optimal performance, cost-effectiveness, and sustainability of energy asset operations."@en ;
  dct:identifier  "urn:uuid:1b9f7cbb-fd15-4be0-859e-ead30e77cd71" ;
  dct:type        archi:BusinessCollaboration ;
  owl:versionInfo "1" ;
  skos:broader    :25 ;
#  skos:topConceptOf :Ontology ;
  skos:inScheme   :Ontology .

:126
  a               skos:Concept ;
  skos:prefLabel  "Grid Management"@en, "Netbeheer"@nl ;
  skos:definition "It is the optimization of, and coordination in, the functionality of any energy grid. It involves avoidance and solving outages, enabling work* activities in the grid while ensuring the safety through all controls in the grid."@en ;
  dct:identifier  "urn:uuid:79ee8ea2-5918-4641-b315-48d7ef88aadf" ;
  dct:type        archi:BusinessCollaboration ;
  owl:versionInfo "1" ;
  skos:broader    :25 ;
#  skos:topConceptOf :Ontology ;
  skos:inScheme   :Ontology .

:127
  a               skos:Concept ;
  skos:prefLabel  "Capacity Management"@en, "Capaciteitsbeheer"@nl ;
  skos:definition "Capacity management is the practice of aligning demand and response for transport and distribution capacity among DSO’s, TSO and market participants at total scope of the DSO’s energy system, at specific area’s and at timeframes, to ensure a safety through all controls in the system."@en ;
  dct:identifier  "urn:uuid:f43ed679-3f20-4010-92e8-8e5e25fc10ee" ;
  dct:type        archi:BusinessCollaboration ;
  owl:versionInfo "1" ;
  skos:broader    :25 ;
#  skos:topConceptOf :Ontology ;
  skos:inScheme   :Ontology .

:128
  a               skos:Concept ;
  skos:prefLabel  "Market Management"@en, "Marktbeheer"@nl ;
  skos:definition "Organize and coordinate transport and distribution capacity with several market participants under several national and international market mechanisms, currently limited to capacity management market(s) including the energy system reliability."@en ;
  dct:identifier  "urn:uuid:8d1e39df-d077-4d18-b587-1bca1b910055" ;
  dct:type        archi:BusinessCollaboration ;
  owl:versionInfo "1" ;
  skos:broader    :25 ;
#  skos:topConceptOf :Ontology ;
  skos:inScheme   :Ontology .

:129
  a                 skos:Concept ;
  skos:prefLabel    "Multiple Suppliers on a single Connection"@en, "Meerdere Leveranciers op een aansluiting"@nl ;
  skos:altLabel     "MLOEA" ;
  skos:definition   "means that more than one supplier can deliver energy to or take off energy from a single connection point to the energy system."@en,
                    "betekent dat meer dan één leverancier energie kan leveren aan of energie kan afnemen van een enkel aansluitpunt op het energiesysteem."@nl ;
  dct:identifier    "urn:uuid:893b11aa-28cc-4040-8ee3-e9b46db9c878" ;
  owl:versionInfo   "1" ;
  skos:topConceptOf :Ontology ;
  skos:inScheme     :Ontology .

:130
  a                  skos:Concept ;
  skos:prefLabel     "Ordinary contingency"@en ;
  skos:altLabel      "Point Contingency"@en, "Point System Operation"@en ;
  skos:definition    "Loss of a single element (branch, injection, etc.). These are more frequent / higher probability.” "@en ;
  skos:example       "E.g. one transmission line goes out, one transformer, one generator, or one demand facility fails."@en ;
  skos:editorialNote "These are more frequent / higher probability."@en ;
  dct:identifier     "urn:uuid:111bc9ed-ca1d-494f-acef-4b4f7acd72d5" ;
  dct:type           archi:BusinessObject ;
  dct:source         "ENTSO-E" ;
  skos:changeNote    "In Review"@en ;
  skos:broader       :54 ;
  owl:versionInfo    "1" ;
#  skos:topConceptOf  :Ontology ;
  skos:inScheme      :Ontology .

:131
  a               skos:Concept ;
  skos:prefLabel  "Exceptional contingency"@en ;
  skos:altLabel   "Area Contingency"@en, "Area System Operation"@en ;
  skos:definition "Simultaneous loss of multiple elements that share a common cause. These are rarer than ordinary, but still foreseen in planning/operations."@en ;
  skos:example    "E.g. multiple lines that share the same tower; cables in the same trench; multiple generators under a protection scheme failing together."@en ;
  dct:identifier  "urn:uuid:f36d2a05-ea6d-4f68-a9f4-a34592e589c5" ;
  dct:type        archi:BusinessObject ;
  dct:source      "ENTSO-E" ;
  skos:broader    :54 ;
  owl:versionInfo "1" ;
#  skos:topConceptOf :Ontology ;
  skos:inScheme   :Ontology .

:132
  a                  skos:Concept ;
  skos:prefLabel     "Out-of-range contingency"@en ;
  skos:definition    "Simultaneous loss of multiple elements without a common cause, or loss of generating modules exceeding some “reference incident” (i.e. very large severity or rare events)."@en ;
  skos:example       "E.g. multiple independent failures, or large generation loss beyond what is usually assumed in planning."@en ;
  skos:editorialNote "These are very rare, high‐impact."@en ;
  dct:identifier     "urn:uuid:86b4425a-3c1c-4b52-88ad-6b5e2b0806cc" ;
  dct:type           archi:BusinessObject ;
  dct:source         "ENTSO-E" ;
  skos:broader       :54 ;
  owl:versionInfo    "1" ;
#  skos:topConceptOf  :Ontology ;
  skos:inScheme      :Ontology .

:133
  a               skos:Concept ;
  skos:prefLabel  "Conducting Equipment Limit"@en ;
  skos:definition """A Conducting Equipment Limit defines the maximum load that conducting equipment (such as cables, busbars, or connectors) can safely carry without exceeding its thermal or design constraints, under specified operating and environmental conditions."""@en,
                  """Een limiet voor geleidende apparatuur definieert de maximale belasting die geleidend materieel (zoals kabels, rails of connectoren) veilig kan dragen zonder de thermische of ontwerpbeperkingen te overschrijden, onder gespecificeerde bedrijfs- en omgevingsomstandigheden."""@nl ;
  skos:scopeNote  "Intrinsic to device characteristics."@en ;
  dct:identifier  "urn:uuid:22e27483-108b-4545-9cf2-db96d53c0afa" ;
  dct:type        archi:BusinessObject ;
  skos:broader    :71 ;
  skos:changeNote "In Review"@en ;
  owl:versionInfo "1" ;
#  skos:topConceptOf :Ontology ;
  skos:inScheme   :Ontology .

:134
  a               skos:Concept ;
  skos:prefLabel  "Equipment Container Limit"@en, "Aggregeerde limiet"@nl ;
  skos:altLabel   "System Limit - K&O" ;
  skos:definition "A limit that applies to an equipment container (e.g., substation, bay, voltage level), representing aggregated or contextual security constraints such as transfer capacity, voltage stability, or short-circuit withstand."@en ;
  skos:scopeNote  "Emerges from power system context rather than individual device properties."@en ;
  skos:editorialNote
                  """The System Limit is used by K&O for expressing the BZIV (BedrijsZekerInstallatieVermogen - Installatie) and a Chain (Keten) """@en,
                  """De System Limit wordt door K&O gebruikt voor het uitdrukken van het BZIV (BedrijfsZekerInstallatieVermogen - Installatie) en een Keten (Keten)"""@nl ;
  skos:broader    :71 ;
  skos:changeNote "In Review"@en ;
  owl:versionInfo "1" ;
  dct:identifier  "urn:uuid:92f84fda-3145-4e04-b7fc-85c5cc9a9466" ;
  dct:type        archi:BusinessObject ;
#  skos:topConceptOf :Ontology ;
  skos:inScheme   :Ontology .

:135
  a                 skos:Concept ;
  skos:prefLabel    "System Flexibility"@en ;
  skos:definition   "System flexibility is defined as the ability of supply-side and demand-side resources to respond to system changes and uncertainties. Flexibility also includes the ability to store energy for delivery in the future and the operational flexibility to schedule/dispatch resources in the most efficient manner."@en ;
  dct:identifier    "urn:uuid:1343037e-a73a-4f88-9541-d334db0c40e4" ;
  dct:source        "NERC" ;
  rdfs:seeAlso      "https://www.nerc.com/pa/RAPA/ra/Reliability%20Assessments%20DL/IVGTF_Task_1_5_Final.pdf" ;
  owl:versionInfo   "1" ;
  skos:topConceptOf :Ontology ;
  skos:inScheme     :Ontology .

:136
  a                 skos:Concept ;
  skos:prefLabel    "Distributed Energy Source"@en, "Gedistribueerde Energiebron"@nl ;
  skos:altLabel     "DER" ;
  skos:definition   "A device that produces/consumes electricity and is connected to the electrical system, either 'behind the meter' in the customer's premises, or on the utility's primary distribution system"@en ;
  dct:identifier    "urn:uuid:ffcd97ef-a332-4e78-b1ef-0c3f56e0bed2" ;
  dct:type          archi:BusinessObject ;
  owl:versionInfo   "1" ;
  skos:topConceptOf :Ontology ;
  skos:inScheme     :Ontology .

:137
  a                 skos:Concept ;
  skos:prefLabel    "Transactive energy"@en, "Transactieve energie"@nl ;
  skos:definition   "A system of economic and control mechanisms that allows the dynamic balance of supply and demand across the entire electrical infrastructure using value as a key operational parameter"@en,
                    "Een systeem van economische en regelmechanismen dat de dynamische balans tussen vraag en aanbod over de gehele elektrische infrastructuur mogelijk maakt, waarbij waarde als een belangrijke operationele parameter wordt gebruikt"@nl ;
  dct:identifier    "urn:uuid:e163a9ab-e0a5-4c9b-b806-0cc82445dd69" ;
  owl:versionInfo   "1" ;
  skos:topConceptOf :Ontology ;
  skos:inScheme     :Ontology .

:138
  a                  skos:Concept ;
  skos:prefLabel     "Behind the Meter"@en, "Achter de Meter"@nl ;
  skos:altLabel      "BTM" ;
  skos:definition    "Anything located behind the point of transfer, allocation point, or meter and outside the direct responsibility of the network operator."@en,
                     "Alles wat zich achter het overdrachtspunt, allocatiepunt of de meter bevindt en buiten de directe verantwoordelijkheid van de netbeheerder valt."@nl ;
  dct:identifier     "urn:uuid:1edc2391-5e5d-4062-a7cc-32a17c2a5fc8" ;
  skos:editorialNote """The European Commission and the Agency for the Cooperation of Energy Regulators (ACER) use the term 'Behind-the-Meter' in technical documents and network codes, such as:
* NC RfG (Requirements for Generators)
* NC DCC (Demand Connection Code)
These codes set requirements for installations that are connected to the grid, including those located behind the meter. The EU recognizes BTM systems as essential for flexibility, decentralized generation, and end-user participation in the energy market."""@en, """De Europese Commissie en het Agentschap voor de samenwerking tussen energieregulators (ACER) hanteren het begrip Behind-the-Meter in technische documenten en netcodes, zoals:
* NC RfG (Requirements for Generators)
* NC DCC (Demand Connection Code)
Deze codes stellen eisen aan installaties die op het net worden aangesloten, inclusief die zich achter de meter bevinden. De EU erkent BTM-systemen als essentieel voor flexibiliteit, decentrale opwek en participatie van eindgebruikers in de energiemarkt"""@nl ;
  owl:versionInfo    "1" ;
  rdfs:seeAlso       <https://energiehubs.nl/begrippen/achter-de-meter> ;
  skos:topConceptOf  :Ontology ;
  skos:inScheme      :Ontology .

:139
  a                 skos:Concept ;
  skos:prefLabel    "Operational Technology"@en, " Operationele Technologie"@nl ;
  skos:altLabel     "OT" ;
  skos:definition   "This refers to hardware and software systems used to control and monitor physical processes in critical infrastructures, including manufacturing, energy. transportation, and utilities."@en,
                    "Dit verwijst naar hardware- en softwaresystemen die worden gebruikt om fysieke processen in kritieke infrastructuren te controleren en te monitoren, waaronder productie, energie, transport en nutsbedrijven."@nl ;
  skos:editorialNote
                    "Also: Industrial Automation, Industrial (Automated) Control Systems, Process Automation & Control -IA, ICS, IACS or PAC" ;
  dct:identifier    "urn:uuid:d38e73fe-5a82-49c9-826b-16d9c713117d" ;
  owl:versionInfo   "1" ;
  skos:topConceptOf :Ontology ;
  skos:inScheme     :Ontology .

:140
  a                 skos:Concept ;
  skos:prefLabel    "Service Delivery Point"@en, "Dienstverleningspunt"@nl ;
  skos:definition   """A Service Delivery Point is the physical or virtual location where a flexibility or demand‑response service is operationally delivered. It defines where activation is measured or controlled and may represent aggregated or virtualized resources."""@en,
                    """Een dienstverleningspunt is de fysieke of virtuele locatie waar een flexibiliteits- of vraagresponsdienst operationeel wordt geleverd. Het bepaalt waar activering wordt gemeten of gecontroleerd en kan geaggregeerde of gevirtualiseerde middelen vertegenwoordigen."""@nl ;
  dct:identifier    "urn:uuid:44c64086-4b28-40f4-b6d9-d7e143150585" ;
  dct:type          archi:BusinessObject ;
  owl:versionInfo   "1" ;
  skos:topConceptOf :Ontology ;
  skos:inScheme     :Ontology .

:141
  a                 skos:Concept ;
  skos:prefLabel    "Energy Profile"@en, "Energie Profiel"@nl ;
  skos:definition   """An energy profile represents a time-series description of energy quantities associated with a specific market purpose, such as schedules, forecasts, nominations, or measurements. It expresses how much energy is attributed to discrete time intervals under defined market, contractual, and operational conditions."""@en,
                    """Een energie profiel vertegenwoordigt een tijdreeksbeschrijving van energiekwantiteiten die verband houden met een specifiek marktdoel, zoals schema's, prognoses, nominaties of metingen. Het geeft weer hoeveel energie wordt toegerekend aan afzonderlijke tijdsintervallen onder gedefinieerde markt-, contractuele en operationele omstandigheden."""@nl ;
  dct:identifier    "urn:uuid:3bee7daf-28c4-4c84-ac97-d4c923ed3bee" ;
  dct:type          archi:BusinessObject ;
  owl:versionInfo   "1" ;
  skos:topConceptOf :Ontology ;
  skos:inScheme     :Ontology .

:142
  a                 skos:Concept ;
  skos:prefLabel    "Reference Line"@en ;
  skos:altLabel     "baseline"@en ;
  skos:definition   "A reference line (also called baseline) is the best approximation of the normal load or generation curve for an Accounting Point or Resource (group) without flexibility services being invoked"@en ;
  dct:identifier    "urn:uuid:2c68da1b-73c3-4f03-bf54-1467f0c67d1b" ;
  owl:versionInfo   "1" ;
  skos:topConceptOf :Ontology ;
  skos:inScheme     :Ontology .

:143
  a                  skos:Concept ;
  skos:prefLabel     "Active Customer"@en, "Actieve Afnemer"@nl ;
  skos:definition    "An active consumer is an end consumer who not only purchases electricity, but also produces, stores, shares, sells, or uses it flexibly, and can assume one or more market roles as long as this remains a secondary activity."@en,
                     "Een actieve afnemer is een eindafnemer die elektriciteit niet alleen afneemt, maar ook produceert, opslaat, deelt, verkoopt of flexibel inzet, en daarbij één of meerdere marktrollen kan aannemen zolang dit een nevenactiviteit blijft."@nl ;
  skos:editorialNote "The Explanatory Memorandum states that an active buyer may assume various market roles."@en,
                     "In de Memorie van toelichting wordt gesteld dat een actieve afnemer verschillende marktrollen mag aannemen."@nl ;
  skos:scopeNote     """
Within the ENTSO-E Harmonised Electricity Market Role Model (HEMRM), an Active Customer
is not a distinct market role but a participation pattern. Depending on its activities,
the Active Customer may assume one or more market roles such as Consumer, Producer,
and/or Flexibility Service Provider, either directly or via representation (e.g. an
Aggregator).
"""@en ;
  dct:identifier     "urn:uuid:1e77eec1-f03e-410a-8a9e-7e055a4db02d" ;
  dct:type           archi:BusinessObject, archi:BusinessActor ;
  skos:relatedMatch  elit:944-8 ;
  skos:exactMatch    lido50714:5 ;
  skos:related       hemrm:Consumer, hemrm:Producer, hemrm:FlexibilityServiceProvider, hemrm:ResourceAggregator ;
  rdfs:seeAlso       <https://energiedatawijzer.nl/wp-content/uploads/Topicdocument-TS087-Actieve-afnemer-als-zelfstandige-marktdeelnemer-versie-1.0-1.pdf> ;
  eli:based_on       <http://data.europa.eu/eli/dir/2019/944/oj> ;
  owl:versionInfo    "1" ;
  skos:topConceptOf  :Ontology ;
  skos:inScheme      :Ontology .

:144
  a                 skos:Concept ;
  skos:prefLabel    "Head End"@en ;
  skos:definition   "A component of a metering system that collects data from and issues controls to end devices"@en ;
  dct:identifier    "uri:uuid:99c74106-060b-40d2-8e6c-a6d27a9977b2" ;
  dct:source        "IEC 61968-9:2014" ;
  skos:exactMatch   amw:HeadEnd ;
  owl:versionInfo   "1" ;
  skos:topConceptOf :Ontology ;
  skos:inScheme     :Ontology .

:145
  a                 skos:Concept ;
  skos:prefLabel    "Network Model"@en ;
  skos:definition   "The Network Model business object includes the functional description of the network grid that used in one or more network analysis."@en ;
  skos:editorialNote
                    """The model supports the grid in several defined state (build, operational, energized) to perform a hypothesis."""@en ;
  skos:related      :26 ;
  dct:identifier    "urn:uuid:a22344b5-1e68-4e03-b627-084dae2f2ec5" ;
  owl:versionInfo   "1" ;
  skos:topConceptOf :Ontology ;
  skos:inScheme     :Ontology .

:146
  a                 skos:Concept ;
  skos:prefLabel    "Exchange Point"@en ;
  skos:definition   "A domain for establishing energy exchange between two Metering Grid Areas. Additional information: This is a type of Metering Point"@en ;
  dct:identifier    "urn:uuid:3ce73295-57d8-4508-b67c-3fa310331e21" ;
  dct:type          archi:BusinessObject ;
  skos:topConceptOf :Ontology ;
  skos:inScheme     :Ontology .


:147
  a                 skos:Concept ;
  skos:prefLabel    "Metering Point"@en ;
  skos:definition   "An entity where energy products are measured or computed."@en ;
  dct:identifier    "urn:uuid:0321934c-64fe-41d8-9605-24afe410be86" ;
  dct:type          archi:BusinessObject ;
  skos:topConceptOf :Ontology ;
  skos:inScheme     :Ontology .


:148
  a                 skos:Concept ;
  skos:prefLabel    "Accounting Point"@en ;
  skos:definition   "A domain under balance responsibility where Energy Supplier change can take place and for which commercial business processes are defined."@en ;
  dct:identifier    "urn:uuid:b11f8ea7-376a-49a5-9641-3f09bb32ad05" ;
  dct:type          archi:BusinessObject ;
  skos:topConceptOf :Ontology ;
  skos:inScheme     :Ontology .


:149
  a                 skos:Concept ;
  skos:prefLabel    "Auction"@en ;
  skos:definition   ""@en ;
  dct:identifier    "urn:uuid:63b43846-b24d-4db4-b84b-d785faeff274" ;
  dct:type          archi:BusinessObject ;
  skos:topConceptOf :Ontology ;
  skos:inScheme     :Ontology .


:150
  a                 skos:Concept ;
  skos:prefLabel    "Domain"@en ;
  skos:definition   ""@en ;
  dct:identifier    "urn:uuid:b6b7f41f-a5ed-48bc-9fa4-fd67a74c721a" ;
  dct:type          archi:BusinessObject ;
  skos:topConceptOf :Ontology ;
  skos:inScheme     :Ontology .


:151
  a                 skos:Concept ;
  skos:prefLabel    "Market"@en ;
  skos:definition   ""@en ;
  dct:identifier    "urn:uuid:779fb060-7362-417f-aa20-cb4bac26092d" ;
  dct:type          archi:BusinessObject ;
  skos:topConceptOf :Ontology ;
  skos:inScheme     :Ontology .


:152
  a                 skos:Concept ;
  skos:prefLabel    "Market Role"@en ;
  skos:definition   ""@en ;
  dct:identifier    "urn:uuid:a0d43d4a-d52f-4dec-89db-96643aede841" ;
  dct:type          archi:BusinessObject ;
  skos:topConceptOf :Ontology ;
  skos:inScheme     :Ontology .


:153
  a                 skos:Concept ;
  skos:prefLabel    "Period"@en ;
  skos:definition   ""@en ;
  dct:identifier    "urn:uuid:e006886d-8dcb-4b26-8e5a-db7d9d3ee9c8" ;
  dct:type          archi:BusinessObject ;
  skos:topConceptOf :Ontology ;
  skos:inScheme     :Ontology .


:154
  a                 skos:Concept ;
  skos:prefLabel    "Point"@en ;
  skos:definition   ""@en ;
  dct:identifier    "urn:uuid:b3126cd2-48d2-417f-bcbf-8a9de456e6d2" ;
  dct:type          archi:BusinessObject ;
  skos:topConceptOf :Ontology ;
  skos:inScheme     :Ontology .


:155
  a                 skos:Concept ;
  skos:prefLabel    "Quantity"@en ;
  skos:definition   ""@en ;
  dct:identifier    "urn:uuid:96bc5d30-8278-4d04-80b2-97d1dd279a0f" ;
  dct:type          archi:BusinessObject ;
  skos:topConceptOf :Ontology ;
  skos:inScheme     :Ontology .


:156
  a                 skos:Concept ;
  skos:prefLabel    "Reason"@en ;
  skos:definition   ""@en ;
  dct:identifier    "urn:uuid:0b70fd06-a923-4e54-a1b8-ddb35e87b3bc" ;
  dct:type          archi:BusinessObject ;
  skos:topConceptOf :Ontology ;
  skos:inScheme     :Ontology .


:157
  a                 skos:Concept ;
  skos:prefLabel    "Registered Resource"@en ;
  skos:definition   "A Resource delivers the capability to modify generation injection and/or consumption patterns in the energy system (like electricity or gas). It is a market representation of an asset, or a group of assets having this capability.  A Resource represents for example grid assets, energy generating units, energy consuming units, energy storing units or a virtual power plant.  http://data.acer.europa.eu/terms/TechnicalResource  DER"@en ;
  dct:identifier    "urn:uuid:e0dfa767-0ac4-4c2c-9a34-f50608f9a165" ;
  dct:type          archi:BusinessObject ;
  skos:topConceptOf :Ontology ;
  skos:inScheme     :Ontology .


:158
  a                 skos:Concept ;
  skos:prefLabel    "Resource Capacity"@en ;
  skos:definition   ""@en ;
  dct:identifier    "urn:uuid:9acc2f4b-343d-4983-b494-51467f39eb7b" ;
  dct:type          archi:BusinessObject ;
  skos:topConceptOf :Ontology ;
  skos:inScheme     :Ontology .


:159
  a                 skos:Concept ;
  skos:prefLabel    "Service Category"@en ;
  skos:definition   "The different types of services that may be used by an organization, i.e., electric, gas, water"@en ;
  dct:identifier    "urn:uuid:f5ff107d-5bd1-410e-ba88-1ac8105a608c" ;
  dct:type          archi:BusinessObject ;
  skos:topConceptOf :Ontology ;
  skos:inScheme     :Ontology .


:160
  a                 skos:Concept ;
  skos:prefLabel    "End Device Asset"@en ;
  skos:definition   "- iec 61968-14  section in profile: - ComFunction - ConnectDisconnetFunction - ElectricMeteringFunction - EndDeviceAsset - ReadingType - Register  "@en ;
  dct:identifier    "urn:uuid:782873b4-eace-4f9f-a160-c42506af65e0" ;
  dct:type          archi:BusinessObject ;
  skos:topConceptOf :Ontology ;
  skos:inScheme     :Ontology .


:161
  a                 skos:Concept ;
  skos:prefLabel    "SDP Location"@en ;
  skos:definition   "- iec 61968-14  Service Delivery Point configuration. SDPLocationConfig contains additional position point information in addition to mail address and contact information."@en ;
  dct:identifier    "urn:uuid:7205a27d-7a46-43b7-9944-d9334f6c76b1" ;
  dct:type          archi:BusinessObject ;
  skos:topConceptOf :Ontology ;
  skos:inScheme     :Ontology .


:162
  a                 skos:Concept ;
  skos:prefLabel    "Service Location"@en ;
  skos:definition   ""@en ;
  dct:identifier    "urn:uuid:5cc2a799-6ce2-42c9-867f-0e4f5b0d690d" ;
  dct:type          archi:BusinessObject ;
  skos:topConceptOf :Ontology ;
  skos:inScheme     :Ontology .


:163
  a                 skos:Concept ;
  skos:prefLabel    "Remedial Action Schedules"@en ;
  skos:definition   "The Remedial Action Schedules business object includes the description of preventive, curative and restorative remedial action and the schedule for the activation. System Integrity Protection Scheme (SIPS) would be part of the network model. However, activation and arming of existing SIPS would be part of remedial action schedules. In addition, it includes proposals for new SIPS as part of system development planning.  == Remedial Action Plan --> Remedial Action -->   Remedial Action Schedules (as defined in Operating Constrains)"@en ;
  dct:identifier    "urn:uuid:3b45cff9-2ec2-4399-b3e1-5c8b005c8fa3" ;
  dct:type          archi:BusinessObject ;
  skos:topConceptOf :Ontology ;
  skos:inScheme     :Ontology .


:164
  a                 skos:Concept ;
  skos:prefLabel    "Availability Schedule"@en ;
  skos:definition   "The Availability Schedule business object includes the time intervals during which a grid element is available or not.   For grid elements normally in service, the focus is on the period that the grid element will not be available to provide functionality to the network. For grid elements normally out of service, or that have been forced out of service through network constrains or faults, the focus would be on when it is back in service.   For grid elements in test mode, the focus is on the period during which it will be in service."@en ;
  dct:identifier    "urn:uuid:c5e49ea0-914b-4684-955c-2d5d9fca4512" ;
  dct:type          archi:BusinessObject ;
  skos:topConceptOf :Ontology ;
  skos:inScheme     :Ontology .


:165
  a                 skos:Concept ;
  skos:prefLabel    "Adequate Assessment"@en ;
  skos:definition   "The Adequate Assessment business object includes the assessment of expected consumption compared to available production and transmission capacity."@en ;
  dct:identifier    "urn:uuid:4379ce3c-b1cf-4583-aa49-43f2ab91df9b" ;
  dct:type          archi:BusinessObject ;
  skos:topConceptOf :Ontology ;
  skos:inScheme     :Ontology .


:166
  a                 skos:Concept ;
  skos:prefLabel    "Operational Settings Schedule"@en ;
  skos:definition   "The Operational Settings business object includes the schedule for: • device status (switch status, tap position, shunt bank position); • control settings (voltage regulation, flow regulation);  • monitoring (operational limit determination, critical grid elements, topology limitation (power transfer corridors) and stability limits."@en ;
  dct:identifier    "urn:uuid:2ce5d574-b244-44fb-aca4-4434b6807dd5" ;
  dct:type          archi:BusinessObject ;
  skos:topConceptOf :Ontology ;
  skos:inScheme     :Ontology .


:167
  a                 skos:Concept ;
  skos:prefLabel    "Contingency List"@en ;
  skos:definition   "The Contingency List business object includes the list of grid elements that should be included as part of contingency assessment"@en ;
  dct:identifier    "urn:uuid:24170a73-6af3-42be-85da-9f77fc5606a7" ;
  dct:type          archi:BusinessObject ;
  skos:topConceptOf :Ontology ;
  skos:inScheme     :Ontology .


:168
  a                 skos:Concept ;
  skos:prefLabel    "Planned Customer Outage"@en ;
  skos:definition   "The Planned Customer Outage business object describe a planned event and the related information in regard to not being able to deliver the customer the committed service according to the customer agreement. The customer may or may not be compensated. The customer is informed in advance of planned outages. The reason for the outages is normally related to new construction, maintenance or repair either directly on the customer installation or to a nearby part of the Customer Installation connected to the grid."@en ;
  dct:identifier    "urn:uuid:5c87bbd8-320d-45a2-9715-9af992201483" ;
  dct:type          archi:BusinessObject ;
  skos:topConceptOf :Ontology ;
  skos:inScheme     :Ontology .


:169
  a                 skos:Concept ;
  skos:prefLabel    "Network Capacity Assessment"@en ;
  skos:definition   ""@en ;
  dct:identifier    "urn:uuid:e36c6b72-96a2-4dff-bb8d-3248f653e269" ;
  dct:type          archi:BusinessObject ;
  skos:topConceptOf :Ontology ;
  skos:inScheme     :Ontology .


:170
  a                 skos:Concept ;
  skos:prefLabel    "Swtiching Schedule"@en ;
  skos:definition   "The Switching Schedule business object includes the schedule and sequence for the opening and closing of switches."@en ;
  dct:identifier    "urn:uuid:bce10b9b-eee0-4baa-b88b-fbcc67973b79" ;
  dct:type          archi:BusinessObject ;
  skos:topConceptOf :Ontology ;
  skos:inScheme     :Ontology .


:171
  a                 skos:Concept ;
  skos:prefLabel    "Predictive Energy Schedule"@en ;
  skos:definition   "Scheduled energy volume submitted to EPEX for day-ahead market. Contains 96 quarter-hour intervals. Forms basis for imbalance calculation when compared with allocation."@en ;
  dct:identifier    "urn:uuid:f4dd9f7e-af84-4eab-0915-5f6630c2f4dd" ;
  dct:type          archi:BusinessObject ;
  skos:topConceptOf :Ontology ;
  skos:inScheme     :Ontology .


:172
  a                 skos:Concept ;
  skos:prefLabel    "Work Order"@en ;
  skos:definition   "The Work Order business object includes the identity of the asset, schedule constraints (e.g. done by), prioritisation, work- breakdown-structure (WBS), crew skill requirement, procedure reference, material, tools, services, testing, etc. Here are some Work Order types: • request for maintenance, maintenance order, e.g. refurbish a given power transformer; • request for construction work, e.g. line extension or construction, substation extension or construction; • request for service, service order, e.g. meter reading, meter replacement, turn-on, turn-off; • work request, e.g. forest clearing/thinning; • emergency work, that could be triggered by trouble ticket, or switch request given by network operation."@en ;
  dct:identifier    "urn:uuid:37de49a7-30a4-4298-ce0d-8bfa6c9d37de" ;
  dct:type          archi:BusinessObject ;
  skos:topConceptOf :Ontology ;
  skos:inScheme     :Ontology .


:173
  a                 skos:Concept ;
  skos:prefLabel    "Frequency Response Activation"@en ;
  skos:definition   "The Frequency Response Activation business object includes the description of activation of frequency reserve in regard to correct an over or under frequency event."@en ;
  dct:identifier    "urn:uuid:89a6ce12-50e7-4bc5-beb5-f46fee13b84d" ;
  dct:type          archi:BusinessObject ;
  skos:topConceptOf :Ontology ;
  skos:inScheme     :Ontology .


:174
  a                 skos:Concept ;
  skos:prefLabel    "Control Execution"@en ;
  skos:definition   "The Control Execution business object includes the control commands to remotely operated devices and monitors the responses back to ensure correct operation or create an alarm if the operation fails."@en ;
  dct:identifier    "urn:uuid:a8264ed4-afbb-405d-b859-daa33115c2ad" ;
  dct:type          archi:BusinessObject ;
  skos:topConceptOf :Ontology ;
  skos:inScheme     :Ontology .


:175
  a                 skos:Concept ;
  skos:prefLabel    "Switch Execution"@en ;
  skos:definition   "The Switch Execution business object includes the description of the act of manually opening or closing a switch by a field crew, rather than via remote control"@en ;
  dct:identifier    "urn:uuid:2c637a02-e24e-4d8f-9102-11b8ee74de3e" ;
  dct:type          archi:BusinessObject ;
  skos:topConceptOf :Ontology ;
  skos:inScheme     :Ontology .


:176
  a                 skos:Concept ;
  skos:prefLabel    "Forced Unavailability"@en ;
  skos:definition   "The Forced Unavailability business object includes the description of a piece of equipment's unavailability by the utility owing to operating constraints or in the course of restoring an unplanned outage in the same part of the network"@en ;
  dct:identifier    "urn:uuid:e318c126-9eae-49bc-91b8-8386ff16acc2" ;
  dct:type          archi:BusinessObject ;
  skos:topConceptOf :Ontology ;
  skos:inScheme     :Ontology .


:177
  a                 skos:Concept ;
  skos:prefLabel    "Energy Schedule"@en ;
  skos:definition   "The Energy Schedule business object includes the schedule for consumption (conformed or non-conformed, including demand response), production (primarily intermittent or price inelastic production), direct current and area inter-exchange. This also includes the energy forecast for intermittent or price inelastic production that is part of Distributed Energy Resources (DER)"@en ;
  dct:identifier    "urn:uuid:0087e5ad-bd8e-4b1d-97f2-5f77813f0886" ;
  dct:type          archi:BusinessObject ;
  skos:topConceptOf :Ontology ;
  skos:inScheme     :Ontology .


:178
  a                 skos:Concept ;
  skos:prefLabel    "Real-Time Measurement"@en ;
  skos:definition   "The Real-Time Measurement business object includes measurements from any source. Examples include: – RTU; – PMU;  – ICCP;  – AMI;  – smart devices;  – protection;  – IEC 61850"@en ;
  dct:identifier    "urn:uuid:b1a52dd3-51d0-4a7b-ace7-24c8adb8b2e2" ;
  dct:type          archi:BusinessObject ;
  skos:topConceptOf :Ontology ;
  skos:inScheme     :Ontology .


:179
  a                 skos:Concept ;
  skos:prefLabel    "Post Event Assessment"@en ;
  skos:definition   "The Post Event Assessment business object describes the results of post-event analysis."@en ;
  dct:identifier    "urn:uuid:efd7bce5-9f12-4601-a6b7-0eef0bd79097" ;
  dct:type          archi:BusinessObject ;
  skos:topConceptOf :Ontology ;
  skos:inScheme     :Ontology .


:180
  a                 skos:Concept ;
  skos:prefLabel    "Frequency Restoration Reserve"@en ;
  skos:definition   "The Frequency Restoration Reserve business object is a specialisation of Market Result that describes: • aFRR – automatic frequency restoration reserve;  • mFRR – manual frequency restoration reserve;  • frequency containment reserve – nFCR – normal situation;  • dFCR – frequency containment reserve – disturbed situation"@en ;
  dct:identifier    "urn:uuid:692272f3-a35b-4b8c-9d7e-f28c4e98830c" ;
  dct:type          archi:BusinessObject ;
  skos:topConceptOf :Ontology ;
  skos:inScheme     :Ontology .


:181
  a                 skos:Concept ;
  skos:prefLabel    "Network Operating Event"@en ;
  skos:definition   "The Network Operation Event business object include: • event logs information; that capture outage and other relevant • records for equipment incorrect operation; to ascertain the cause of its • planned and unplanned maintenance data including root cause and repair/replacement details."@en ;
  dct:identifier    "urn:uuid:d18fc9b4-5848-49f2-ba3d-b3a94cb63145" ;
  dct:type          archi:BusinessObject ;
  skos:topConceptOf :Ontology ;
  skos:inScheme     :Ontology .


:182
  a                 skos:Concept ;
  skos:prefLabel    "State Assessment"@en ;
  skos:definition   "The State Assessment business object includes:  • alarms to indicate system failure and response required; • load estimation calculated on a more granular basis than load forecasts, based on specified conditions, weather and other events; • load flow/voltage profile of operating conditions and voltage problems;  the network by predicting and analysing preventing • protective relay setting that can be adjusted based on conditions such as weather and operational conditions; • protective relay analysis to coordinate protective schemes such as opening a breaker after a high current is detected; • weather data to predict impacts on the electrical networks, especially where outages are likely to occur due to heavy storm activity. Temperature and wind speed are sometimes used to calculate dynamic load limits on electrical network assets."@en ;
  dct:identifier    "urn:uuid:8a7f9c91-2e33-4a10-804e-bdab337b02de" ;
  dct:type          archi:BusinessObject ;
  skos:topConceptOf :Ontology ;
  skos:inScheme     :Ontology .


:183
  a                 skos:Concept ;
  skos:prefLabel    "State Evaluation Result"@en ;
  skos:definition   ""@en ;
  dct:identifier    "urn:uuid:acd4dcfd-b2ad-43f5-85ca-876213e0cf8c" ;
  dct:type          archi:BusinessObject ;
  skos:topConceptOf :Ontology ;
  skos:inScheme     :Ontology .


:184
  a                 skos:Concept ;
  skos:prefLabel    "Energy Contract"@en ;
  skos:definition   "The Energy Contract business object includes the conditions for demand response and provision of ancillary services or any other energy contract that is relevant for operational control"@en ;
  dct:identifier    "urn:uuid:04fd2d7c-99b8-412c-bd02-02c932dd1424" ;
  dct:type          archi:BusinessObject ;
  skos:topConceptOf :Ontology ;
  skos:inScheme     :Ontology .


:185
  a                 skos:Concept ;
  skos:prefLabel    "Switch Order"@en ;
  skos:definition   "The Switch Order business object includes a sequence of switch open/close operations, tagging operations, device setting changes, other network operations and safety procedures to change the configuration of the network to achieve a particular business goal. The business goal could be to isolate part of the network in order to allow crews to work safely, to isolate a fault or to optimize the network based on various criteria, for example. Switch Orders can also be used to coordinate live line work safely. The switch order records the result of the switching operations, including who performed the switching and when the switching operation was performed. Both the control room operator and field crews, if any, are recorded with the switch order. This information: • includes a view of all incoming work on the systems. Work details are recorded for each set of switching actions (examination of manual and remote-controlled operations, work characteristics, and crews involved in the work); • provides a view of all switching states in addition to the open or closed state of the switch or device. This includes operational tags used to prevent device operations and safety documents to transfer authority between the control room and field crews."@en ;
  dct:identifier    "urn:uuid:5062b688-3fa8-4986-9c9e-9fb1fb769b5b" ;
  dct:type          archi:BusinessObject ;
  skos:topConceptOf :Ontology ;
  skos:inScheme     :Ontology .


:186
  a                 skos:Concept ;
  skos:prefLabel    "Allocation"@en ;
  skos:definition   "Allocated energy volume from EDSN/CARM. Represents actual consumption calculated from meter readings and profiles."@en ;
  dct:identifier    "urn:uuid:9e9adee6-be94-40b1-587f-b9e2c1e79e9a" ;
  dct:type          archi:BusinessObject ;
  skos:topConceptOf :Ontology ;
  skos:inScheme     :Ontology .


:187
  a                 skos:Concept ;
  skos:prefLabel    "Imbalance"@en ;
  skos:definition   "Difference between allocated energy (actual) and nominated energy (scheduled). Calculated per quarter-hour at T+10 days. Settled at TenneT imbalance price."@en ;
  dct:identifier    "urn:uuid:87d5ccac-3b14-488f-bf6c-da070aaa87d5" ;
  dct:type          archi:BusinessObject ;
  skos:topConceptOf :Ontology ;
  skos:inScheme     :Ontology .


:188
  a                 skos:Concept ;
  skos:prefLabel    "Imbalance Price"@en ;
  skos:definition   "TenneT quarter-hourly pricing for energy imbalances. Price varies based on overall system balance."@en ;
  dct:identifier    "urn:uuid:77dd66f4-b8f4-4d92-2bda-167b36d177dd" ;
  dct:type          archi:BusinessObject ;
  skos:topConceptOf :Ontology ;
  skos:inScheme     :Ontology .


:189
  a                 skos:Concept ;
  skos:prefLabel    "Network Connection Assessment"@en ;
  skos:definition   "The Network Connection Assessment business object describes the result of the evaluation of the Network Connection and includes any dependent modification that is needed to the network grid to support the evaluated Network Connection"@en ;
  dct:identifier    "urn:uuid:6b82db32-fea4-4f99-35b9-bc0ee40c6b82" ;
  dct:type          archi:BusinessObject ;
  skos:topConceptOf :Ontology ;
  skos:inScheme     :Ontology .


:190
  a                 skos:Concept ;
  skos:prefLabel    "Network Situation"@en ;
  skos:definition   "The Network Situation business object includes the description of the operational condition, operational settings and estimated injections on the network. Different situations are defined that should be used in training, simulation/analysis and validation"@en ;
  dct:identifier    "urn:uuid:ceceb96b-b879-4ab6-93ab-54baee33995c" ;
  dct:type          archi:BusinessObject ;
  skos:topConceptOf :Ontology ;
  skos:inScheme     :Ontology .


:191
  a                 skos:Concept ;
  skos:prefLabel    "Network Capacity Assessment"@en ;
  skos:definition   "The Network Capacity Assessment business object includes assessment of the maximum secure capacity of an intact network grid"@en ;
  dct:identifier    "urn:uuid:81ee71f3-8e66-492d-ad27-7f0d7199e388" ;
  dct:type          archi:BusinessObject ;
  skos:topConceptOf :Ontology ;
  skos:inScheme     :Ontology .


:192
  a                 skos:Concept ;
  skos:prefLabel    "Settlement Statement Assessment"@en ;
  skos:definition   "The Settlement Statement Assessment business object describes the result of comparing the billing components/Settlement Statement from another party with the internal calculation based on observation and trading records."@en ;
  dct:identifier    "urn:uuid:9e7e841a-7488-43e5-b29f-74fc39280d71" ;
  dct:type          archi:BusinessObject ;
  skos:topConceptOf :Ontology ;
  skos:inScheme     :Ontology .


:193
  a                 skos:Concept ;
  skos:prefLabel    "Settlement Quality Trade"@en ;
  skos:definition   "The Settlement Quality Trade business object describes the data that meets the quality required by the settlement function defined in the Market Rules.  Settlement data may include the measurement of energy produced and consume, instructions issued by market operators to resources, and the response of market resources to these instructions."@en ;
  dct:identifier    "urn:uuid:fe430a1a-8985-430f-8dad-d44f215cd2dc" ;
  dct:type          archi:BusinessObject ;
  skos:topConceptOf :Ontology ;
  skos:inScheme     :Ontology .


:194
  a                 skos:Concept ;
  skos:prefLabel    "Credit Assessment"@en ;
  skos:definition   "The Credit Assessment business object describes the result of calculating the total debt or financial obligation exposure of a given party"@en ;
  dct:identifier    "urn:uuid:c3ec5ce7-ffa4-40b9-737c-efb3cc9bc3ec" ;
  dct:type          archi:BusinessObject ;
  skos:topConceptOf :Ontology ;
  skos:inScheme     :Ontology .


:195
  a                 skos:Concept ;
  skos:prefLabel    "Price Quote"@en ;
  skos:definition   "Energy price quotation from supplier. Contains forward prices for various delivery periods."@en ;
  dct:identifier    "urn:uuid:fe1cbe6c-18b4-4192-e46c-65b79040fe1c" ;
  dct:type          archi:BusinessObject ;
  skos:topConceptOf :Ontology ;
  skos:inScheme     :Ontology .


:196
  a                 skos:Concept ;
  skos:prefLabel    "External Network Injection"@en ;
  skos:definition   "This class represents the external network.  Represents the TenneT connection point."@en ;
  dct:identifier    "urn:uuid:7a827943-81c6-4db1-b273-6c33e1d2c06d" ;
  dct:type          archi:BusinessObject ;
  skos:topConceptOf :Ontology ;
  skos:inScheme     :Ontology .


:197
  a                 skos:Concept ;
  skos:prefLabel    "Network Connection"@en ;
  skos:definition   "The Network Connection business object describes the conditional requirement for connecting equipment to the network grid.  > dutch relation is: aansluiting > https://vocabs.alliander.com/ESAV/nl/page/55"@en ;
  dct:identifier    "urn:uuid:e77e0d9b-3b0d-4670-979a-10c5dfa29284" ;
  dct:type          archi:BusinessObject ;
  skos:topConceptOf :Ontology ;
  skos:inScheme     :Ontology .


:198
  a                 skos:Concept ;
  skos:prefLabel    "Network Model"@en ;
  skos:definition   "The Network Model business object includes the functional description of the network grid that used in one or more network analysis."@en ;
  dct:identifier    "urn:uuid:a22344b5-1e68-4e03-b627-084dae2f2ec5" ;
  dct:type          archi:BusinessObject ;
  skos:topConceptOf :Ontology ;
  skos:inScheme     :Ontology .


:199
  a                 skos:Concept ;
  skos:prefLabel    "Trouble Ticket"@en ;
  skos:definition   "The Trouble Ticket business object describes the event and/or symptoms that may or may not affect the grid that is reported by a customer or third-party observer. The trouble ticket might be linked to an Incident, Unplanned Customer Outage or in some cases a Planned Customer Outage."@en ;
  dct:identifier    "urn:uuid:c8c88494-5ff1-47ae-85c4-8633ce5d4216" ;
  dct:type          archi:BusinessObject ;
  skos:topConceptOf :Ontology ;
  skos:inScheme     :Ontology .


:200
  a                 skos:Concept ;
  skos:prefLabel    "Network Extention Agreement"@en ;
  skos:definition   "The Network Extension Agreement (or Network Extension Contract) business object is a specialisation of Customer Agreement where the commitment is in relation to extending an existing customer installation or the creation of a new customer installation"@en ;
  dct:identifier    "urn:uuid:aeab83cc-ed97-433b-b4c2-e67cd3061881" ;
  dct:type          archi:BusinessObject ;
  skos:topConceptOf :Ontology ;
  skos:inScheme     :Ontology .


:201
  a                 skos:Concept ;
  skos:prefLabel    "Connection Feasibility"@en ;
  skos:definition   "The Connection Feasibility business object described the result of a feasibility study for connection."@en ;
  dct:identifier    "urn:uuid:58ceecf7-f3ca-4efd-9769-6630a30c6e13" ;
  dct:type          archi:BusinessObject ;
  skos:topConceptOf :Ontology ;
  skos:inScheme     :Ontology .


:202
  a                 skos:Concept ;
  skos:prefLabel    "Customer Inquiry"@en ;
  skos:definition   "The Customer Inquiry business object describes the inquiries from a given customer"@en ;
  dct:identifier    "urn:uuid:4f34c04a-a938-4605-966a-c014a5d5e3f1" ;
  dct:type          archi:BusinessObject ;
  skos:topConceptOf :Ontology ;
  skos:inScheme     :Ontology .


:203
  a                 skos:Concept ;
  skos:prefLabel    "Energy Agreement"@en ;
  skos:definition   "The Energy Agreement (or Energy Contract) business object is a specialisation of Customer Agreement where the commitment is in relation to the delivery of energy to or from a given customer installation and customer. In some cases, this could also describe agreement in regard to active power that is delivered or consumed as well."@en ;
  dct:identifier    "urn:uuid:9a7e6d31-d370-4cfb-95f6-4fda563fac0c" ;
  dct:type          archi:BusinessObject ;
  skos:topConceptOf :Ontology ;
  skos:inScheme     :Ontology .


:204
  a                 skos:Concept ;
  skos:prefLabel    "Customer Agreement"@en ;
  skos:definition   "The Customer Agreement (or Customer Contract) business object describes the commitment between the service provider and a customer.   The agreement describes the aspects of the service in regard to quality, availability and responsibilities.  Agreement between the customer and the service supplier to pay for service at a specific service location. It records certain billing information about the type of service provided at the service location and is used during charge creation to determine the type of service"@en ;
  dct:identifier    "urn:uuid:acf39ca9-27e6-4998-9aca-00bc79da0470" ;
  dct:type          archi:BusinessObject ;
  skos:topConceptOf :Ontology ;
  skos:inScheme     :Ontology .


:205
  a                 skos:Concept ;
  skos:prefLabel    "Customer Installation"@en ;
  skos:definition   "The Customer Installation business object describes the content of the installation on the customer premises in regard to installation, premise, point of delivery and device (e.g. a meter for meter reading) and their location (directly or relative to the connection to the grid)"@en ;
  dct:identifier    "urn:uuid:b82b2db9-8ace-464d-bc0a-50b798a5a7cd" ;
  dct:type          archi:BusinessObject ;
  skos:topConceptOf :Ontology ;
  skos:inScheme     :Ontology .


:206
  a                 skos:Concept ;
  skos:prefLabel    "Grid Connection Agreement"@en ;
  skos:definition   "The Grid Agreement (or Grid Contract) business object is a specialisation of Customer Agreement where the commitment is in relation to the connection into the grid, distribution or transmission."@en ;
  dct:identifier    "urn:uuid:9f8e09ce-6c5b-4774-b705-3faad09974fa" ;
  dct:type          archi:BusinessObject ;
  skos:topConceptOf :Ontology ;
  skos:inScheme     :Ontology .


:207
  a                 skos:Concept ;
  skos:prefLabel    "Customer Energy Programme"@en ;
  skos:definition   "The Customer Energy Programme business object describes the product that a customer can be entered into agreement with. It normally describes a way for a utility to control the customer installation as a reserve for balancing the grid in regard to demand (or in some cases production surplus). The customer is compensated for providing the flexibility and when the flexibility is activated. This could be a demand response product or other power effect control program"@en ;
  dct:identifier    "urn:uuid:24c07f58-fb22-4521-9ae5-25affa9c574a" ;
  dct:type          archi:BusinessObject ;
  skos:topConceptOf :Ontology ;
  skos:inScheme     :Ontology .


:208
  a                 skos:Concept ;
  skos:prefLabel    "Billing Component"@en ;
  skos:definition   "The Billing Component (or Settlement Statement, Customer Settlement Statement or Customer Billing Statement) business object describes the line items that constitute the charges and payment created as part of settling the contract signed with the customer. This provides some of the input to invoicing were pay and receivable and payment agreement is not included"@en ;
  dct:identifier    "urn:uuid:8eb352ba-a3c0-4ef6-b018-4eb13d8861f9" ;
  dct:type          archi:BusinessObject ;
  skos:topConceptOf :Ontology ;
  skos:inScheme     :Ontology .


:209
  a                 skos:Concept ;
  skos:prefLabel    "Compliance Test Plan"@en ;
  skos:definition   "The Compliance Test Plan business object includes legal (e.g. ownership), commercial, (e.g. supplier), financial (e.g. different type of cost), technical and managerial information for substation and network, energy resource (including distributed energy resource (DER)), and non-electrical asset that are included and used in a defence and restoration plan.  Identification of the network function and the physical assets are central items that allow for the retrieval of additional information associated with the asset and its network function."@en ;
  dct:identifier    "urn:uuid:f53fa723-516c-41b8-bf6b-2fc21a583d95" ;
  dct:type          archi:BusinessObject ;
  skos:topConceptOf :Ontology ;
  skos:inScheme     :Ontology .


:210
  a                 skos:Concept ;
  skos:prefLabel    "Compliance Test Result"@en ;
  skos:definition   ""@en ;
  dct:identifier    "urn:uuid:d3cc4951-4ebf-495f-86ed-aea2acdb003f" ;
  dct:type          archi:BusinessObject ;
  skos:topConceptOf :Ontology ;
  skos:inScheme     :Ontology .


:211
  a                 skos:Concept ;
  skos:prefLabel    "Restoration Plan"@en ;
  skos:definition   "The Restoration Plan business object includes the all technical and organisational measures necessary for the restoration of the system back to normal state."@en ;
  dct:identifier    "urn:uuid:84390bf8-d081-4504-99d6-943d04ed161a" ;
  dct:type          archi:BusinessObject ;
  skos:topConceptOf :Ontology ;
  skos:inScheme     :Ontology .


:212
  a                 skos:Concept ;
  skos:prefLabel    "System Defence Plan"@en ;
  skos:definition   ""@en ;
  dct:identifier    "urn:uuid:ae203b5a-c33e-4d65-83a5-29a8ccdf8ce4" ;
  dct:type          archi:BusinessObject ;
  skos:topConceptOf :Ontology ;
  skos:inScheme     :Ontology .


:213
  a                 skos:Concept ;
  skos:prefLabel    "Settlement Quality Assessment"@en ;
  skos:definition   "The Settlement Quality Assessment business object describes the compliance with the observation supervision rules to see if the data is fit for purpose."@en ;
  dct:identifier    "urn:uuid:35172287-c19e-4b8d-87bf-84c543e6f1b4" ;
  dct:type          archi:BusinessObject ;
  skos:topConceptOf :Ontology ;
  skos:inScheme     :Ontology .


:214
  a                 skos:Concept ;
  skos:prefLabel    "Meter Grid Area"@en ;
  skos:definition   "The Meter Grid Area business object includes the description of an electrical area that has metered flow in and out of the area. Only a single entity is responsible for the metering of the area."@en ;
  dct:identifier    "urn:uuid:1c507b6a-fc6d-44a7-839f-949bc766c5b4" ;
  dct:type          archi:BusinessObject ;
  skos:topConceptOf :Ontology ;
  skos:inScheme     :Ontology .


:215
  a                 skos:Concept ;
  skos:prefLabel    "Trade Bit"@en ;
  skos:definition   "The Trade Bid business object can be a bid or an offer on an identified resource and product with a price dependency. The bid/offer can be a curve of quantity of product offered or demanded at different price levels"@en ;
  dct:identifier    "urn:uuid:df7b76df-06a6-4123-9721-3ade60246ee8" ;
  dct:type          archi:BusinessObject ;
  skos:topConceptOf :Ontology ;
  skos:inScheme     :Ontology .


:216
  a                 skos:Concept ;
  skos:prefLabel    "Energy Congestion Zone"@en ;
  skos:definition   "The Energy Congestion Zone business object includes the description of the board of the delivery of energy and capacity market products. Market participants' bids and offers can be cleared without congestion constraints. This is used in a zonal-based market, such as the European-style market"@en ;
  dct:identifier    "urn:uuid:45ad120f-2d28-46bc-a640-f86a85b5d621" ;
  dct:type          archi:BusinessObject ;
  skos:topConceptOf :Ontology ;
  skos:inScheme     :Ontology .


:217
  a                 skos:Concept ;
  skos:prefLabel    "Market Result"@en ;
  skos:definition   "The Market Result business object describes the matched and cleared result of the trading. It includes the identification of resource, product and matched price.  == Settlement Dossier (Market Result)"@en ;
  dct:identifier    "urn:uuid:693088cd-0f08-4676-bb74-7c9ccf8da0cc" ;
  dct:type          archi:BusinessObject ;
  skos:topConceptOf :Ontology ;
  skos:inScheme     :Ontology .


:218
  a                 skos:Concept ;
  skos:prefLabel    "Market Definition"@en ;
  skos:definition   "The Market Definition business object describes the market definition, including products and pricing"@en ;
  dct:identifier    "urn:uuid:dc907d2e-87eb-4791-b8b5-bfc0b5542e27" ;
  dct:type          archi:BusinessObject ;
  skos:topConceptOf :Ontology ;
  skos:inScheme     :Ontology .


:219
  a                 skos:Concept ;
  skos:prefLabel    "Unified Pricing Location"@en ;
  skos:definition   "The Unified Pricing Location business object is a set of network nodes at which energy is injected or withdrawn from the network. The price of energy and ancillary services at each node within a pricing location is the same. The price of energy and ancillary services may be unique at different pricing locations. This is used in a nodal-based market, such as the North American-style market  == CIM: PricingNode"@en ;
  dct:identifier    "urn:uuid:615209a9-9da3-467a-a29c-8d7508109bb1" ;
  dct:type          archi:BusinessObject ;
  skos:topConceptOf :Ontology ;
  skos:inScheme     :Ontology .


:220
  a                 skos:Concept ;
  skos:prefLabel    "Rules Compliance Assessment"@en ;
  skos:definition   "The Compliance Assessment business object describes the entity's compliance to one or more market rules"@en ;
  dct:identifier    "urn:uuid:b2a4aa00-0974-4789-9c6a-02d58929b2a4" ;
  dct:type          archi:BusinessObject ;
  skos:topConceptOf :Ontology ;
  skos:inScheme     :Ontology .


:221
  a                 skos:Concept ;
  skos:prefLabel    "Observation Supervision Rule"@en ;
  skos:definition   "The Observation Supervision Rule business object is a specialization of the Rules that describes the rules which observations that are going to be exchanged need to follow between parties in a compliance market."@en ;
  dct:identifier    "urn:uuid:92f1ff67-3034-41af-bf1b-33ecb81b92f1" ;
  dct:type          archi:BusinessObject ;
  skos:topConceptOf :Ontology ;
  skos:inScheme     :Ontology .


:222
  a                 skos:Concept ;
  skos:prefLabel    "System Operator"@en ;
  skos:definition   "The System Operator business object is a specialization of Entity that describes an entity who is responsible for a stable and balanced power system operation for a given part of the power grid."@en ;
  dct:identifier    "urn:uuid:7e321914-4b7b-4d8e-94d8-49b7b3053ebb" ;
  dct:type          archi:BusinessObject ;
  skos:topConceptOf :Ontology ;
  skos:inScheme     :Ontology .


:223
  a                 skos:Concept ;
  skos:prefLabel    "Rules"@en ;
  skos:definition   "The Rules business object describes the rules that applies to all entities in a given market or inter-party operation. It describes the different roles that can be performed by the different parities to meet the covered compliance"@en ;
  dct:identifier    "urn:uuid:7fb55b59-7adc-49cf-8868-abbe0ef9266b" ;
  dct:type          archi:BusinessObject ;
  skos:topConceptOf :Ontology ;
  skos:inScheme     :Ontology .


:224
  a                 skos:Concept ;
  skos:prefLabel    "Market Participant"@en ;
  skos:definition   "A Market Participant is an entity that participates in one or more energy markets by producing, consuming, trading, or providing flexibility, capacity, or ancillary services."@en ;
  dct:identifier    "urn:uuid:a8f4acc9-ffdc-46e1-9a7c-12d9cd888087" ;
  dct:type          archi:BusinessObject ;
  skos:topConceptOf :Ontology ;
  skos:inScheme     :Ontology .


:225
  a                 skos:Concept ;
  skos:prefLabel    "Observation Provider"@en ;
  skos:definition   ""@en ;
  dct:identifier    "urn:uuid:41cb3643-03d4-448d-5abe-d197109f41cb" ;
  dct:type          archi:BusinessObject ;
  skos:topConceptOf :Ontology ;
  skos:inScheme     :Ontology .


:226
  a                 skos:Concept ;
  skos:prefLabel    "Dispute Resolution Result"@en ;
  skos:definition   ""@en ;
  dct:identifier    "urn:uuid:c10771b2-dd54-41ae-b333-f10d762ec107" ;
  dct:type          archi:BusinessObject ;
  skos:topConceptOf :Ontology ;
  skos:inScheme     :Ontology .


:227
  a                 skos:Concept ;
  skos:prefLabel    "Entity"@en ;
  skos:definition   "The Entity business object describes the role that is governed by compliance."@en ;
  dct:identifier    "urn:uuid:6d585f80-2134-4b9d-b61b-8608da096d58" ;
  dct:type          archi:BusinessObject ;
  skos:topConceptOf :Ontology ;
  skos:inScheme     :Ontology .


:228
  a                 skos:Concept ;
  skos:prefLabel    "Certification"@en ;
  skos:definition   "The Certification business object describe a given entity's compliance with one or more market or supervision rules. An example is the certification of meeting the requirement for acting in the role of metering data provider. "@en ;
  dct:identifier    "urn:uuid:f852cfc8-d1b9-48c8-abbf-2494fa1250d2" ;
  dct:type          archi:BusinessObject ;
  skos:topConceptOf :Ontology ;
  skos:inScheme     :Ontology .


:229
  a                 skos:Concept ;
  skos:prefLabel    "Grid Operator"@en ;
  skos:definition   "The Grid Operator business object is a specialization of Party that describes an entity who is responsible for operating a power grid that provides connection for a customer through a customer connection agreement. The grid operator may operate a high-voltage grid, a distribution-voltage grid, micro- grid or any combination."@en ;
  dct:identifier    "urn:uuid:612fe995-abe4-49bd-b639-38150b8a612f" ;
  dct:type          archi:BusinessObject ;
  skos:topConceptOf :Ontology ;
  skos:inScheme     :Ontology .


:230
  a                 skos:Concept ;
  skos:prefLabel    "Energy Supplier"@en ;
  skos:definition   "The Energy Supplier business object is a specialization of Party that describes an entity who is responsible for providing the energy to a customer in a retail energy market according to the customer energy agreement."@en ;
  dct:identifier    "urn:uuid:aa6b8732-afc4-4496-de25-23ad2188aa6b" ;
  dct:type          archi:BusinessObject ;
  skos:topConceptOf :Ontology ;
  skos:inScheme     :Ontology .


:231
  a                 skos:Concept ;
  skos:prefLabel    "Market Operator"@en ;
  skos:definition   "The Market Operator business object is a specialization of Party that describes an entity who is responsible for operating one or more market places by matching bids and offers and that confirms a trade and/or market prices"@en ;
  dct:identifier    "urn:uuid:c4f4ea04-7ea4-459c-9d14-15477b60c4f4" ;
  dct:type          archi:BusinessObject ;
  skos:topConceptOf :Ontology ;
  skos:inScheme     :Ontology .


:232
  a                 skos:Concept ;
  skos:prefLabel    "Incident"@en ;
  skos:definition   "The Incident business object describes an occurrence in the field that impacts or may impact the network grid. An incident may be reported as part of a trouble ticket. It may or may not be associated with an outage. An Incident is defined as a planned or unplanned interruption or reduction in quality of an service that has the potential to result in a breach or degradation of system state of the grid."@en ;
  dct:identifier    "urn:uuid:a7aa75c1-a0de-4a3c-a58e-f56435f700f9" ;
  dct:type          archi:BusinessObject ;
  skos:topConceptOf :Ontology ;
  skos:inScheme     :Ontology .


:233
  a                 skos:Concept ;
  skos:prefLabel    "Fault Assessment"@en ;
  skos:definition   "The Fault Assessment business object includes the result of analyses data received about the fault, in order to estimate the probable location of the fault."@en ;
  dct:identifier    "urn:uuid:0622cf41-7f25-4113-8a70-adccf00f0db8" ;
  dct:type          archi:BusinessObject ;
  skos:topConceptOf :Ontology ;
  skos:inScheme     :Ontology .


:234
  a                 skos:Concept ;
  skos:prefLabel    "Estimated Restoration Time"@en ;
  skos:definition   "The Estimated Restoration Time business object is the time and date that service is expected to be restored for a particular fault. Estimated Restoration Time can be calculated automatically or can be based on estimates provided by field crews assigned to repairing the fault. The accuracy of Estimated Restoration Time can vary through the course of the lifecycle of each fault."@en ;
  dct:identifier    "urn:uuid:c696ea1a-d866-4da2-9dd3-ba48754e6372" ;
  dct:type          archi:BusinessObject ;
  skos:topConceptOf :Ontology ;
  skos:inScheme     :Ontology .


:235
  a                 skos:Concept ;
  skos:prefLabel    "Field Fault Assessment"@en ;
  skos:definition   "The Field Fault Assessment business object includes the information that is provided by a field crew sent to a predicted fault event. The field crew travels to the predicted location and determines if this is the actual location. If the predicted fault location is confirmed, then the assessment is complete. If the predicted fault location is incorrect, the field crew investigates other possible fault locations and reports the actual fault location, completing the assessment. The field crew may also subsequently report the cause of the fault, if the cause can be determined."@en ;
  dct:identifier    "urn:uuid:90831df9-94ff-48eb-b2a1-3d9c97d88bf1" ;
  dct:type          archi:BusinessObject ;
  skos:topConceptOf :Ontology ;
  skos:inScheme     :Ontology .


:236
  a                 skos:Concept ;
  skos:prefLabel    "Unplanned Customer Outage"@en ;
  skos:definition   "The Unplanned Customer Outage business object describes an unplanned event and the related failure of delivery the customer the committed service in accordance with the customer agreement. The customer may or may not be compensated."@en ;
  dct:identifier    "urn:uuid:b674a9bc-300f-4321-8dd4-7b3b86a653d8" ;
  dct:type          archi:BusinessObject ;
  skos:topConceptOf :Ontology ;
  skos:inScheme     :Ontology .


:237
  a                 skos:Concept ;
  skos:prefLabel    "Predictive Fault Event"@en ;
  skos:definition   "The Predicted Fault Event business object includes the result of Fault Identification analysing input data, such as telemetered values, Trouble Tickets, End Device Events and field Fault Assessment data. The Predicted Fault Event is described by location, faulty equipment and phases."@en ;
  dct:identifier    "urn:uuid:460385e3-108b-47eb-bde2-616b2e5f3be8" ;
  dct:type          archi:BusinessObject ;
  skos:topConceptOf :Ontology ;
  skos:inScheme     :Ontology .


:238
  a                 skos:Concept ;
  skos:prefLabel    "Settlement Quality Observation"@en ;
  skos:definition   "The Settlement Quality Observation business object describes the data that meets the quality required by the settlement \"function defined in the Market Rules. For example, a meter\" reading can include the cumulative kWh value that needs to have the previous meter reading subtracted to calculate the consumption from previous billing components. The consumption value could be considered as settlement ready data that meets the requirement defined in the market rules."@en ;
  dct:identifier    "urn:uuid:bc63cb21-5334-4598-d2eb-096f0176bc63" ;
  dct:type          archi:BusinessObject ;
  skos:topConceptOf :Ontology ;
  skos:inScheme     :Ontology .


:239
  a                 skos:Concept ;
  skos:prefLabel    "End Device Reading"@en ;
  skos:definition   "The End Device Reading business object represents the data that have been acquired by the end device. A meter reading that provides the cumulative kWh value recorded by a meter device from a previous reading, or a meter reading on an hourly resolution for a period are examples of end device readings. A fault reading from a remote fault recorder is also an example of an end device reading"@en ;
  dct:identifier    "urn:uuid:1d6fd339-00f5-4f98-b110-8a2acc15e523" ;
  dct:type          archi:BusinessObject ;
  skos:topConceptOf :Ontology ;
  skos:inScheme     :Ontology .


:240
  a                 skos:Concept ;
  skos:prefLabel    "End Device Configuration"@en ;
  skos:definition   "The End Device Configuration business object describe the configuration of the end device. This can include communication settings, establishing unique identification, control settings, acquisition setting in regard to measurement, accuracy, sampling rate and quality monitoring"@en ;
  dct:identifier    "urn:uuid:a322dd35-05d4-4081-520d-3568a805a322" ;
  dct:type          archi:BusinessObject ;
  skos:topConceptOf :Ontology ;
  skos:inScheme     :Ontology .


:241
  a                 skos:Concept ;
  skos:prefLabel    "Telemeter Fault Signature"@en ;
  skos:definition   "The Telemetered Fault Signature business object includes one or more remotely monitored measurements from sensors that are used to identify the location of a Predicted Fault Event. The Telemetered Fault Signature could be waveform data from a fault recording device, fault passage and direction from fault passage indicator devices, fault distance from a relay, fault current from a relay, the open/close status of a switch or an analogue voltage/flow measurement"@en ;
  dct:identifier    "urn:uuid:d1f41c10-e714-4991-a31f-07f59852d1f4" ;
  dct:type          archi:BusinessObject ;
  skos:topConceptOf :Ontology ;
  skos:inScheme     :Ontology .


:242
  a                 skos:Concept ;
  skos:prefLabel    "End Device Command"@en ;
  skos:definition   "The End Device Command business object represent the command communicated to the end device, e.g. change temperature setting on the air condition"@en ;
  dct:identifier    "urn:uuid:8df23cf7-5ad6-47c8-a238-75c3f225c844" ;
  dct:type          archi:BusinessObject ;
  skos:topConceptOf :Ontology ;
  skos:inScheme     :Ontology .


:243
  a                 skos:Concept ;
  skos:prefLabel    "End Device Event"@en ;
  skos:definition   "The End Device Event business object is information provided by the end device based on the end device configuration and represents the occurrence of an event that has been under monitoring. Meter tampering and grounding error are examples of end device events"@en ;
  dct:identifier    "urn:uuid:438a006a-6f1c-4817-b689-ed7c6111fd40" ;
  dct:type          archi:BusinessObject ;
  skos:topConceptOf :Ontology ;
  skos:inScheme     :Ontology .


:244
  a                 skos:Concept ;
  skos:prefLabel    "Meter Data"@en ;
  skos:definition   "Meter data that are integrated over a period of time before being presented for billing or other purposes."@en ;
  dct:identifier    "urn:uuid:8009eadd-5e18-4a49-9a9d-f89d867fcd0c" ;
  dct:type          archi:BusinessObject ;
  skos:topConceptOf :Ontology ;
  skos:inScheme     :Ontology .


:245
  a                 skos:Concept ;
  skos:prefLabel    "Environment Event"@en ;
  skos:definition   ""@en ;
  dct:identifier    "urn:uuid:dbbf2f05-c2f0-489a-8902-dccb2b5dc639" ;
  dct:type          archi:BusinessObject ;
  skos:topConceptOf :Ontology ;
  skos:inScheme     :Ontology .


:246
  a                 skos:Concept ;
  skos:prefLabel    "Environmental Information"@en ;
  skos:definition   ""@en ;
  dct:identifier    "urn:uuid:55825d50-26ff-4f13-845c-b76eac4e3186" ;
  dct:type          archi:BusinessObject ;
  skos:topConceptOf :Ontology ;
  skos:inScheme     :Ontology .


:247
  a                 skos:Concept ;
  skos:prefLabel    "Environment Alert"@en ;
  skos:definition   ""@en ;
  dct:identifier    "urn:uuid:dbbf2f05-c2f0-489a-8902-dccb2b5dc639" ;
  dct:type          archi:BusinessObject ;
  skos:topConceptOf :Ontology ;
  skos:inScheme     :Ontology .


:248
  a                 skos:Concept ;
  skos:prefLabel    "Environment Forecast"@en ;
  skos:definition   "The Environment Forecast business object includes the estimation of the intensity, nature, and timing of the external forces that may affect the performance of individual assets in the grid or the grid as a whole. This includes forecast or hindcast on: • space (solar flares);  • atmospheric conditions (wind speed gust, humidity etc.);  • geospheric conditions (fire, earthquake etc.);  • hydrospheric conditions (flood level, water temperature, surface temperature etc."@en ;
  dct:identifier    "urn:uuid:498d19e2-bf46-46b7-ab3a-4ef406887b67" ;
  dct:type          archi:BusinessObject ;
  skos:topConceptOf :Ontology ;
  skos:inScheme     :Ontology .


:249
  a                 skos:Concept ;
  skos:prefLabel    "Environmental Inspection Record"@en ;
  skos:definition   ""@en ;
  dct:identifier    "urn:uuid:d0061a47-2848-46ea-963f-533657c181be" ;
  dct:type          archi:BusinessObject ;
  skos:topConceptOf :Ontology ;
  skos:inScheme     :Ontology .


:250
  a                 skos:Concept ;
  skos:prefLabel    "Environment Observation"@en ;
  skos:definition   "The Environment Observation business object describes the recorded environmental data"@en ;
  dct:identifier    "urn:uuid:0a396a40-fc5a-4d44-8077-b38cfdf86dc3" ;
  dct:type          archi:BusinessObject ;
  skos:topConceptOf :Ontology ;
  skos:inScheme     :Ontology .


:251
  a                 skos:Concept ;
  skos:prefLabel    "Asset Maintenance Plan"@en ;
  skos:definition   "The Asset Maintenance Plan business object specifies the activities, resources and timescales required for an individual asset, or a grouping of assets, to achieve the organization’s asset management objectives and prevent expected impact of asset failure."@en ;
  dct:identifier    "urn:uuid:8234c896-eff6-4b07-bafc-409b64089ee4" ;
  dct:type          archi:BusinessObject ;
  skos:topConceptOf :Ontology ;
  skos:inScheme     :Ontology .


:252
  a                 skos:Concept ;
  skos:prefLabel    "Asset Work Record"@en ;
  skos:definition   "The Asset Analytics Result business object includes various analytic scores for the asset, asset type or group of asset (e.g. breakers from a given manufacture) that describe the criticality to the organisation, performance targets or standards, non-conformance criteria, operating cost, replacement value, downtime impact and health assessment"@en ;
  dct:identifier    "urn:uuid:0c680091-f9a0-4610-8a64-8f26ae315d92" ;
  dct:type          archi:BusinessObject ;
  skos:topConceptOf :Ontology ;
  skos:inScheme     :Ontology .


:253
  a                 skos:Concept ;
  skos:prefLabel    "Asset Test Result"@en ;
  skos:definition   "The Asset Analytics Result business object includes various analytic scores for the asset, asset type or group of asset (e.g. breakers from a given manufacture) that describe the criticality to the organisation, performance targets or standards, non-conformance criteria, operating cost, replacement value, downtime impact and health assessment"@en ;
  dct:identifier    "urn:uuid:e51bd60c-ede7-4a23-b5da-94cb6b510805" ;
  dct:type          archi:BusinessObject ;
  skos:topConceptOf :Ontology ;
  skos:inScheme     :Ontology .


:254
  a                 skos:Concept ;
  skos:prefLabel    "Asset Catalogue"@en ;
  skos:definition   "The Asset Catalogue (AC) business object includes the information of asset grouping with relevant specification to provide information on a given set of generic asset material to be used in strategic planning, design/acquisition, operations, maintenance and renewal/disposal."@en ;
  dct:identifier    "urn:uuid:81fe2e25-40cf-4bc3-a93d-58295650e42d" ;
  dct:type          archi:BusinessObject ;
  skos:topConceptOf :Ontology ;
  skos:inScheme     :Ontology .


:255
  a                 skos:Concept ;
  skos:prefLabel    "Asset Maintenance Strategy"@en ;
  skos:definition   "The Asset Maintenance Plan business object specifies the activities, resources and timescales required for an individual asset, or a grouping of assets, to achieve the organization’s asset management objectives and prevent expected impact of asset failure."@en ;
  dct:identifier    "urn:uuid:8234c896-eff6-4b07-bafc-409b64089ee4" ;
  dct:type          archi:BusinessObject ;
  skos:topConceptOf :Ontology ;
  skos:inScheme     :Ontology .


:256
  a                 skos:Concept ;
  skos:prefLabel    "Asset"@en ;
  skos:definition   "An Asset is a tangible resource of the utility, such as power system equipment, end devices, vehicles, tools, cabinets, and buildings. For electrical network equipment, its functional role is modeled using the PowerSystemResource hierarchy defined in the CIM model (IEC 61970). Asset information covers legal (ownership), commercial (supplier), financial (cost types), technical, and managerial aspects. The description emphasizes physical characteristics and lifecycle, while relying on PowerSystemResource for electrical connectivity. Identification numbers (e.g., specification, product, serial) are key for linking additional asset-related data."@en ;
  dct:identifier    "urn:uuid:e81be5a4-4843-4bfe-92ba-53ec88e2c381" ;
  dct:type          archi:BusinessObject ;
  skos:topConceptOf :Ontology ;
  skos:inScheme     :Ontology .


:257
  a                 skos:Concept ;
  skos:prefLabel    "Asset Condition"@en ;
  skos:definition   "The Asset Condition business object describes a given asset or asset type key performance indicators for given operational condition, performance targets or standard, operational safety and reliability assessment."@en ;
  dct:identifier    "urn:uuid:4a6c0ba4-4307-48c6-b192-ca9f4fa7fd14" ;
  dct:type          archi:BusinessObject ;
  skos:topConceptOf :Ontology ;
  skos:inScheme     :Ontology .


:258
  a                 skos:Concept ;
  skos:prefLabel    "Asset Failure"@en ;
  skos:definition   "The Asset Failure business object describes the failure history or statistics associated with a given asset, asset type or asset group (e.g. breakers from a given manufacturer). This includes burnout and accidents."@en ;
  dct:identifier    "urn:uuid:8ff03f43-a43c-41b9-ae43-661496f158d0" ;
  dct:type          archi:BusinessObject ;
  skos:topConceptOf :Ontology ;
  skos:inScheme     :Ontology .


:259
  a                 skos:Concept ;
  skos:prefLabel    "Asset Analytics Result"@en ;
  skos:definition   "The Asset Analytics Result business object includes various analytic scores for the asset, asset type or group of asset (e.g. breakers from a given manufacture) that describe the criticality to the organisation, performance targets or standards, non-conformance criteria, operating cost, replacement value, downtime impact and health assessment"@en ;
  dct:identifier    "urn:uuid:4308e6c3-41ff-4852-8e11-bb2ec44a8fcb" ;
  dct:type          archi:BusinessObject ;
  skos:topConceptOf :Ontology ;
  skos:inScheme     :Ontology .


:260
  a                 skos:Concept ;
  skos:prefLabel    "Asset Compliance Reporting"@en ;
  skos:definition   "The Asset Compliance Reporting business object describes compliance to organisation realisation of asset management in regard to value, efficiency and effectiveness, integrity, execution and leadership against regulatory, standard and business requirements. This could include reporting on compliance to maintenance strategy, maintenance execution, deliverables, and continual improvement. Reporting can be done on individual asset, asset type and asset group in regard to operational, reliability and security standards and regulations. It can also include their impact on the environment in regard to government regulation."@en ;
  dct:identifier    "urn:uuid:5748c930-ed53-4e83-b53d-09263e325870" ;
  dct:type          archi:BusinessObject ;
  skos:topConceptOf :Ontology ;
  skos:inScheme     :Ontology .


:261
  a                 skos:Concept ;
  skos:prefLabel    "Asset Financial Performance"@en ;
  skos:definition   ""@en ;
  dct:identifier    "urn:uuid:e81be5a4-4843-4bfe-92ba-53ec88e2c381" ;
  dct:type          archi:BusinessObject ;
  skos:topConceptOf :Ontology ;
  skos:inScheme     :Ontology .


:262
  a                 skos:Concept ;
  skos:prefLabel    "Budget Allocation"@en ;
  skos:definition   ""@en ;
  dct:identifier    "urn:uuid:7e149677-8184-44ac-5f5f-36b916117e14" ;
  dct:type          archi:BusinessObject ;
  skos:topConceptOf :Ontology ;
  skos:inScheme     :Ontology .


:263
  a                 skos:Concept ;
  skos:prefLabel    "Invoice"@en ;
  skos:definition   ""@en ;
  dct:identifier    "urn:uuid:c198d520-ca34-4496-fc27-1088c873c198" ;
  dct:type          archi:BusinessObject ;
  skos:topConceptOf :Ontology ;
  skos:inScheme     :Ontology .


:264
  a                 skos:Concept ;
  skos:prefLabel    "Flexible Connection Agreement"@en ;
  skos:definition   """"""@en ;
  dct:identifier    "urn:uuid:076b5efc-c803-4320-aa10-dd3bdd2d45fe" ;
  dct:type          archi:BusinessObject ;
  dct:link          <https://vocabs.alliander.com/EURLEX/en/page/944-24c> ;
  skos:topConceptOf :Ontology ;
  skos:inScheme     :Ontology .


:265
  a                 skos:Concept ;
  skos:prefLabel    "Fault"@en ;
  skos:definition   "All types of short-circuits (single-, double- and triple-phase, with and without earth contact), a broken conductor, interrupted circuit, or an intermittent connection, resulting in the permanent non-availability of the affected transmission system element;  "@en ;
  dct:identifier    "urn:uuid:c95d088c-7b46-4a93-b293-d4824c3ebde3" ;
  dct:type          archi:BusinessObject ;
  skos:topConceptOf :Ontology ;
  skos:inScheme     :Ontology .


:266
  a                 skos:Concept ;
  skos:prefLabel    "Consession"@en ;
  skos:definition   "A concession is a contract for works or services, where the right to exploit the works/services is granted to the concessionaire, possibly combined with a payment, and where operational risk is transferred to the economic operator.  📎 Source: Directive 2014/23/EU on the award of concession contracts"@en ;
  dct:identifier    "urn:uuid:c08122b1-64fa-49cb-b44a-11027b0f005e" ;
  dct:type          archi:BusinessObject ;
  skos:topConceptOf :Ontology ;
  skos:inScheme     :Ontology .


:267
  a                 skos:Concept ;
  skos:prefLabel    "Weather Predictions"@en ;
  skos:definition   ""@en ;
  dct:identifier    "urn:uuid:c86cb756-02a5-494b-8635-49eba136c28f" ;
  dct:type          archi:BusinessObject ;
  skos:topConceptOf :Ontology ;
  skos:inScheme     :Ontology .


:268
  a                 skos:Concept ;
  skos:prefLabel    "Control Action Report"@en ;
  skos:definition   "The action control represents the expected capacity behaviour defined by the operating and financial constraints as part of a Settlement. The operating contraint is exchange as a schedule with the Market Participant on a defined RegisteredIntertie. This operating constraint is then related to the EnergyConsumer as ControlAction to make this connectively available for grid-calculations."@en ;
  dct:identifier    "urn:uuid:d69cbb46-105b-4d52-bc42-35b6c78db186" ;
  dct:type          archi:BusinessObject ;
  skos:topConceptOf :Ontology ;
  skos:inScheme     :Ontology .


:269
  a                 skos:Concept ;
  skos:prefLabel    "Operational Security Limit"@en ;
  skos:definition   ""@en ;
  dct:identifier    "urn:uuid:a141e630-5989-4557-b46b-b6e2cf49ad57" ;
  dct:type          archi:BusinessObject ;
  skos:topConceptOf :Ontology ;
  skos:inScheme     :Ontology .


:270
  a                 skos:Concept ;
  skos:prefLabel    "Compliance Report"@en ;
  skos:definition   ""@en ;
  dct:identifier    "urn:uuid:6084f7b0-6dc6-41a5-8a8e-502f5e44951b" ;
  dct:type          archi:BusinessObject ;
  skos:topConceptOf :Ontology ;
  skos:inScheme     :Ontology .


:271
  a                 skos:Concept ;
  skos:prefLabel    "Procurement Agreement"@en ;
  skos:definition   ""@en ;
  dct:identifier    "urn:uuid:747b7fa2-d2b4-44bb-4dda-f49d6098747b" ;
  dct:type          archi:BusinessObject ;
  skos:topConceptOf :Ontology ;
  skos:inScheme     :Ontology .


:272
  a                 skos:Concept ;
  skos:prefLabel    "Consumption Profile"@en ;
  skos:definition   "Standard load profile for allocation. Applied to non-smart-metered connections. Defined by EDSN per customer category."@en ;
  dct:identifier    "urn:uuid:99049072-8ba4-4ca8-6cbe-cb629d959904" ;
  dct:type          archi:BusinessObject ;
  skos:topConceptOf :Ontology ;
  skos:inScheme     :Ontology .


:273
  a                 skos:Concept ;
  skos:prefLabel    "Correction Report"@en ;
  skos:definition   "T+1 year correction report. Typical correction: 5-6% of annual volume. Adjusts for meter corrections, profile updates."@en ;
  dct:identifier    "urn:uuid:a39dfeb7-e5f4-42a8-22e5-cede77fda39d" ;
  dct:type          archi:BusinessObject ;
  skos:topConceptOf :Ontology ;
  skos:inScheme     :Ontology .


:274
  a                 skos:Concept ;
  skos:prefLabel    "Price Quote"@en ;
  skos:definition   "Energy price quotation from supplier. Contains forward prices for various delivery periods."@en ;
  dct:identifier    "urn:uuid:a7d59f2d-2134-49a1-a32c-e3d00236a7d5" ;
  dct:type          archi:BusinessObject ;
  skos:topConceptOf :Ontology ;
  skos:inScheme     :Ontology .


:275
  a                 skos:Concept ;
  skos:prefLabel    "Procurement Contract"@en ;
  skos:definition   "OTC bilateral contract with energy supplier. Duration: 1-4 years. Volume: 1-5 MW blocks. Strategy: 25% rolling quarterly procurement."@en ;
  dct:identifier    "urn:uuid:5de29bb3-01e4-4291-ba1e-36fff17c5de2" ;
  dct:type          archi:BusinessObject ;
  skos:topConceptOf :Ontology ;
  skos:inScheme     :Ontology .


:276
  a                 skos:Concept ;
  skos:prefLabel    "Residual Volume"@en ;
  skos:definition   "Unmatched energy volume after allocation process. Under Allocatie 2.0 (May 2026), assigned to DSO network losses."@en ;
  dct:identifier    "urn:uuid:77c2f1cb-cc04-48b8-9fbb-3b506fca77c2" ;
  dct:type          archi:BusinessObject ;
  skos:topConceptOf :Ontology ;
  skos:inScheme     :Ontology .


:277
  a                 skos:Concept ;
  skos:prefLabel    "Procurement Strategy Policy"@en ;
  skos:definition   ""@en ;
  dct:identifier    "urn:uuid:11a5ab84-8984-4c93-13bc-abf6e97011a5" ;
  dct:type          archi:BusinessObject ;
  skos:topConceptOf :Ontology ;
  skos:inScheme     :Ontology .


:278
  a                 skos:Concept ;
  skos:prefLabel    "Network Loss Volume"@en ;
  skos:definition   "Calculated network loss volume. Annual totals: 1.4 TWh electricity, 35M m³ gas. Value: ~165M EUR."@en ;
  dct:identifier    "urn:uuid:a2220383-7ed4-41b1-6c9b-b9afe91aa222" ;
  dct:type          archi:BusinessObject ;
  skos:topConceptOf :Ontology ;
  skos:inScheme     :Ontology .


:279
  a                 skos:Concept ;
  skos:prefLabel    "Guarantee of Origin (GvO)"@en ;
  skos:definition   "Certificate proving renewable energy source. Purchased to offset network loss CO2 footprint. Represents 92% of Alliander emissions."@en ;
  dct:identifier    "urn:uuid:4381bcb4-5964-49a0-b612-b58cc5734381" ;
  dct:type          archi:BusinessObject ;
  skos:topConceptOf :Ontology ;
  skos:inScheme     :Ontology .


:280
  a                 skos:Concept ;
  skos:prefLabel    "Measurement"@en ;
  skos:definition   "A Measurement is a representation of a quantifiable electrical or operational property of a power system equipment or process, expressed as a value associated with a specific measurement type (e.g., voltage, current, power, status). Within telemetry data collection, a Measurement constitutes the atomic unit of observed data transmitted from end devices, sensors to operational systems.  A Measurement corresponds to the abstract concept defined in IEC 61970-301 (Measurement, Analog, Discrete, Accumulator) that models what is being observed, not the observation itself. It provides:  - the semantic meaning (e.g., this is the phase-A voltage at feeder X), - a reference to a power system resource (e.g., ConductingEquipment, Terminal), - the measurement type, units, and engineering limits, - the link to one or more MeasurementValue instances (actual readings)."@en ;
  dct:identifier    "urn:uuid:6cc290ae-3436-4ece-9cbd-33870e2e87a2" ;
  dct:type          archi:BusinessObject ;
  skos:topConceptOf :Ontology ;
  skos:inScheme     :Ontology .


:281
  a                 skos:Concept ;
  skos:prefLabel    "Measurement Value"@en ;
  skos:definition   "A MeasurementValue is the time-dependent numerical or logical value associated with a Measurement, typically acquired through telemetry, metering systems, or sensors."@en ;
  dct:identifier    "urn:uuid:ddc69b7f-e864-45a2-e5c5-fce60fa8ddc6" ;
  dct:type          archi:BusinessObject ;
  skos:topConceptOf :Ontology ;
  skos:inScheme     :Ontology .


:282
  a                 skos:Concept ;
  skos:prefLabel    "Telemetry Data Point"@en ;
  skos:definition   "A Telemetry Data Point is a single observation consisting of a measured or calculated value, a timestamp, and associated metadata that describes the state of a specific electrical quantity or grid condition at a given moment. It represents the smallest unit of time-series telemetry used for monitoring, analytics, and operational decision-making."@en ;
  dct:identifier    "urn:uuid:d5a4d282-f274-4b8c-f000-60693653d5a4" ;
  dct:type          archi:BusinessObject ;
  skos:topConceptOf :Ontology ;
  skos:inScheme     :Ontology .


:283
  a                 skos:Concept ;
  skos:prefLabel    "Fault Logs"@en ;
  skos:definition   ""@en ;
  dct:identifier    "urn:uuid:4766a996-b916-48ee-94cb-0ca1d74c7560" ;
  dct:type          archi:BusinessObject ;
  skos:topConceptOf :Ontology ;
  skos:inScheme     :Ontology .


:284
  a                 skos:Concept ;
  skos:prefLabel    "Compliance Reports"@en ;
  skos:definition   ""@en ;
  dct:identifier    "urn:uuid:a0fbd1af-e4d7-4141-aeeb-9fcffb0c4b4b" ;
  dct:type          archi:BusinessObject ;
  skos:topConceptOf :Ontology ;
  skos:inScheme     :Ontology .


:285
  a                 skos:Concept ;
  skos:prefLabel    "Restoration Timelines"@en ;
  skos:definition   ""@en ;
  dct:identifier    "urn:uuid:83b84e0d-650e-4082-b1e0-a5bb67356c7e" ;
  dct:type          archi:BusinessObject ;
  skos:topConceptOf :Ontology ;
  skos:inScheme     :Ontology .


:286
  a                 skos:Concept ;
  skos:prefLabel    "Location Estimation"@en ;
  skos:definition   ""@en ;
  dct:identifier    "urn:uuid:384d2563-f239-4966-8409-07a3015fe727" ;
  dct:type          archi:BusinessObject ;
  skos:topConceptOf :Ontology ;
  skos:inScheme     :Ontology .


:287
  a                 skos:Concept ;
  skos:prefLabel    "Fault"@en ;
  skos:definition   ""@en ;
  dct:identifier    "urn:uuid:91ff64ce-8344-479e-425f-e3ee6def91ff" ;
  dct:type          archi:BusinessObject ;
  skos:topConceptOf :Ontology ;
  skos:inScheme     :Ontology .


:288
  a                 skos:Concept ;
  skos:prefLabel    "Unplanned Outage"@en ;
  skos:definition   ""@en ;
  dct:identifier    "urn:uuid:b606cb51-5ef4-4fa7-c37e-5198d493b606" ;
  dct:type          archi:BusinessObject ;
  skos:topConceptOf :Ontology ;
  skos:inScheme     :Ontology .


:289
  a                 skos:Concept ;
  skos:prefLabel    "Environmental Asset Information"@en ;
  skos:definition   "An Asset Conditional Information describes the rule and value, under which conditions to operate a asset."@en ;
  dct:identifier    "urn:uuid:86736515-dce8-4095-996d-09e83348060a" ;
  dct:type          archi:BusinessObject ;
  skos:topConceptOf :Ontology ;
  skos:inScheme     :Ontology .


:290
  a                 skos:Concept ;
  skos:prefLabel    "Technical Asset Information"@en ;
  skos:definition   "Technical Asset Information is the structured set of technical characteristics, states, and constraints of assets, including their interdependencies and relationships with other assets."@en ;
  dct:identifier    "urn:uuid:8d8b9d61-2acd-4a0e-ab35-8dce69c12247" ;
  dct:type          archi:BusinessObject ;
  skos:topConceptOf :Ontology ;
  skos:inScheme     :Ontology .


:291
  a                 skos:Concept ;
  skos:prefLabel    "Transformer Asset Specification"@en ;
  skos:definition   "Technical specifications for network transformers. Includes rated capacity, losses at load levels, efficiency curves."@en ;
  dct:identifier    "urn:uuid:420a2cd4-c5f4-44b2-adca-c40f10ae420a" ;
  dct:type          archi:BusinessObject ;
  skos:topConceptOf :Ontology ;
  skos:inScheme     :Ontology .


:292
  a                 skos:Concept ;
  skos:prefLabel    "End Device Meter"@en ;
  skos:definition   ""@en ;
  dct:identifier    "urn:uuid:b2f9a23d-94ed-4ec8-b64c-6289598c0202" ;
  dct:type          archi:BusinessObject ;
  skos:topConceptOf :Ontology ;
  skos:inScheme     :Ontology .


:293
  a                 skos:Concept ;
  skos:prefLabel    "End Device Asset"@en ;
  skos:definition   "an asset not under control of the DSO and part of the infrastructure of the party connected to the grid."@en ;
  dct:identifier    "urn:uuid:ff7f9039-b724-4582-8286-cf08c09cff7f" ;
  dct:type          archi:BusinessObject ;
  skos:topConceptOf :Ontology ;
  skos:inScheme     :Ontology .


:294
  a                 skos:Concept ;
  skos:prefLabel    "Customer Account"@en ;
  skos:definition   "Assignment of a group of products and services purchased by the customer through a customer agreement, used as a mechanism for customer billing and payment.  It contains common information from the various types of customer agreements to create billings (invoices) for a customer and receive payment."@en ;
  dct:identifier    "urn:uuid:8e3c7e7f-7ab0-4698-8dc3-08e958bb84dc" ;
  dct:type          archi:BusinessObject ;
  skos:topConceptOf :Ontology ;
  skos:inScheme     :Ontology .


:295
  a                 skos:Concept ;
  skos:prefLabel    "Customer contact"@en ;
  skos:definition   ""@en ;
  dct:identifier    "urn:uuid:b4e98487-0a34-479d-3a5b-f010ae30b4e9" ;
  dct:type          archi:BusinessObject ;
  skos:topConceptOf :Ontology ;
  skos:inScheme     :Ontology .


:296
  a                 skos:Concept ;
  skos:prefLabel    "Energy Capacity Needs"@en ;
  skos:definition   ""@en ;
  dct:identifier    "urn:uuid:fc24c2b4-d91b-4f19-bf7e-24d5659de065" ;
  dct:type          archi:BusinessObject ;
  skos:topConceptOf :Ontology ;
  skos:inScheme     :Ontology .


#:297
#  a                 skos:Concept ;
#  skos:prefLabel    ""@en ;
#  skos:definition   ""@en ;
#  dct:identifier    "urn:uuid:36273241-3693-462c-b422-66b8e5afd4be" ;
#
#  dct:type          archi:BusinessObject ;
#  skos:topConceptOf :Ontology ;
#  skos:inScheme     :Ontology .


:298
  a                 skos:Concept ;
  skos:prefLabel    "Pricing Component"@en ;
  skos:definition   ""@en ;
  dct:identifier    "urn:uuid:793fe9c1-7944-4d97-4dce-8f382618793f" ;
  dct:type          archi:BusinessObject ;
  skos:topConceptOf :Ontology ;
  skos:inScheme     :Ontology .


:299
  a                 skos:Concept ;
  skos:prefLabel    "Availability Term"@en ;
  skos:definition   "Availability is the contracted state in which a demand/response resource is ready and capable to be activated, meaning it meets the agreed technical, temporal, and operational conditions (e.g. capacity, response time, and monitoring) during a specified availability window, regardless of whether activation actually occurs."@en ;
  skos:relatedMatch :36, :97 ;
  dct:identifier    "urn:uuid:95ab04f5-4154-4a8e-da4d-c34b5ca595ab" ;
  dct:type          archi:BusinessObject ;
  skos:topConceptOf :Ontology ;
  skos:inScheme     :Ontology .


:300
  a                 skos:Concept ;
  skos:prefLabel    "Activation Term"@en ;
  skos:definition   "Activation is the execution of a contracted flexibility action, whereby an eligible resource increases or decreases demand or generation in response to an operational constrain, within agreed volume, timing, duration, and verification conditions, to support system balance, congestion relief, or security of supply."@en ;
  skos:relatedMatch :36, :97 ;
  dct:identifier    "urn:uuid:ef341459-1dc4-419a-827a-a164988aef34" ;
  dct:type          archi:BusinessObject ;
  skos:topConceptOf :Ontology ;
  skos:inScheme     :Ontology .


:301
  a                 skos:Concept ;
  skos:prefLabel    "Remedial Action Evaluation Report"@en ;
  skos:definition   "The Evalution Action Report is the result of a verificatio process to determine whether a market participant has complied with settlement conditions, such as operating and financial constraints.   -> proposal to rename this: remedial action evaluation report "@en ;
  dct:identifier    "urn:uuid:e9799291-2ce2-4884-942a-dad0024f98e5" ;
  dct:type          archi:BusinessObject ;
  skos:topConceptOf :Ontology ;
  skos:inScheme     :Ontology .


:302
  a                 skos:Concept ;
  skos:prefLabel    "Product Assignment Policies"@en ;
  skos:definition   "The represents policies for mix and match of products within tolopological island.  For compliancy requirements, the policies applied are traceable over time.  "@en ;
  dct:identifier    "urn:uuid:a74f9ffa-093c-4dd1-b458-ac654bf53956" ;
  dct:type          archi:BusinessObject ;
  skos:topConceptOf :Ontology ;
  skos:inScheme     :Ontology .


:303
  a                 skos:Concept ;
  skos:prefLabel    "Capacity Settlement Dossier"@en ;
  skos:definition   "A capacity settlement dossier is the result of cary-out a solution fulfillment for capacity management.    Naming of Settlement is taken from: REDISPATCH & COUNTERTRADE COST SHARING IMPLEMENTATION GUIDE https://eepublicdownloads.entsoe.eu/clean-documents/CIM_documents/Grid_Model_CIM/RD_CT_Cost_Sharing_IG_v1.0.pdf"@en ;
  dct:identifier    "urn:uuid:5d2507ac-0566-4609-9254-543544e9438d" ;
  dct:type          archi:BusinessObject ;
  skos:topConceptOf :Ontology ;
  skos:inScheme     :Ontology .


:304
  a                 skos:Concept ;
  skos:prefLabel    "Bid"@en ;
  skos:definition   "A proposal or tender submitted by a supplier in response to a call for competition. A bid outlines how the supplier will meet the requirements and at what price. In public procurement, submitting a bid means the company is competing for a contract by offering to supply certain goods, services, or works."@en ;
  dct:identifier    "uri:uuid:b447d54c-879e-4dd0-bdcc-1b0ed591f3ee" ;
  dct:type          archi:BusinessObject ;
  foaf:homepage     <https://www.tendify.eu/resources/public-procurement-glossary#bid> ;
  skos:topConceptOf :Ontology ;
  skos:inScheme     :Ontology .


:305
  a                 skos:Concept ;
  skos:prefLabel    "Offer"@en ;
  skos:definition   "Another word for a bid or proposal submitted by a supplier. An offer indicates what the supplier commits to provide (in terms of goods/services) and at what price, under the conditions of the tender. In everyday language, a bidder “makes an offer” to fulfill the contract. (In formal terms, the tender documentation often states that the submitted offer is binding for a certain validity period once the deadline passes.)"@en ;
  dct:identifier    "uri:uuid:defac7b6-ca19-48a6-89db-27ca2389fc3a" ;
  dct:type          archi:BusinessObject ;
  foaf:homepage     <https://www.tendify.eu/resources/public-procurement-glossary#offer> ;
  skos:topConceptOf :Ontology ;
  skos:inScheme     :Ontology .


:306
  a                 skos:Concept ;
  skos:prefLabel    "Validated Bid Stack"@en ;
  skos:definition   ""@en ;
  dct:identifier    "uri:uuid:087d005a-cab9-430e-8c56-77fc90654728" ;
  dct:type          archi:BusinessObject ;
  skos:topConceptOf :Ontology ;
  skos:inScheme     :Ontology .


:307
  a                 skos:Concept ;
  skos:prefLabel    "Equipment Operating Limit"@en ;
  skos:definition   "An Equipment Operating Limit is a generic operational constraint that defines the maximum permissible operating conditions of grid equipment, expressed in physical, electrical, or derived terms, to ensure safe, reliable, and secure operation under defined system conditions."@en ;
  skos:narrower     :133, :308 ;
  dct:identifier    "urn:uuid:90a818be-9005-44c3-85c0-fd6134d7d8ca" ;
  dct:type          archi:BusinessObject ;
  skos:topConceptOf :Ontology ;
  skos:inScheme     :Ontology .


:308
  a                 skos:Concept ;
  skos:prefLabel    "Container Equipment Limit"@en ;
  skos:definition   "A Container Equipment Limit is an operational constraint defined at the level of an equipment container, expressing the maximum allowable combined loading or operational condition of the equipment it contains, derived from underlying conducting-equipment limits or engineering studies, and used to ensure safe and secure operation under defined N and, where applicable, N-1 system conditions, with limits expressed as static or cyclic values."@en ;
  skos:broader      :307 ;
  dct:identifier    "urn:uuid:13014176-f7d4-4dbe-754d-5ca0fcad1301" ;
  dct:type          archi:BusinessObject ;
  skos:topConceptOf :Ontology ;
  skos:inScheme     :Ontology .


:309
  a                  skos:Concept ;
  skos:prefLabel     "Feeder Limit"@en ;
  skos:definition    "A Feeder Limit is an operating constraint applied to a feeder as an equipment container, defining the maximum allowable loading or operating condition of the feeder as a whole—typically expressed in aggregated terms such as current, power, or capacity—and derived from the limits of its underlying conducting elements."@en ;
  skos:editorialNote """Two variants: - H1 :- vooralarm - H2 :- hoofdalarm"""@en ;
  dct:identifier     "urn:uuid:1265405b-a0f4-4e84-3fd3-f8a38f0d1265" ;
  dct:language       "en" ;
  dct:type           archi:BusinessObject ;
  skos:topConceptOf  :Ontology ;
  skos:inScheme      :Ontology .


:310
  a                 skos:Concept ;
  skos:prefLabel    "Meter Acquisition Parameters"@en ;
  skos:definition   "Contains settings for data acquisition such as sampling rate, source ID, etc."@en ;
  dct:identifier    "urn:uuid:bb0e2184-8a2f-4928-bdc9-035a76fc6b38" ;
  dct:type          archi:BusinessObject ;
  skos:topConceptOf :Ontology ;
  skos:inScheme     :Ontology .


:311
  a                 skos:Concept ;
  skos:prefLabel    "Alarm Configuration"@en ;
  skos:definition   "Defines alarm thresholds, types, priorities, and associated actions."@en ;
  dct:identifier    "urn:uuid:dd548026-e6cb-4e37-9f51-c38800896095" ;
  dct:type          archi:BusinessObject ;
  skos:topConceptOf :Ontology ;
  skos:inScheme     :Ontology .


:312
  a                 skos:Concept ;
  skos:prefLabel    "Measurement Definition"@en ;
  skos:definition   "Describes the structure, units, and types of measurements collected."@en ;
  dct:identifier    "urn:uuid:06ad2f5d-384c-4fd6-b6b8-19332aa64d1f" ;
  dct:type          archi:BusinessObject ;
  skos:topConceptOf :Ontology ;
  skos:inScheme     :Ontology .


:313
  a                 skos:Concept ;
  skos:prefLabel    "Quality Constraints"@en ;
  skos:definition   "Specifies rules and thresholds for data accuracy, completeness, and timeliness."@en ;
  dct:identifier    "urn:uuid:000985bd-14df-4ead-9111-11362ed88d18" ;
  dct:type          archi:BusinessObject ;
  skos:topConceptOf :Ontology ;
  skos:inScheme     :Ontology .


:314
  a                 skos:Concept ;
  skos:prefLabel    "Registered Inter Tie"@en ;
  skos:definition   "A RegisteredInterTie is a formally registered interconnection between two grid areas or market zones, representing a recognized interface whose capacity, direction, availability, and constraints are explicitly defined and used for operational planning, market clearing, settlement, and security analysis."@en ;
  dct:identifier    "urn:uuid:ab6f87f9-7f3a-4096-90c1-a91f7db9aa5f" ;
  dct:type          archi:BusinessObject ;
  skos:topConceptOf :Ontology ;
  skos:inScheme     :Ontology .


:315
  a                 skos:Concept ;
  skos:prefLabel    "Registered Resource"@en ;
  skos:definition   "The Registered Resource represents the operational conditions of the D/R product as operated by the Market Participant in order to change the potential behaviour on the point of common coupling (usage point) ."@en ;
  dct:identifier    "urn:uuid:3396fe2e-5e82-4ac6-82b5-9b4d46bae212" ;
  dct:type          archi:BusinessObject ;
  skos:topConceptOf :Ontology ;
  skos:inScheme     :Ontology .


:316
  a                 skos:Concept ;
  skos:prefLabel    "Usage Point"@en ;
  skos:definition   "Logical or physical point in the network to which readings or events may be attributed. Used at the place where a physical or virtual meter may be located; however, it is not required that a meter be present.  ‘Connection point’ means an interface as defined in Article 2 (15) of Regulation (EU) 2016/631.  alias: point-of-common-coupling alias: overdrachtspunt  A Usage Point is reference by a EAN18 identifier in the dutch energy area."@en ;
  dct:identifier    "urn:uuid:7cfbf7a3-a05e-4cf6-85e8-f2d6ef8b0a8e" ;
  dct:type          archi:BusinessObject ;
  skos:topConceptOf :Ontology ;
  skos:inScheme     :Ontology .


:317
  a                 skos:Concept ;
  skos:prefLabel    "Agentic Forecast Prediction Model"@en ;
  skos:definition   "An Agentic Forecast Prediction Model is an autonomous, goal-driven forecasting system composed of cooperating software agents that continuously observe data, select models or actions, adapt assumptions, and refine predictions over time, in order to produce context-aware, explainable forecasts that respond dynamically to changing conditions and feedback."@en ;
  dct:identifier    "urn:uuid:18582fa9-1d04-4ea7-c69b-1cf646721858" ;
  dct:type          archi:BusinessObject ;
  skos:topConceptOf :Ontology ;
  skos:inScheme     :Ontology .


:318
  a                 skos:Concept ;
  skos:prefLabel    "Contingency Study"@en ;
  skos:definition   "A study is a set of analysis and/or solutions with a common purpose performed as part of a single business process.  The study defines the unit-of-work."@en ;
  dct:identifier    "urn:uuid:f81bd8f8-c3fb-423e-9180-8a0cc6225e87" ;
  dct:type          archi:BusinessObject ;
  skos:topConceptOf :Ontology ;
  skos:inScheme     :Ontology .


:319
  a                 skos:Concept ;
  skos:prefLabel    "Scenario Analysis"@en ;
  skos:definition   "A scenario defines the operating parameters, when executing a study on a contingency."@en ;
  dct:identifier    "urn:uuid:0021d4a4-0652-495c-afea-e56261903877" ;
  dct:type          archi:BusinessObject ;
  skos:topConceptOf :Ontology ;
  skos:inScheme     :Ontology .


:320
  a                 skos:Concept ;
  skos:prefLabel    "Sensitivity Scenario"@en ;
  skos:definition   "A Sensitivity Scenario (for grid calculation) is a variant of a base-case network model in which one or more key assumptions are deliberately adjusted—such as load, generation/DER output, interchange, topology/outages, setpoints, or equipment limits—and the resulting case is re-run in a power-flow / contingency / security calculation to quantify how sensitive voltages, line/transformer loadings, losses, and constraint violations are to those changes."@en ;
  dct:identifier    "urn:uuid:53b99b8d-d3e4-4b8c-9900-da9521c153b9" ;
  dct:type          archi:BusinessObject ;
  skos:topConceptOf :Ontology ;
  skos:inScheme     :Ontology .


:321
  a                 skos:Concept ;
  skos:prefLabel    "Capacity Adequacy Sensitivity Result"@en ;
  skos:definition   "A structured result set describing the impact of forecast-driven demand variations on capacity adequacy outcomes for a defined assessment horizon, including derived inputs for loss and network performance predictions."@en ;
  dct:identifier    "urn:uuid:b2fbdbe3-af94-45b0-a4ef-948615deb2fb" ;
  dct:type          archi:BusinessObject ;
  skos:topConceptOf :Ontology ;
  skos:inScheme     :Ontology .


:322
  a                 skos:Concept ;
  skos:prefLabel    "Safety Assessment"@en ;
  skos:definition   "A safety assessment is a result of a performed risk assessment and represents the 'system state' of an analysed part of the grid.   This includes: - the topological island with related equipments,  - the connectivity between these equipments, - the exceedense of the operational limits , - the identified contingency equipments (the one causing the transport limitations) - the allocated operating constrains exchanged with the market-participants  The 'system state' gives direction in the possibility of reaching a solution. Here, the action perspective plays a role and thus also determines the serverity level."@en ;
  dct:identifier    "urn:uuid:6d0b804c-efa3-4c14-b02e-8cc9fed66b4a" ;
  dct:type          archi:BusinessObject ;
  skos:topConceptOf :Ontology ;
  skos:inScheme     :Ontology .


:323
  a                 skos:Concept ;
  skos:prefLabel    "Risk Evaluation Policies"@en ;
  skos:definition   "To determine the risk level and corresponding 'energy system state', like alert state or emergency state policies applied. The specified policies are related to the different equipments and other parts of the grid.   risk = impact * change  drivers for risk determination: - VBM (CAIDI - calculated average interuption duration index) - potential power lost (not relevant for TenneT process integration) - unreliable frequency containment reserve ( due to contingencies in DSO grid) - Low Frequency Demand Disconnect (LFDD) not in an effective state"@en ;
  dct:identifier    "urn:uuid:f9831549-265f-4203-a68b-f18cba81541a" ;
  dct:type          archi:BusinessObject ;
  skos:topConceptOf :Ontology ;
  skos:inScheme     :Ontology .


:324
  a                 skos:Concept ;
  skos:prefLabel    "Reconciliation Record"@en ;
  skos:definition   "Settlement reconciliation at T+10 days. Compares nominations with allocations. Forms basis for imbalance settlement."@en ;
  dct:identifier    "urn:uuid:4386b06d-0024-4fb3-79f0-81df53b74386" ;
  dct:type          archi:BusinessObject ;
  skos:topConceptOf :Ontology ;
  skos:inScheme     :Ontology .


:325
  a                 skos:Concept ;
  skos:prefLabel    "Cost Center"@en ;
  skos:definition   "For each contingency a cost-center is registered for accumulate financial expenses/revenues  to report on."@en ;
  dct:identifier    "urn:uuid:4aef1314-79bd-4f8f-87cb-09844358f224" ;
  dct:type          archi:BusinessObject ;
  skos:topConceptOf :Ontology ;
  skos:inScheme     :Ontology .


:326
  a                 skos:Concept ;
  skos:prefLabel    "Financial Report"@en ;
  skos:definition   ""@en ;
  dct:identifier    "urn:uuid:68642a3b-50d1-487a-a016-d141970555e7" ;
  dct:type          archi:BusinessObject ;
  skos:topConceptOf :Ontology ;
  skos:inScheme     :Ontology .


:327
  a                 skos:Concept ;
  skos:prefLabel    "Regulatory Supervision Rules"@en ;
  skos:definition   ""@en ;
  dct:identifier    "urn:uuid:5f1b77f5-9ae4-44ac-ab52-840a2ac45f1b" ;
  dct:type          archi:BusinessObject ;
  skos:topConceptOf :Ontology ;
  skos:inScheme     :Ontology .

:328
  a                 skos:Concept ;
  skos:prefLabel    "By Order"@en, "Inkoop Order"@nl ;
  skos:definition   """A Redispatch bid whereby the User offers to purchase more electricity or produce less electricity on a specified connection than stated in the Forecast for that connection."""@en,
                    """Een bieding Redispatch waarbij de Gebruiker aanbiedt om op een gespecificeerde aansluiting meer elektriciteit af te nemen dan wel minder elektriciteit te produceren dan opgegeven in de prognose voor die aansluiting."""@nl ;
  skos:broader      :332 ;
  dct:identifier    "urn:uuid:82a98ee0-eecb-437b-aca2-13d0a40b9f85" ;
  dct:source        "GOPACS" ;
  dct:type          archi:BusinessObject ;
  skos:topConceptOf :Ontology ;
  skos:inScheme     :Ontology .


:329
  a                 skos:Concept ;
  skos:prefLabel    "Capacity Limitation"@en, "Capaciteitsbeperking"@nl ;
  skos:definition   """The situation in which a User waives the use of its (contracted) transmission capacity during an agreed period at the request of the Grid Operator."""@en,
                    """De situatie waarin een Gebruiker op verzoek van netbeheerder afziet van het gebruik van zijn (gecontracteerde) transportvermogen gedurende een afgesproken periode. Wettelijk product vastgelegd in bijlage 12 van Netcode Elektriciteit."""@nl ;
  dct:identifier    "urn:uuid:82a98ee0-eecb-437b-aca2-13d0a40b9f85" ;
  dct:source        "GOPACS" ;
  skos:topConceptOf :Ontology ;
  skos:inScheme     :Ontology .

:330
  a                 skos:Concept ;
  skos:prefLabel    "Congestion Area"@en, "Congestiegebied"@nl ;
  skos:definition   """A defined area where there may be or is a shortage of available transmission capacity and the Grid Operator has placed a (pre)announcement."""@en,
                    """Een afgebakend gebied waarbij sprake kan zijn of is van een tekort aan beschikbare transportcapaciteit en de netbeheerder een (voor)aankondiging heeft geplaatst."""@nl ;
  dct:identifier    "urn:uuid:7aed277a-2846-46a2-893b-c631aefeb484" ;
  dct:source        "GOPACS" ;
  skos:topConceptOf :Ontology ;
  skos:inScheme     :Ontology .

:330
  a                 skos:Concept ;
  skos:prefLabel    "Clearing Price"@en, "Clearingprijs"@nl ;
  skos:altLabel     "Evenwichtsprijs"@nl ;
  skos:definition   """"""@en,
                    """De door de CSP opgegeven prijs van een Buy Order of Sell Order. De prijs waarbij de totale ingediende biedingen (aanbod) gelijk zijn aan de totale gevraagde volumes (vraag)."""@nl ;
  skos:editorialNote
                    "In Nederland gebruiken energie- en financiële markten de term clearingprijs het meest, soms ook evenwichtsprijs als meer economische term."@nl ;
  dct:identifier    "urn:" ;
  dct:source        "GOPACS" ;
  skos:topConceptOf :Ontology ;
  skos:inScheme     :Ontology .

:331
  a                 skos:Concept ;
  skos:prefLabel    "Redispatch"@en, ""@nl ;
  skos:definition   """A modification of the generation and/or load inputs on connections as a result of activation of one or more Buy Order(s) and one or more Sell Order(s), as further defined in Section 5.1 of these Product Conditions, for the purpose of resolving congestion in the network."""@en,
                    """"""@nl ;
  dct:identifier    "urn:uuid:91c2cba4-9f83-4c3e-9851-ecddf9dc93da" ;
  dct:source        "GOPACS" ;
  skos:topConceptOf :Ontology ;
  skos:inScheme     :Ontology .

:332
  a                 skos:Concept ;
  skos:prefLabel    "Order"@en, "Order"@nl ;
  skos:definition   """"""@en, """"""@nl ;
  skos:broader      :333 ;
  dct:identifier    "urn:uuid:73a9a357-1f0b-4473-ab12-6b7e36a8766a" ;
  dct:source        "GOPACS" ;
  skos:topConceptOf :Ontology ;
  skos:inScheme     :Ontology .

:333
  a                 skos:Concept ;
  skos:prefLabel    "Sel Order"@en, ""@nl ;
  skos:definition   """A Redispatch bid whereby the User offers to purchase less electricity or produce more electricity on a specified connection than specified in the Forecast for that connection."""@en,
                    """Een bieding Redispatch waarbij de Gebruiker aanbiedt om op een gespecificeerde aansluiting minder elektriciteit af te nemen dan wel meer elektriciteit te produceren dan opgegeven in de prognose voor die aansluiting"""@nl ;
  skos:narrower     :332 ;
  dct:identifier    "urn:uuid:be957842-21f0-4b2c-807e-b35be5da24b1" ;
  dct:source        "GOPACS" ;
  skos:topConceptOf :Ontology ;
  skos:inScheme     :Ontology .

:334
  a                 skos:Concept ;
  skos:prefLabel    "Spread"@en, "Spread"@nl ;
  skos:definition   """The price difference between one or more Buy Order(s) and one or more Sell Order(s) which determines the cost to the Grid Operator linked to congestion resolution."""@en,
                    """Het prijsverschil tussen een of meerdere Buy Order(s) en een of meerdere Sell Order(s) wat de kosten voor de Netbeheer bepaalt gekoppeld aan het oplossen van congestie."""@nl ;
  dct:identifier    "urn:uuid:2e0785d2-37c2-4dea-93cd-61b9e4dbab5b" ;
  dct:source        "GOPACS" ;
  skos:topConceptOf :Ontology ;
  skos:inScheme     :Ontology .

:335
  a                 skos:Concept ;
  skos:prefLabel    "Procurement"@en, "Inkoop"@nl ;
  skos:definition   """The process of acquiring goods, services, or works from external sources. This encompasses the entire cycle from identifying needs, specifying requirements, and tendering, to evaluating offers, awarding a contract, and managing the contract. In a general sense, “procurement” can refer to any organization’s purchasing process. In public procurement, the process must adhere to principles of transparency, competition, and value for money as set out in law."""@en,
                    """"""@nl ;
  dct:identifier    "urn:uuid:17e22e52-535e-4a94-ad63-e41c9af520cc" ;
  foaf:homepage     <https://www.tendify.eu/resources/public-procurement-glossary#procurement> ;
  skos:topConceptOf :Ontology ;
  skos:inScheme     :Ontology .

#:<number>
#  a                 skos:Concept ;
#  skos:prefLabel    ""@en, ""@nl ;
#  skos:definition   """"""@en,
#                    """"""@nl ;
#  dct:identifier    "urn:" ;
#  dct:source        "" ;
#  skos:topConceptOf :Ontology ;
#  skos:inScheme     :Ontology .
#
